<?xml version="1.0"?>
<rdf:RDF xmlns="http://purl.obolibrary.org/obo/foodon/imports/robot_process_import.owl#"
     xml:base="http://purl.obolibrary.org/obo/foodon/imports/robot_process_import.owl"
     xmlns:obo="http://purl.obolibrary.org/obo/"
     xmlns:owl="http://www.w3.org/2002/07/owl#"
     xmlns:rdf="http://www.w3.org/1999/02/22-rdf-syntax-ns#"
     xmlns:xml="http://www.w3.org/XML/1998/namespace"
     xmlns:xsd="http://www.w3.org/2001/XMLSchema#"
     xmlns:rdfs="http://www.w3.org/2000/01/rdf-schema#"
     xmlns:oboInOwl="http://www.geneontology.org/formats/oboInOwl#">
    <owl:Ontology rdf:about="http://purl.obolibrary.org/obo/foodon/imports/robot_process_import.owl"/>
    


    <!-- 
    ///////////////////////////////////////////////////////////////////////////////////////
    //
    // Annotation properties
    //
    ///////////////////////////////////////////////////////////////////////////////////////
     -->

    


    <!-- http://purl.obolibrary.org/obo/IAO_0000114 -->

    <owl:AnnotationProperty rdf:about="http://purl.obolibrary.org/obo/IAO_0000114"/>
    


    <!-- http://purl.obolibrary.org/obo/IAO_0000115 -->

    <owl:AnnotationProperty rdf:about="http://purl.obolibrary.org/obo/IAO_0000115"/>
    


    <!-- http://purl.obolibrary.org/obo/IAO_0000117 -->

    <owl:AnnotationProperty rdf:about="http://purl.obolibrary.org/obo/IAO_0000117"/>
    


    <!-- http://purl.obolibrary.org/obo/IAO_0000119 -->

    <owl:AnnotationProperty rdf:about="http://purl.obolibrary.org/obo/IAO_0000119"/>
    


    <!-- http://www.geneontology.org/formats/oboInOwl#hasDbXref -->

    <owl:AnnotationProperty rdf:about="http://www.geneontology.org/formats/oboInOwl#hasDbXref"/>
    


    <!-- http://www.geneontology.org/formats/oboInOwl#hasExactSynonym -->

    <owl:AnnotationProperty rdf:about="http://www.geneontology.org/formats/oboInOwl#hasExactSynonym"/>
    


    <!-- http://www.geneontology.org/formats/oboInOwl#hasNarrowSynonym -->

    <owl:AnnotationProperty rdf:about="http://www.geneontology.org/formats/oboInOwl#hasNarrowSynonym"/>
    


    <!-- http://www.geneontology.org/formats/oboInOwl#hasSynonym -->

    <owl:AnnotationProperty rdf:about="http://www.geneontology.org/formats/oboInOwl#hasSynonym"/>
    


    <!-- 
    ///////////////////////////////////////////////////////////////////////////////////////
    //
    // Object Properties
    //
    ///////////////////////////////////////////////////////////////////////////////////////
     -->

    


    <!-- http://purl.obolibrary.org/obo/RO_0002233 -->

    <owl:ObjectProperty rdf:about="http://purl.obolibrary.org/obo/RO_0002233"/>
    


    <!-- http://purl.obolibrary.org/obo/RO_0002234 -->

    <owl:ObjectProperty rdf:about="http://purl.obolibrary.org/obo/RO_0002234"/>
    


    <!-- 
    ///////////////////////////////////////////////////////////////////////////////////////
    //
    // Classes
    //
    ///////////////////////////////////////////////////////////////////////////////////////
     -->

    


    <!-- http://purl.obolibrary.org/obo/BFO_0000015 -->

    <owl:Class rdf:about="http://purl.obolibrary.org/obo/BFO_0000015">
        <rdfs:label xml:lang="en">process</rdfs:label>
    </owl:Class>
    


    <!-- http://purl.obolibrary.org/obo/FOODON_00000071 -->

    <owl:Class rdf:about="http://purl.obolibrary.org/obo/FOODON_00000071">
        <rdfs:subClassOf rdf:resource="http://purl.obolibrary.org/obo/FOODON_03460130"/>
        <obo:IAO_0000115 xml:lang="en">A process of cutting food into smaller pieces, chunks or slices.</obo:IAO_0000115>
        <obo:IAO_0000117 rdf:datatype="http://www.w3.org/2001/XMLSchema#string">Damion Dooley</obo:IAO_0000117>
        <rdfs:label xml:lang="en">food cutting process</rdfs:label>
    </owl:Class>
    


    <!-- http://purl.obolibrary.org/obo/FOODON_00001181 -->

    <owl:Class rdf:about="http://purl.obolibrary.org/obo/FOODON_00001181"/>
    


    <!-- http://purl.obolibrary.org/obo/FOODON_00001258 -->

    <owl:Class rdf:about="http://purl.obolibrary.org/obo/FOODON_00001258"/>
    


    <!-- http://purl.obolibrary.org/obo/FOODON_00001304 -->

    <owl:Class rdf:about="http://purl.obolibrary.org/obo/FOODON_00001304">
        <rdfs:subClassOf rdf:resource="http://purl.obolibrary.org/obo/FOODON_03460119"/>
        <rdfs:subClassOf rdf:resource="http://purl.obolibrary.org/obo/FOODON_03470107"/>
        <rdfs:subClassOf>
            <owl:Restriction>
                <owl:onProperty rdf:resource="http://purl.obolibrary.org/obo/RO_0002234"/>
                <owl:someValuesFrom rdf:resource="http://purl.obolibrary.org/obo/FOODON_00001258"/>
            </owl:Restriction>
        </rdfs:subClassOf>
        <obo:IAO_0000115 xml:lang="en">A fermentation process in which either carbohydrates, proteins or fats are modified through microbial, enzymatic and/or other biological process.</obo:IAO_0000115>
        <obo:IAO_0000117 rdf:datatype="http://www.w3.org/2001/XMLSchema#string">Damion Dooley</obo:IAO_0000117>
        <rdfs:label xml:lang="en">food fermentation</rdfs:label>
    </owl:Class>
    


    <!-- http://purl.obolibrary.org/obo/FOODON_00001868 -->

    <owl:Class rdf:about="http://purl.obolibrary.org/obo/FOODON_00001868">
        <rdfs:label xml:lang="en">food filling product</rdfs:label>
    </owl:Class>
    


    <!-- http://purl.obolibrary.org/obo/FOODON_00002403 -->

    <owl:Class rdf:about="http://purl.obolibrary.org/obo/FOODON_00002403">
        <rdfs:label xml:lang="en">food material</rdfs:label>
    </owl:Class>
    


    <!-- http://purl.obolibrary.org/obo/FOODON_00002404 -->

    <owl:Class rdf:about="http://purl.obolibrary.org/obo/FOODON_00002404">
        <rdfs:subClassOf rdf:resource="http://purl.obolibrary.org/obo/FOODON_03450005"/>
        <obo:IAO_0000115 xml:lang="en">Roasting is a baking process when the food being baked is meats</obo:IAO_0000115>
        <obo:IAO_0000117 rdf:datatype="http://www.w3.org/2001/XMLSchema#string">Damion Dooley</obo:IAO_0000117>
        <rdfs:label xml:lang="en">meat roasting</rdfs:label>
    </owl:Class>
    


    <!-- http://purl.obolibrary.org/obo/FOODON_00002409 -->

    <owl:Class rdf:about="http://purl.obolibrary.org/obo/FOODON_00002409">
        <rdfs:subClassOf rdf:resource="http://purl.obolibrary.org/obo/FOODON_03460130"/>
        <obo:IAO_0000115 xml:lang="en">Modification through physical treatment to affect the shape quality of a food product.</obo:IAO_0000115>
        <obo:IAO_0000117 rdf:datatype="http://www.w3.org/2001/XMLSchema#string">Damion Dooley</obo:IAO_0000117>
        <rdfs:label xml:lang="en">food physical forming process</rdfs:label>
    </owl:Class>
    


    <!-- http://purl.obolibrary.org/obo/FOODON_00002414 -->

    <owl:Class rdf:about="http://purl.obolibrary.org/obo/FOODON_00002414">
        <rdfs:subClassOf rdf:resource="http://purl.obolibrary.org/obo/FOODON_03460130"/>
        <obo:IAO_0000115 xml:lang="en">Extraction of substance(s) from a food source using a solvent such as alcohol, hexane, or ethanol.</obo:IAO_0000115>
        <obo:IAO_0000117 rdf:datatype="http://www.w3.org/2001/XMLSchema#string">Damion Dooley</obo:IAO_0000117>
        <rdfs:label xml:lang="en">food solvent extraction process</rdfs:label>
    </owl:Class>
    


    <!-- http://purl.obolibrary.org/obo/FOODON_00002415 -->

    <owl:Class rdf:about="http://purl.obolibrary.org/obo/FOODON_00002415">
        <rdfs:subClassOf rdf:resource="http://purl.obolibrary.org/obo/FOODON_00002409"/>
        <rdfs:subClassOf>
            <owl:Restriction>
                <owl:onProperty rdf:resource="http://purl.obolibrary.org/obo/RO_0002234"/>
                <owl:someValuesFrom rdf:resource="http://purl.obolibrary.org/obo/FOODON_00002649"/>
            </owl:Restriction>
        </rdfs:subClassOf>
        <obo:IAO_0000115 xml:lang="en">The process of milling grain into flour, usually performed by a grist mill, corn mill or flour mill.</obo:IAO_0000115>
        <obo:IAO_0000117 rdf:datatype="http://www.w3.org/2001/XMLSchema#string">Damion Dooley</obo:IAO_0000117>
        <rdfs:label xml:lang="en">food milling process</rdfs:label>
    </owl:Class>
    


    <!-- http://purl.obolibrary.org/obo/FOODON_00002416 -->

    <owl:Class rdf:about="http://purl.obolibrary.org/obo/FOODON_00002416">
        <rdfs:subClassOf rdf:resource="http://purl.obolibrary.org/obo/FOODON_03460130"/>
        <rdfs:subClassOf>
            <owl:Restriction>
                <owl:onProperty rdf:resource="http://purl.obolibrary.org/obo/RO_0002234"/>
                <owl:someValuesFrom rdf:resource="http://purl.obolibrary.org/obo/FOODON_00002418"/>
            </owl:Restriction>
        </rdfs:subClassOf>
        <obo:IAO_0000117 rdf:datatype="http://www.w3.org/2001/XMLSchema#string">Damion Dooley</obo:IAO_0000117>
        <rdfs:label xml:lang="en">food canning process</rdfs:label>
    </owl:Class>
    


    <!-- http://purl.obolibrary.org/obo/FOODON_00002418 -->

    <owl:Class rdf:about="http://purl.obolibrary.org/obo/FOODON_00002418"/>
    


    <!-- http://purl.obolibrary.org/obo/FOODON_00002419 -->

    <owl:Class rdf:about="http://purl.obolibrary.org/obo/FOODON_00002419">
        <rdfs:subClassOf rdf:resource="http://purl.obolibrary.org/obo/FOODON_03460130"/>
        <obo:IAO_0000115 xml:lang="en">A food evaporation process is the process of removing water from a food.</obo:IAO_0000115>
        <obo:IAO_0000117 rdf:datatype="http://www.w3.org/2001/XMLSchema#string">Damion Dooley</obo:IAO_0000117>
        <rdfs:label xml:lang="en">food evaporation process</rdfs:label>
    </owl:Class>
    


    <!-- http://purl.obolibrary.org/obo/FOODON_00002451 -->

    <owl:Class rdf:about="http://purl.obolibrary.org/obo/FOODON_00002451">
        <rdfs:subClassOf rdf:resource="http://purl.obolibrary.org/obo/BFO_0000015"/>
        <rdfs:subClassOf>
            <owl:Restriction>
                <owl:onProperty rdf:resource="http://purl.obolibrary.org/obo/RO_0002234"/>
                <owl:someValuesFrom rdf:resource="http://purl.obolibrary.org/obo/FOODON_00002403"/>
            </owl:Restriction>
        </rdfs:subClassOf>
        <obo:IAO_0000114 rdf:datatype="http://www.w3.org/2001/XMLSchema#string">requires discussion</obo:IAO_0000114>
        <obo:IAO_0000115 xml:lang="en">A process involving the physical transformation of a food source or food product into some derived organic material or food product</obo:IAO_0000115>
        <obo:IAO_0000117 rdf:datatype="http://www.w3.org/2001/XMLSchema#string">Damion Dooley</obo:IAO_0000117>
        <rdfs:label xml:lang="en">food transformation process</rdfs:label>
    </owl:Class>
    


    <!-- http://purl.obolibrary.org/obo/FOODON_00002456 -->

    <owl:Class rdf:about="http://purl.obolibrary.org/obo/FOODON_00002456"/>
    


    <!-- http://purl.obolibrary.org/obo/FOODON_00002462 -->

    <owl:Class rdf:about="http://purl.obolibrary.org/obo/FOODON_00002462">
        <rdfs:subClassOf rdf:resource="http://purl.obolibrary.org/obo/FOODON_03450026"/>
        <rdfs:subClassOf>
            <owl:Restriction>
                <owl:onProperty rdf:resource="http://purl.obolibrary.org/obo/RO_0002234"/>
                <owl:someValuesFrom rdf:resource="http://purl.obolibrary.org/obo/FOODON_00002660"/>
            </owl:Restriction>
        </rdfs:subClassOf>
        <obo:IAO_0000115 xml:lang="en">A form of frying characterized by the use of minimal cooking oil or fat (compared to shallow frying or deep frying); typically using just enough oil to lubricate the pan. A pan fry takes place at lower heat than does a sauté.</obo:IAO_0000115>
        <obo:IAO_0000117 rdf:datatype="http://www.w3.org/2001/XMLSchema#string">Damion Dooley</obo:IAO_0000117>
        <rdfs:label xml:lang="en">pan frying</rdfs:label>
    </owl:Class>
    


    <!-- http://purl.obolibrary.org/obo/FOODON_00002648 -->

    <owl:Class rdf:about="http://purl.obolibrary.org/obo/FOODON_00002648">
        <rdfs:subClassOf rdf:resource="http://purl.obolibrary.org/obo/FOODON_03450002"/>
        <obo:IAO_0000115 xml:lang="en">A method of precooking food where a liquid is heated to just below the boiling point. Often used to retard the spoiling of milk.</obo:IAO_0000115>
        <obo:IAO_0000117 rdf:datatype="http://www.w3.org/2001/XMLSchema#string">Damion Dooley</obo:IAO_0000117>
        <oboInOwl:hasExactSynonym xml:lang="en">scalding</oboInOwl:hasExactSynonym>
        <rdfs:label xml:lang="en">food scalding</rdfs:label>
    </owl:Class>
    


    <!-- http://purl.obolibrary.org/obo/FOODON_00002649 -->

    <owl:Class rdf:about="http://purl.obolibrary.org/obo/FOODON_00002649"/>
    


    <!-- http://purl.obolibrary.org/obo/FOODON_00002655 -->

    <owl:Class rdf:about="http://purl.obolibrary.org/obo/FOODON_00002655"/>
    


    <!-- http://purl.obolibrary.org/obo/FOODON_00002657 -->

    <owl:Class rdf:about="http://purl.obolibrary.org/obo/FOODON_00002657"/>
    


    <!-- http://purl.obolibrary.org/obo/FOODON_00002659 -->

    <owl:Class rdf:about="http://purl.obolibrary.org/obo/FOODON_00002659"/>
    


    <!-- http://purl.obolibrary.org/obo/FOODON_00002660 -->

    <owl:Class rdf:about="http://purl.obolibrary.org/obo/FOODON_00002660"/>
    


    <!-- http://purl.obolibrary.org/obo/FOODON_00002688 -->

    <owl:Class rdf:about="http://purl.obolibrary.org/obo/FOODON_00002688"/>
    


    <!-- http://purl.obolibrary.org/obo/FOODON_00002707 -->

    <owl:Class rdf:about="http://purl.obolibrary.org/obo/FOODON_00002707">
        <rdfs:subClassOf rdf:resource="http://purl.obolibrary.org/obo/FOODON_03460130"/>
        <rdfs:subClassOf>
            <owl:Restriction>
                <owl:onProperty rdf:resource="http://purl.obolibrary.org/obo/RO_0002234"/>
                <owl:someValuesFrom rdf:resource="http://purl.obolibrary.org/obo/FOODON_00002708"/>
            </owl:Restriction>
        </rdfs:subClassOf>
        <obo:IAO_0000115 xml:lang="en">The process of cleaning food to separate other environmental materials or body substances.</obo:IAO_0000115>
        <obo:IAO_0000117 rdf:datatype="http://www.w3.org/2001/XMLSchema#string">Damion Dooley</obo:IAO_0000117>
        <rdfs:label xml:lang="en">food cleaning process</rdfs:label>
    </owl:Class>
    


    <!-- http://purl.obolibrary.org/obo/FOODON_00002708 -->

    <owl:Class rdf:about="http://purl.obolibrary.org/obo/FOODON_00002708"/>
    


    <!-- http://purl.obolibrary.org/obo/FOODON_00002720 -->

    <owl:Class rdf:about="http://purl.obolibrary.org/obo/FOODON_00002720"/>
    


    <!-- http://purl.obolibrary.org/obo/FOODON_00002721 -->

    <owl:Class rdf:about="http://purl.obolibrary.org/obo/FOODON_00002721">
        <rdfs:subClassOf rdf:resource="http://purl.obolibrary.org/obo/FOODON_03460238"/>
        <rdfs:subClassOf>
            <owl:Restriction>
                <owl:onProperty rdf:resource="http://purl.obolibrary.org/obo/RO_0002234"/>
                <owl:someValuesFrom rdf:resource="http://purl.obolibrary.org/obo/FOODON_00002720"/>
            </owl:Restriction>
        </rdfs:subClassOf>
        <obo:IAO_0000115 xml:lang="en">Dehulling is the process of removing the hulls (or chaff) from beans and other seeds.</obo:IAO_0000115>
        <obo:IAO_0000117 rdf:datatype="http://www.w3.org/2001/XMLSchema#string">Damion Dooley</obo:IAO_0000117>
        <rdfs:label xml:lang="en">food dehulling process</rdfs:label>
    </owl:Class>
    


    <!-- http://purl.obolibrary.org/obo/FOODON_00002722 -->

    <owl:Class rdf:about="http://purl.obolibrary.org/obo/FOODON_00002722">
        <rdfs:subClassOf rdf:resource="http://purl.obolibrary.org/obo/FOODON_03460238"/>
        <obo:IAO_0000115 xml:lang="en">Husking of corn is the process of removing its outer layers, leaving only the cob or seed rack of the corn</obo:IAO_0000115>
        <obo:IAO_0000117 rdf:datatype="http://www.w3.org/2001/XMLSchema#string">Damion Dooley</obo:IAO_0000117>
        <oboInOwl:hasExactSynonym xml:lang="en">husking</oboInOwl:hasExactSynonym>
        <rdfs:label xml:lang="en">corn husking process</rdfs:label>
    </owl:Class>
    


    <!-- http://purl.obolibrary.org/obo/FOODON_00002732 -->

    <owl:Class rdf:about="http://purl.obolibrary.org/obo/FOODON_00002732">
        <rdfs:subClassOf rdf:resource="http://purl.obolibrary.org/obo/FOODON_03460225"/>
        <obo:IAO_0000115 xml:lang="en">A process of applying a seasoning mixture to a given food.</obo:IAO_0000115>
        <obo:IAO_0000117 rdf:datatype="http://www.w3.org/2001/XMLSchema#string">Damion Dooley</obo:IAO_0000117>
        <oboInOwl:hasExactSynonym xml:lang="en">seasoning</oboInOwl:hasExactSynonym>
        <rdfs:label xml:lang="en">food seasoning process</rdfs:label>
    </owl:Class>
    


    <!-- http://purl.obolibrary.org/obo/FOODON_00002739 -->

    <owl:Class rdf:about="http://purl.obolibrary.org/obo/FOODON_00002739"/>
    


    <!-- http://purl.obolibrary.org/obo/FOODON_00002740 -->

    <owl:Class rdf:about="http://purl.obolibrary.org/obo/FOODON_00002740">
        <rdfs:subClassOf rdf:resource="http://purl.obolibrary.org/obo/FOODON_00002451"/>
        <rdfs:subClassOf>
            <owl:Restriction>
                <owl:onProperty rdf:resource="http://purl.obolibrary.org/obo/RO_0002234"/>
                <owl:someValuesFrom rdf:resource="http://purl.obolibrary.org/obo/FOODON_00002739"/>
            </owl:Restriction>
        </rdfs:subClassOf>
        <obo:IAO_0000115 xml:lang="en">A process that applies packaging material to a food product for preservation, shipping and/or presentation purposes.</obo:IAO_0000115>
        <obo:IAO_0000117 rdf:datatype="http://www.w3.org/2001/XMLSchema#string">Damion Dooley</obo:IAO_0000117>
        <rdfs:label xml:lang="en">food packaging process</rdfs:label>
    </owl:Class>
    


    <!-- http://purl.obolibrary.org/obo/FOODON_00002814 -->

    <owl:Class rdf:about="http://purl.obolibrary.org/obo/FOODON_00002814">
        <rdfs:subClassOf rdf:resource="http://purl.obolibrary.org/obo/FOODON_03460111"/>
        <obo:IAO_0000115 xml:lang="en">Ikejime is a method of slaughtering fish to maintain the quality of its meat. The technique originated in Japan, but is now in widespread use. It involves the insertion of a spike quickly and directly into the hindbrain, usually located slightly behind and above the eye, thereby causing immediate brain death.</obo:IAO_0000115>
        <obo:IAO_0000117 rdf:datatype="http://www.w3.org/2001/XMLSchema#string">Damion Dooley</obo:IAO_0000117>
        <obo:IAO_0000119 rdf:datatype="http://www.w3.org/2001/XMLSchema#string">https://en.wikipedia.org/wiki/Ikejime</obo:IAO_0000119>
        <oboInOwl:hasExactSynonym xml:lang="en">Ikijime|活き締め|活け締め</oboInOwl:hasExactSynonym>
        <rdfs:comment xml:lang="en">When spiked correctly, the fish fins flare and the fish relaxes, immediately ceasing all motion. Destroying the brain and the spinal cord of the fish will prevent reflex action from happening; such muscle movements would otherwise consume adenosine triphosphate (ATP) in the muscle, and as a result produce lactic acid and ammonia, making the fish sour, soggy and less tasteful. Furthermore, the blood contained in the fish flesh retracts to the gut cavity, which produces a better coloured and flavoured fillet, and prolongs shelf life. [Wikipedia]</rdfs:comment>
        <rdfs:label xml:lang="en">ikajime</rdfs:label>
    </owl:Class>
    


    <!-- http://purl.obolibrary.org/obo/FOODON_00003203 -->

    <owl:Class rdf:about="http://purl.obolibrary.org/obo/FOODON_00003203">
        <rdfs:subClassOf rdf:resource="http://purl.obolibrary.org/obo/FOODON_00002451"/>
        <rdfs:subClassOf>
            <owl:Restriction>
                <owl:onProperty rdf:resource="http://purl.obolibrary.org/obo/RO_0002233"/>
                <owl:someValuesFrom rdf:resource="http://purl.obolibrary.org/obo/FOODON_00003402"/>
            </owl:Restriction>
        </rdfs:subClassOf>
        <rdfs:subClassOf>
            <owl:Restriction>
                <owl:onProperty rdf:resource="http://purl.obolibrary.org/obo/RO_0002234"/>
                <owl:someValuesFrom rdf:resource="http://purl.obolibrary.org/obo/FOODON_00003374"/>
            </owl:Restriction>
        </rdfs:subClassOf>
        <obo:IAO_0000115 xml:lang="en">A process which takes in some food material from an individual or community of plant or animal organisms in a given context and time, and outputs a precursor or consumable food product. This may include a part of an organism or the whole, and may involve killing the organism.</obo:IAO_0000115>
        <rdfs:comment xml:lang="en">This includes harvesting from plants, hunting a deer, or milking process of a cow.  The food is derived from part or whole of a single organism species (with perhaps a few exceptions, such as lichen).</rdfs:comment>
        <rdfs:label xml:lang="en">food harvesting</rdfs:label>
    </owl:Class>
    


    <!-- http://purl.obolibrary.org/obo/FOODON_00003215 -->

    <owl:Class rdf:about="http://purl.obolibrary.org/obo/FOODON_00003215">
        <rdfs:subClassOf rdf:resource="http://purl.obolibrary.org/obo/FOODON_03460238"/>
        <obo:IAO_0000115 xml:lang="en">Winterization of oil is a process that uses a solvent and cold temperatures to separate lipids and other desired oil compounds from waxes. Winterization is a type of fractionation, the general process of separating the triglycerides found in fats and oils, using the difference in their melting points, solubility, and volatility.</obo:IAO_0000115>
        <oboInOwl:hasExactSynonym xml:lang="en">fractionate crystallization</oboInOwl:hasExactSynonym>
        <rdfs:label xml:lang="en">winterization of oil</rdfs:label>
    </owl:Class>
    


    <!-- http://purl.obolibrary.org/obo/FOODON_00003307 -->

    <owl:Class rdf:about="http://purl.obolibrary.org/obo/FOODON_00003307">
        <rdfs:subClassOf rdf:resource="http://purl.obolibrary.org/obo/FOODON_03460238"/>
        <obo:IAO_0000115 xml:lang="en">A process which separates a culinary nut&apos;s shell from its meat, leaving the meat part more or less intact.</obo:IAO_0000115>
        <oboInOwl:hasExactSynonym xml:lang="en">shelling|shelling process</oboInOwl:hasExactSynonym>
        <rdfs:label xml:lang="en">shell removal process</rdfs:label>
    </owl:Class>
    


    <!-- http://purl.obolibrary.org/obo/FOODON_00003374 -->

    <owl:Class rdf:about="http://purl.obolibrary.org/obo/FOODON_00003374">
        <rdfs:label xml:lang="en">harvested food material</rdfs:label>
    </owl:Class>
    


    <!-- http://purl.obolibrary.org/obo/FOODON_00003402 -->

    <owl:Class rdf:about="http://purl.obolibrary.org/obo/FOODON_00003402">
        <rdfs:label xml:lang="en">pre-harvest food material</rdfs:label>
    </owl:Class>
    


    <!-- http://purl.obolibrary.org/obo/FOODON_03000001 -->

    <owl:Class rdf:about="http://purl.obolibrary.org/obo/FOODON_03000001">
        <rdfs:subClassOf rdf:resource="http://purl.obolibrary.org/obo/FOODON_03460130"/>
        <rdfs:subClassOf>
            <owl:Restriction>
                <owl:onProperty rdf:resource="http://purl.obolibrary.org/obo/RO_0002234"/>
                <owl:someValuesFrom rdf:resource="http://purl.obolibrary.org/obo/FOODON_00002655"/>
            </owl:Restriction>
        </rdfs:subClassOf>
        <obo:IAO_0000115 xml:lang="en">peeling&quot; is the process of removing the outer covering, layer or skin from a fruit, vegetable, or plant or animal (such as a shrimp).</obo:IAO_0000115>
        <obo:IAO_0000117 rdf:datatype="http://www.w3.org/2001/XMLSchema#string">Damion Dooley</obo:IAO_0000117>
        <rdfs:label xml:lang="en">food peeling process</rdfs:label>
    </owl:Class>
    


    <!-- http://purl.obolibrary.org/obo/FOODON_03307052 -->

    <owl:Class rdf:about="http://purl.obolibrary.org/obo/FOODON_03307052"/>
    


    <!-- http://purl.obolibrary.org/obo/FOODON_03411345 -->

    <owl:Class rdf:about="http://purl.obolibrary.org/obo/FOODON_03411345">
        <rdfs:label xml:lang="en">yeast</rdfs:label>
    </owl:Class>
    


    <!-- http://purl.obolibrary.org/obo/FOODON_03450002 -->

    <owl:Class rdf:about="http://purl.obolibrary.org/obo/FOODON_03450002">
        <rdfs:subClassOf rdf:resource="http://purl.obolibrary.org/obo/FOODON_00002451"/>
        <rdfs:subClassOf>
            <owl:Restriction>
                <owl:onProperty rdf:resource="http://purl.obolibrary.org/obo/RO_0002234"/>
                <owl:someValuesFrom rdf:resource="http://purl.obolibrary.org/obo/FOODON_00001181"/>
            </owl:Restriction>
        </rdfs:subClassOf>
        <oboInOwl:hasDbXref rdf:datatype="http://www.w3.org/2001/XMLSchema#string">http://www.langual.org/langual_thesaurus.asp?termid=G0002</oboInOwl:hasDbXref>
        <rdfs:label xml:lang="en">food cooking</rdfs:label>
    </owl:Class>
    


    <!-- http://purl.obolibrary.org/obo/FOODON_03450004 -->

    <owl:Class rdf:about="http://purl.obolibrary.org/obo/FOODON_03450004">
        <rdfs:subClassOf rdf:resource="http://purl.obolibrary.org/obo/FOODON_03450002"/>
        <obo:IAO_0000115 xml:lang="en">Cooked at moderate to high levels of heat in which no liquid is added and only small amounts of fat may be added to prevent sticking.</obo:IAO_0000115>
        <oboInOwl:hasDbXref rdf:datatype="http://www.w3.org/2001/XMLSchema#string">http://www.langual.org/langual_thesaurus.asp?termid=G0004</oboInOwl:hasDbXref>
        <oboInOwl:hasSynonym xml:lang="en">dry cooked</oboInOwl:hasSynonym>
        <rdfs:label xml:lang="en">cooking by dry heat</rdfs:label>
    </owl:Class>
    


    <!-- http://purl.obolibrary.org/obo/FOODON_03450005 -->

    <owl:Class rdf:about="http://purl.obolibrary.org/obo/FOODON_03450005">
        <rdfs:subClassOf rdf:resource="http://purl.obolibrary.org/obo/FOODON_03450004"/>
        <rdfs:subClassOf>
            <owl:Restriction>
                <owl:onProperty rdf:resource="http://purl.obolibrary.org/obo/RO_0002234"/>
                <owl:someValuesFrom rdf:resource="http://purl.obolibrary.org/obo/FOODON_00002456"/>
            </owl:Restriction>
        </rdfs:subClassOf>
        <obo:IAO_0000115 xml:lang="en">Cooked without moisture, covered or uncovered, in an oven.</obo:IAO_0000115>
        <obo:IAO_0000117 rdf:datatype="http://www.w3.org/2001/XMLSchema#string">Damion Dooley</obo:IAO_0000117>
        <oboInOwl:hasDbXref rdf:datatype="http://www.w3.org/2001/XMLSchema#string">http://www.langual.org/langual_thesaurus.asp?termid=G0005</oboInOwl:hasDbXref>
        <oboInOwl:hasSynonym xml:lang="en">roasting</oboInOwl:hasSynonym>
        <rdfs:label xml:lang="en">food baking</rdfs:label>
    </owl:Class>
    


    <!-- http://purl.obolibrary.org/obo/FOODON_03450006 -->

    <owl:Class rdf:about="http://purl.obolibrary.org/obo/FOODON_03450006">
        <rdfs:subClassOf rdf:resource="http://purl.obolibrary.org/obo/FOODON_03450004"/>
        <obo:IAO_0000115 xml:lang="en">Cooked without moisture under or over intense direct heat.</obo:IAO_0000115>
        <oboInOwl:hasDbXref rdf:datatype="http://www.w3.org/2001/XMLSchema#string">http://www.langual.org/langual_thesaurus.asp?termid=G0006</oboInOwl:hasDbXref>
        <oboInOwl:hasNarrowSynonym xml:lang="en">barbecuing|broiling|grilling</oboInOwl:hasNarrowSynonym>
        <rdfs:label xml:lang="en">broiling or grilling</rdfs:label>
    </owl:Class>
    


    <!-- http://purl.obolibrary.org/obo/FOODON_03450007 -->

    <owl:Class rdf:about="http://purl.obolibrary.org/obo/FOODON_03450007">
        <rdfs:subClassOf rdf:resource="http://purl.obolibrary.org/obo/FOODON_03450006"/>
        <obo:IAO_0000115 xml:lang="en">Cooked without moisture over direct heat from a charcoal fire.</obo:IAO_0000115>
        <oboInOwl:hasDbXref rdf:datatype="http://www.w3.org/2001/XMLSchema#string">http://www.langual.org/langual_thesaurus.asp?termid=G0007</oboInOwl:hasDbXref>
        <rdfs:label xml:lang="en">charcoal broiling</rdfs:label>
    </owl:Class>
    


    <!-- http://purl.obolibrary.org/obo/FOODON_03450008 -->

    <owl:Class rdf:about="http://purl.obolibrary.org/obo/FOODON_03450008">
        <rdfs:subClassOf rdf:resource="http://purl.obolibrary.org/obo/FOODON_03450004"/>
        <obo:IAO_0000115 xml:lang="en">Cooking on a flat surface at medium heat with only a sufficient amount of fat used to prevent sticking.</obo:IAO_0000115>
        <oboInOwl:hasDbXref rdf:datatype="http://www.w3.org/2001/XMLSchema#string">http://www.langual.org/langual_thesaurus.asp?termid=G0008</oboInOwl:hasDbXref>
        <rdfs:label xml:lang="en">griddle cooking</rdfs:label>
    </owl:Class>
    


    <!-- http://purl.obolibrary.org/obo/FOODON_03450009 -->

    <owl:Class rdf:about="http://purl.obolibrary.org/obo/FOODON_03450009">
        <rdfs:subClassOf rdf:resource="http://purl.obolibrary.org/obo/FOODON_03450004"/>
        <obo:IAO_0000115 xml:lang="en">Cooking by agitating the food over a dry, high heat source, resulting in exploding.</obo:IAO_0000115>
        <oboInOwl:hasDbXref rdf:datatype="http://www.w3.org/2001/XMLSchema#string">http://www.langual.org/langual_thesaurus.asp?termid=G0009</oboInOwl:hasDbXref>
        <rdfs:label xml:lang="en">cooked by popping</rdfs:label>
    </owl:Class>
    


    <!-- http://purl.obolibrary.org/obo/FOODON_03450010 -->

    <owl:Class rdf:about="http://purl.obolibrary.org/obo/FOODON_03450010">
        <rdfs:subClassOf rdf:resource="http://purl.obolibrary.org/obo/FOODON_03450004"/>
        <rdfs:subClassOf>
            <owl:Restriction>
                <owl:onProperty rdf:resource="http://purl.obolibrary.org/obo/RO_0002234"/>
                <owl:someValuesFrom rdf:resource="http://purl.obolibrary.org/obo/FOODON_00002659"/>
            </owl:Restriction>
        </rdfs:subClassOf>
        <obo:IAO_0000115 xml:lang="en">Cooking with direct heat until the surface of the food is browned, usually associated with bread or sandwiches.</obo:IAO_0000115>
        <oboInOwl:hasDbXref rdf:datatype="http://www.w3.org/2001/XMLSchema#string">http://www.langual.org/langual_thesaurus.asp?termid=G0010</oboInOwl:hasDbXref>
        <rdfs:label xml:lang="en">food toasting</rdfs:label>
    </owl:Class>
    


    <!-- http://purl.obolibrary.org/obo/FOODON_03450011 -->

    <owl:Class rdf:about="http://purl.obolibrary.org/obo/FOODON_03450011">
        <rdfs:subClassOf rdf:resource="http://purl.obolibrary.org/obo/FOODON_03450002"/>
        <obo:IAO_0000115 xml:lang="en">Cooking in a microwave oven.</obo:IAO_0000115>
        <oboInOwl:hasDbXref rdf:datatype="http://www.w3.org/2001/XMLSchema#string">http://www.langual.org/langual_thesaurus.asp?termid=G0011</oboInOwl:hasDbXref>
        <rdfs:label xml:lang="en">cooking by microwave</rdfs:label>
    </owl:Class>
    


    <!-- http://purl.obolibrary.org/obo/FOODON_03450012 -->

    <owl:Class rdf:about="http://purl.obolibrary.org/obo/FOODON_03450012">
        <rdfs:subClassOf rdf:resource="http://purl.obolibrary.org/obo/FOODON_03450002"/>
        <obo:IAO_0000115 xml:lang="en">Cooking in varying amounts of water, water-based liquid or steam.</obo:IAO_0000115>
        <oboInOwl:hasDbXref rdf:datatype="http://www.w3.org/2001/XMLSchema#string">http://www.langual.org/langual_thesaurus.asp?termid=G0012</oboInOwl:hasDbXref>
        <rdfs:comment xml:lang="en">LanguaL curation note: If the food absorbs a significant amount of water, also used *REHYDRATED* or *WATER ADDED*.</rdfs:comment>
        <rdfs:label xml:lang="en">cooking by moist heat</rdfs:label>
    </owl:Class>
    


    <!-- http://purl.obolibrary.org/obo/FOODON_03450013 -->

    <owl:Class rdf:about="http://purl.obolibrary.org/obo/FOODON_03450013">
        <rdfs:subClassOf rdf:resource="http://purl.obolibrary.org/obo/FOODON_03450012"/>
        <oboInOwl:hasDbXref rdf:datatype="http://www.w3.org/2001/XMLSchema#string">http://www.langual.org/langual_thesaurus.asp?termid=G0013</oboInOwl:hasDbXref>
        <rdfs:label xml:lang="en">cooking in water or water-based liquid</rdfs:label>
    </owl:Class>
    


    <!-- http://purl.obolibrary.org/obo/FOODON_03450014 -->

    <owl:Class rdf:about="http://purl.obolibrary.org/obo/FOODON_03450014">
        <rdfs:subClassOf rdf:resource="http://purl.obolibrary.org/obo/FOODON_03450013"/>
        <rdfs:subClassOf>
            <owl:Restriction>
                <owl:onProperty rdf:resource="http://purl.obolibrary.org/obo/RO_0002234"/>
                <owl:someValuesFrom rdf:resource="http://purl.obolibrary.org/obo/FOODON_00002688"/>
            </owl:Restriction>
        </rdfs:subClassOf>
        <obo:IAO_0000115 xml:lang="en">Cooked in boiling water at 100 degrees C (212 degrees F).</obo:IAO_0000115>
        <oboInOwl:hasDbXref rdf:datatype="http://www.w3.org/2001/XMLSchema#string">http://www.langual.org/langual_thesaurus.asp?termid=G0014</oboInOwl:hasDbXref>
        <rdfs:label xml:lang="en">boiling</rdfs:label>
    </owl:Class>
    


    <!-- http://purl.obolibrary.org/obo/FOODON_03450015 -->

    <owl:Class rdf:about="http://purl.obolibrary.org/obo/FOODON_03450015">
        <rdfs:subClassOf rdf:resource="http://purl.obolibrary.org/obo/FOODON_03450014"/>
        <obo:IAO_0000115 xml:lang="en">Cooked in boiling water at 212 degrees F.; water that is not absorbed into the food product is discarded after cooking.</obo:IAO_0000115>
        <oboInOwl:hasDbXref rdf:datatype="http://www.w3.org/2001/XMLSchema#string">http://www.langual.org/langual_thesaurus.asp?termid=G0015</oboInOwl:hasDbXref>
        <rdfs:label xml:lang="en">boiling and then draining</rdfs:label>
    </owl:Class>
    


    <!-- http://purl.obolibrary.org/obo/FOODON_03450016 -->

    <owl:Class rdf:about="http://purl.obolibrary.org/obo/FOODON_03450016">
        <rdfs:subClassOf rdf:resource="http://purl.obolibrary.org/obo/FOODON_03450015"/>
        <obo:IAO_0000115 xml:lang="en">Cooked in boiling water at 212 degrees F. Liquid to solid ratio is greater than 2:1.</obo:IAO_0000115>
        <oboInOwl:hasDbXref rdf:datatype="http://www.w3.org/2001/XMLSchema#string">http://www.langual.org/langual_thesaurus.asp?termid=G0016</oboInOwl:hasDbXref>
        <rdfs:label xml:lang="en">boiling in large amount of liquid</rdfs:label>
    </owl:Class>
    


    <!-- http://purl.obolibrary.org/obo/FOODON_03450017 -->

    <owl:Class rdf:about="http://purl.obolibrary.org/obo/FOODON_03450017">
        <rdfs:subClassOf rdf:resource="http://purl.obolibrary.org/obo/FOODON_03450015"/>
        <oboInOwl:hasDbXref rdf:datatype="http://www.w3.org/2001/XMLSchema#string">http://www.langual.org/langual_thesaurus.asp?termid=G0017</oboInOwl:hasDbXref>
        <rdfs:label xml:lang="en">boiling in small amount of liquid</rdfs:label>
    </owl:Class>
    


    <!-- http://purl.obolibrary.org/obo/FOODON_03450018 -->

    <owl:Class rdf:about="http://purl.obolibrary.org/obo/FOODON_03450018">
        <rdfs:subClassOf rdf:resource="http://purl.obolibrary.org/obo/FOODON_03450014"/>
        <obo:IAO_0000115 xml:lang="en">Cooked in boiling water at 212 degrees F. The water incorporates itself into the product being cooked or is not discarded when cooking is through.</obo:IAO_0000115>
        <oboInOwl:hasDbXref rdf:datatype="http://www.w3.org/2001/XMLSchema#string">http://www.langual.org/langual_thesaurus.asp?termid=G0018</oboInOwl:hasDbXref>
        <rdfs:label xml:lang="en">boiling without draining</rdfs:label>
    </owl:Class>
    


    <!-- http://purl.obolibrary.org/obo/FOODON_03450019 -->

    <owl:Class rdf:about="http://purl.obolibrary.org/obo/FOODON_03450019">
        <rdfs:subClassOf rdf:resource="http://purl.obolibrary.org/obo/FOODON_03450013"/>
        <obo:IAO_0000115 xml:lang="en">Browned initially in fat and then tightly covered and cooked over low heat in a small amount of water.</obo:IAO_0000115>
        <oboInOwl:hasDbXref rdf:datatype="http://www.w3.org/2001/XMLSchema#string">http://www.langual.org/langual_thesaurus.asp?termid=G0019</oboInOwl:hasDbXref>
        <rdfs:label xml:lang="en">cooking by braising</rdfs:label>
    </owl:Class>
    


    <!-- http://purl.obolibrary.org/obo/FOODON_03450020 -->

    <owl:Class rdf:about="http://purl.obolibrary.org/obo/FOODON_03450020">
        <rdfs:subClassOf rdf:resource="http://purl.obolibrary.org/obo/FOODON_03450013"/>
        <obo:IAO_0000115 xml:lang="en">Cooking in a moderate amount of liquid at just below the boiling point.</obo:IAO_0000115>
        <oboInOwl:hasDbXref rdf:datatype="http://www.w3.org/2001/XMLSchema#string">http://www.langual.org/langual_thesaurus.asp?termid=G0020</oboInOwl:hasDbXref>
        <oboInOwl:hasSynonym xml:lang="en">poaching|stewing</oboInOwl:hasSynonym>
        <rdfs:label xml:lang="en">cooking by simmering</rdfs:label>
    </owl:Class>
    


    <!-- http://purl.obolibrary.org/obo/FOODON_03450021 -->

    <owl:Class rdf:about="http://purl.obolibrary.org/obo/FOODON_03450021">
        <rdfs:subClassOf rdf:resource="http://purl.obolibrary.org/obo/FOODON_03450012"/>
        <rdfs:subClassOf>
            <owl:Restriction>
                <owl:onProperty rdf:resource="http://purl.obolibrary.org/obo/RO_0002234"/>
                <owl:someValuesFrom rdf:resource="http://purl.obolibrary.org/obo/FOODON_00002657"/>
            </owl:Restriction>
        </rdfs:subClassOf>
        <oboInOwl:hasDbXref rdf:datatype="http://www.w3.org/2001/XMLSchema#string">http://www.langual.org/langual_thesaurus.asp?termid=G0021</oboInOwl:hasDbXref>
        <rdfs:label xml:lang="en">cooking in steam</rdfs:label>
    </owl:Class>
    


    <!-- http://purl.obolibrary.org/obo/FOODON_03450022 -->

    <owl:Class rdf:about="http://purl.obolibrary.org/obo/FOODON_03450022">
        <rdfs:subClassOf rdf:resource="http://purl.obolibrary.org/obo/FOODON_03450021"/>
        <obo:IAO_0000115 xml:lang="en">Cooked in a pressure cooker.</obo:IAO_0000115>
        <oboInOwl:hasDbXref rdf:datatype="http://www.w3.org/2001/XMLSchema#string">http://www.langual.org/langual_thesaurus.asp?termid=G0022</oboInOwl:hasDbXref>
        <oboInOwl:hasSynonym xml:lang="en">pressure-cooked</oboInOwl:hasSynonym>
        <rdfs:label xml:lang="en">steaming with pressure</rdfs:label>
    </owl:Class>
    


    <!-- http://purl.obolibrary.org/obo/FOODON_03450023 -->

    <owl:Class rdf:about="http://purl.obolibrary.org/obo/FOODON_03450023">
        <rdfs:subClassOf rdf:resource="http://purl.obolibrary.org/obo/FOODON_03450021"/>
        <obo:IAO_0000115 xml:lang="en">Cooked suspended above boiling water.</obo:IAO_0000115>
        <oboInOwl:hasDbXref rdf:datatype="http://www.w3.org/2001/XMLSchema#string">http://www.langual.org/langual_thesaurus.asp?termid=G0023</oboInOwl:hasDbXref>
        <rdfs:label xml:lang="en">steaming without pressure</rdfs:label>
    </owl:Class>
    


    <!-- http://purl.obolibrary.org/obo/FOODON_03450024 -->

    <owl:Class rdf:about="http://purl.obolibrary.org/obo/FOODON_03450024">
        <rdfs:subClassOf rdf:resource="http://purl.obolibrary.org/obo/FOODON_03450002"/>
        <oboInOwl:hasDbXref rdf:datatype="http://www.w3.org/2001/XMLSchema#string">http://www.langual.org/langual_thesaurus.asp?termid=G0024</oboInOwl:hasDbXref>
        <oboInOwl:hasSynonym xml:lang="en">frying</oboInOwl:hasSynonym>
        <rdfs:label xml:lang="en">cooking with fat or oil</rdfs:label>
    </owl:Class>
    


    <!-- http://purl.obolibrary.org/obo/FOODON_03450025 -->

    <owl:Class rdf:about="http://purl.obolibrary.org/obo/FOODON_03450025">
        <rdfs:subClassOf rdf:resource="http://purl.obolibrary.org/obo/FOODON_03450024"/>
        <obo:IAO_0000115 xml:lang="en">Cooked by adding fat or oil to those foods that do not contain fat or oil that would render during the cooking process.</obo:IAO_0000115>
        <oboInOwl:hasDbXref rdf:datatype="http://www.w3.org/2001/XMLSchema#string">http://www.langual.org/langual_thesaurus.asp?termid=G0025</oboInOwl:hasDbXref>
        <oboInOwl:hasSynonym xml:lang="en">oil roasted</oboInOwl:hasSynonym>
        <rdfs:label xml:lang="en">cooking with added fat or oil</rdfs:label>
    </owl:Class>
    


    <!-- http://purl.obolibrary.org/obo/FOODON_03450026 -->

    <owl:Class rdf:about="http://purl.obolibrary.org/obo/FOODON_03450026">
        <rdfs:subClassOf rdf:resource="http://purl.obolibrary.org/obo/FOODON_03450025"/>
        <obo:IAO_0000115 xml:lang="en">Cooked with sufficient fat or oil to coat and moisten the food being prepared, but not cooked in enough fat or oil to immerse the food.</obo:IAO_0000115>
        <oboInOwl:hasDbXref rdf:datatype="http://www.w3.org/2001/XMLSchema#string">http://www.langual.org/langual_thesaurus.asp?termid=G0026</oboInOwl:hasDbXref>
        <rdfs:comment xml:lang="en">Use *griddle cooking* when only enough fat or oil is used to prevent sticking.</rdfs:comment>
        <rdfs:label xml:lang="en">cooking in small amount of fat or oil</rdfs:label>
        <rdfs:seeAlso rdf:datatype="http://www.w3.org/2001/XMLSchema#string">http://purl.obolibrary.org/obo/FOODON_03450008</rdfs:seeAlso>
    </owl:Class>
    


    <!-- http://purl.obolibrary.org/obo/FOODON_03450027 -->

    <owl:Class rdf:about="http://purl.obolibrary.org/obo/FOODON_03450027">
        <rdfs:subClassOf rdf:resource="http://purl.obolibrary.org/obo/FOODON_03450026"/>
        <obo:IAO_0000115 xml:lang="en">Cooking in a very small amount of very hot fat, turning and browning the food on all sides.</obo:IAO_0000115>
        <oboInOwl:hasDbXref rdf:datatype="http://www.w3.org/2001/XMLSchema#string">http://www.langual.org/langual_thesaurus.asp?termid=G0027</oboInOwl:hasDbXref>
        <oboInOwl:hasExactSynonym xml:lang="en">sauteing</oboInOwl:hasExactSynonym>
        <rdfs:label xml:lang="en">sautéing</rdfs:label>
    </owl:Class>
    


    <!-- http://purl.obolibrary.org/obo/FOODON_03450028 -->

    <owl:Class rdf:about="http://purl.obolibrary.org/obo/FOODON_03450028">
        <rdfs:subClassOf rdf:resource="http://purl.obolibrary.org/obo/FOODON_03450026"/>
        <obo:IAO_0000115 xml:lang="en">Cooked by frying foods quickly over high heat, stirring constantly. Only enough cooking oil is used to coat the bottom of the pan.</obo:IAO_0000115>
        <oboInOwl:hasDbXref rdf:datatype="http://www.w3.org/2001/XMLSchema#string">http://www.langual.org/langual_thesaurus.asp?termid=G0028</oboInOwl:hasDbXref>
        <rdfs:label xml:lang="en">stir-frying</rdfs:label>
    </owl:Class>
    


    <!-- http://purl.obolibrary.org/obo/FOODON_03450029 -->

    <owl:Class rdf:about="http://purl.obolibrary.org/obo/FOODON_03450029">
        <rdfs:subClassOf rdf:resource="http://purl.obolibrary.org/obo/FOODON_03450025"/>
        <rdfs:subClassOf>
            <owl:Restriction>
                <owl:onProperty rdf:resource="http://purl.obolibrary.org/obo/RO_0002234"/>
                <owl:someValuesFrom rdf:resource="http://purl.obolibrary.org/obo/FOODON_03307052"/>
            </owl:Restriction>
        </rdfs:subClassOf>
        <obo:IAO_0000115 xml:lang="en">Cooked in hot fat or oil deep enough to immerse the food entirely.</obo:IAO_0000115>
        <oboInOwl:hasDbXref rdf:datatype="http://www.w3.org/2001/XMLSchema#string">http://www.langual.org/langual_thesaurus.asp?termid=G0029</oboInOwl:hasDbXref>
        <oboInOwl:hasExactSynonym xml:lang="en">deep-frying</oboInOwl:hasExactSynonym>
        <rdfs:label xml:lang="en">deep-frying process</rdfs:label>
    </owl:Class>
    


    <!-- http://purl.obolibrary.org/obo/FOODON_03450030 -->

    <owl:Class rdf:about="http://purl.obolibrary.org/obo/FOODON_03450030">
        <rdfs:subClassOf rdf:resource="http://purl.obolibrary.org/obo/FOODON_03450024"/>
        <obo:IAO_0000115 xml:lang="en">Cooked in fat or oil rendered from the food being prepared.</obo:IAO_0000115>
        <oboInOwl:hasDbXref rdf:datatype="http://www.w3.org/2001/XMLSchema#string">http://www.langual.org/langual_thesaurus.asp?termid=G0030</oboInOwl:hasDbXref>
        <rdfs:label xml:lang="en">cooking with inherent fat or oil</rdfs:label>
    </owl:Class>
    


    <!-- http://purl.obolibrary.org/obo/FOODON_03450031 -->

    <owl:Class rdf:about="http://purl.obolibrary.org/obo/FOODON_03450031">
        <rdfs:subClassOf rdf:resource="http://purl.obolibrary.org/obo/FOODON_03450032"/>
        <oboInOwl:hasDbXref rdf:datatype="http://www.w3.org/2001/XMLSchema#string">http://www.langual.org/langual_thesaurus.asp?termid=G0031</oboInOwl:hasDbXref>
        <rdfs:comment xml:lang="en">LanguaL curation note: Used when the food is cooked in a closed container such as a pouch immersed in hot water or steam.</rdfs:comment>
        <rdfs:label xml:lang="en">cooking in container immersed in water or steam</rdfs:label>
    </owl:Class>
    


    <!-- http://purl.obolibrary.org/obo/FOODON_03450032 -->

    <owl:Class rdf:about="http://purl.obolibrary.org/obo/FOODON_03450032">
        <rdfs:subClassOf rdf:resource="http://purl.obolibrary.org/obo/FOODON_03450002"/>
        <obo:IAO_0000115 xml:lang="en">The method by which heat is transferred to the outside of the cooking container. The most frequently used method of placing the container on an open flame, a hot metal surface or into an oven are not indexed here.</obo:IAO_0000115>
        <oboInOwl:hasDbXref rdf:datatype="http://www.w3.org/2001/XMLSchema#string">http://www.langual.org/langual_thesaurus.asp?termid=G0032</oboInOwl:hasDbXref>
        <rdfs:label xml:lang="en">cooking using heating container</rdfs:label>
    </owl:Class>
    


    <!-- http://purl.obolibrary.org/obo/FOODON_03450033 -->

    <owl:Class rdf:about="http://purl.obolibrary.org/obo/FOODON_03450033">
        <rdfs:subClassOf rdf:resource="http://purl.obolibrary.org/obo/FOODON_03450032"/>
        <obo:IAO_0000115 xml:lang="en">Cooked in a container that is placed in another container filled with boiling water.</obo:IAO_0000115>
        <oboInOwl:hasDbXref rdf:datatype="http://www.w3.org/2001/XMLSchema#string">http://www.langual.org/langual_thesaurus.asp?termid=G0033</oboInOwl:hasDbXref>
        <oboInOwl:hasSynonym xml:lang="en">cooked over boiling water|double boiler cooked</oboInOwl:hasSynonym>
        <rdfs:label xml:lang="en">cooking in double boiler</rdfs:label>
        <rdfs:seeAlso rdf:datatype="http://www.w3.org/2001/XMLSchema#string">http://purl.obolibrary.org/obo/FOODON_03450034</rdfs:seeAlso>
    </owl:Class>
    


    <!-- http://purl.obolibrary.org/obo/FOODON_03450034 -->

    <owl:Class rdf:about="http://purl.obolibrary.org/obo/FOODON_03450034">
        <rdfs:subClassOf rdf:resource="http://purl.obolibrary.org/obo/FOODON_03450032"/>
        <obo:IAO_0000115 xml:lang="en">Cooking in a container that is placed in another container filled with water kept near the boiling point.</obo:IAO_0000115>
        <oboInOwl:hasDbXref rdf:datatype="http://www.w3.org/2001/XMLSchema#string">http://www.langual.org/langual_thesaurus.asp?termid=G0034</oboInOwl:hasDbXref>
        <oboInOwl:hasSynonym xml:lang="en">bain-marie cooked</oboInOwl:hasSynonym>
        <rdfs:label xml:lang="en">cooking in water bath</rdfs:label>
        <rdfs:seeAlso rdf:datatype="http://www.w3.org/2001/XMLSchema#string">http://purl.obolibrary.org/obo/FOODON_03450033</rdfs:seeAlso>
    </owl:Class>
    


    <!-- http://purl.obolibrary.org/obo/FOODON_03450035 -->

    <owl:Class rdf:about="http://purl.obolibrary.org/obo/FOODON_03450035">
        <rdfs:subClassOf rdf:resource="http://purl.obolibrary.org/obo/FOODON_03450025"/>
        <obo:IAO_0000115 xml:lang="en">A chinese cooking technique similar to sauteing in which thick slices or chunks of floured or battered ingredients are slow seared over moderate to low heat.</obo:IAO_0000115>
        <obo:IAO_0000119 rdf:datatype="http://www.w3.org/2001/XMLSchema#string">Kuo, The key to chinese cooking, Knopf, 1977, p.87</obo:IAO_0000119>
        <oboInOwl:hasDbXref rdf:datatype="http://www.w3.org/2001/XMLSchema#string">http://www.langual.org/langual_thesaurus.asp?termid=G0035</oboInOwl:hasDbXref>
        <oboInOwl:hasExactSynonym xml:lang="en">shallow frying</oboInOwl:hasExactSynonym>
        <rdfs:label xml:lang="en">shallow frying process</rdfs:label>
    </owl:Class>
    


    <!-- http://purl.obolibrary.org/obo/FOODON_03450036 -->

    <owl:Class rdf:about="http://purl.obolibrary.org/obo/FOODON_03450036">
        <rdfs:subClassOf rdf:resource="http://purl.obolibrary.org/obo/FOODON_03450013"/>
        <obo:IAO_0000115 xml:lang="en">Extracting flavor and other components from food sources by immersion in water, usually at near-boiling temperature.</obo:IAO_0000115>
        <oboInOwl:hasDbXref rdf:datatype="http://www.w3.org/2001/XMLSchema#string">http://www.langual.org/langual_thesaurus.asp?termid=G0036</oboInOwl:hasDbXref>
        <rdfs:label xml:lang="en">steeping</rdfs:label>
    </owl:Class>
    


    <!-- http://purl.obolibrary.org/obo/FOODON_03450037 -->

    <owl:Class rdf:about="http://purl.obolibrary.org/obo/FOODON_03450037">
        <rdfs:subClassOf rdf:resource="http://purl.obolibrary.org/obo/FOODON_03450002"/>
        <obo:IAO_0000115 xml:lang="en">A process to bring an already fully cooked product to serving temperature.</obo:IAO_0000115>
        <oboInOwl:hasDbXref rdf:datatype="http://www.w3.org/2001/XMLSchema#string">http://www.langual.org/langual_thesaurus.asp?termid=G0037</oboInOwl:hasDbXref>
        <rdfs:comment xml:lang="en">LanguaL curation note: Do not use for a process that completes the cooking of a partially cooked food.</rdfs:comment>
        <rdfs:label xml:lang="en">food reheating</rdfs:label>
    </owl:Class>
    


    <!-- http://purl.obolibrary.org/obo/FOODON_03450038 -->

    <owl:Class rdf:about="http://purl.obolibrary.org/obo/FOODON_03450038">
        <rdfs:subClassOf rdf:resource="http://purl.obolibrary.org/obo/FOODON_03450037"/>
        <oboInOwl:hasDbXref rdf:datatype="http://www.w3.org/2001/XMLSchema#string">http://www.langual.org/langual_thesaurus.asp?termid=G0038</oboInOwl:hasDbXref>
        <rdfs:label xml:lang="en">food reheating by microwave</rdfs:label>
    </owl:Class>
    


    <!-- http://purl.obolibrary.org/obo/FOODON_03450039 -->

    <owl:Class rdf:about="http://purl.obolibrary.org/obo/FOODON_03450039">
        <rdfs:subClassOf rdf:resource="http://purl.obolibrary.org/obo/FOODON_03450037"/>
        <oboInOwl:hasDbXref rdf:datatype="http://www.w3.org/2001/XMLSchema#string">http://www.langual.org/langual_thesaurus.asp?termid=G0039</oboInOwl:hasDbXref>
        <rdfs:label xml:lang="en">food reheating by dry heat</rdfs:label>
    </owl:Class>
    


    <!-- http://purl.obolibrary.org/obo/FOODON_03450040 -->

    <owl:Class rdf:about="http://purl.obolibrary.org/obo/FOODON_03450040">
        <rdfs:subClassOf rdf:resource="http://purl.obolibrary.org/obo/FOODON_03450037"/>
        <oboInOwl:hasDbXref rdf:datatype="http://www.w3.org/2001/XMLSchema#string">http://www.langual.org/langual_thesaurus.asp?termid=G0040</oboInOwl:hasDbXref>
        <rdfs:label xml:lang="en">food reheating by boil-in-bag</rdfs:label>
    </owl:Class>
    


    <!-- http://purl.obolibrary.org/obo/FOODON_03450041 -->

    <owl:Class rdf:about="http://purl.obolibrary.org/obo/FOODON_03450041">
        <rdfs:subClassOf rdf:resource="http://purl.obolibrary.org/obo/FOODON_03450037"/>
        <oboInOwl:hasDbXref rdf:datatype="http://www.w3.org/2001/XMLSchema#string">http://www.langual.org/langual_thesaurus.asp?termid=G0041</oboInOwl:hasDbXref>
        <rdfs:label xml:lang="en">food reheating in pan or cooking utensil</rdfs:label>
    </owl:Class>
    


    <!-- http://purl.obolibrary.org/obo/FOODON_03450043 -->

    <owl:Class rdf:about="http://purl.obolibrary.org/obo/FOODON_03450043">
        <rdfs:subClassOf rdf:resource="http://purl.obolibrary.org/obo/FOODON_03450014"/>
        <obo:IAO_0000115 xml:lang="en">A Chinese cooking technique to prepare delicate food such as bird nests, shark fins, etc. The food is covered with water and put in a covered ceramic jar and the jar is then steamed for several hours.</obo:IAO_0000115>
        <obo:IAO_0000119 rdf:datatype="http://www.w3.org/2001/XMLSchema#string">https://en.wikipedia.org/wiki/Double_steaming</obo:IAO_0000119>
        <oboInOwl:hasDbXref rdf:datatype="http://www.w3.org/2001/XMLSchema#string">http://www.langual.org/langual_thesaurus.asp?termid=G0043</oboInOwl:hasDbXref>
        <oboInOwl:hasSynonym xml:lang="en">double boiling</oboInOwl:hasSynonym>
        <rdfs:comment xml:lang="en">This technique ensures there is no loss of liquid or moisture (its essences) from the food being cooked, hence it is often used with expensive ingredients like Chinese herbal medicines. [Wikipedia]</rdfs:comment>
        <rdfs:label xml:lang="en">double steaming</rdfs:label>
    </owl:Class>
    


    <!-- http://purl.obolibrary.org/obo/FOODON_03450044 -->

    <owl:Class rdf:about="http://purl.obolibrary.org/obo/FOODON_03450044">
        <rdfs:subClassOf rdf:resource="http://purl.obolibrary.org/obo/FOODON_03450006"/>
        <obo:IAO_0000115 xml:lang="en">Rotisserie is a style of roasting where meat is skewered on a spit and revolves over a flame or other heat source.</obo:IAO_0000115>
        <oboInOwl:hasDbXref rdf:datatype="http://www.w3.org/2001/XMLSchema#string">http://www.langual.org/langual_thesaurus.asp?termid=G0044</oboInOwl:hasDbXref>
        <rdfs:comment xml:lang="en">The rotation cooks the meat evenly in its own juices and allows easy access for continuous basting if desired. [Wikipedia]</rdfs:comment>
        <rdfs:label xml:lang="en">rotisserie roasting</rdfs:label>
    </owl:Class>
    


    <!-- http://purl.obolibrary.org/obo/FOODON_03450045 -->

    <owl:Class rdf:about="http://purl.obolibrary.org/obo/FOODON_03450045">
        <rdfs:subClassOf rdf:resource="http://purl.obolibrary.org/obo/FOODON_03450006"/>
        <obo:IAO_0000115 xml:lang="en">Searing (or pan searing) is a technique used in grilling, roasting, braising, sautéing, etc. that cooks the surface of the food (usually meat, poultry or fish) at high temperature so that a brownish crust forms by Maillard reaction and denaturation of proteins.</obo:IAO_0000115>
        <oboInOwl:hasDbXref rdf:datatype="http://www.w3.org/2001/XMLSchema#string">http://www.langual.org/langual_thesaurus.asp?termid=G0045</oboInOwl:hasDbXref>
        <rdfs:comment xml:lang="en">A similar technique, browning, is typically used to sear or brown all sides of a particular piece of meat, fish, poultry, etc. before finishing it in the oven. To obtain the desired brown crust, the meat surface must exceed 300 °F (150 °C), so searing requires the meat surface be free of water, which boils at around 212 °F (100 °C).</rdfs:comment>
        <rdfs:label xml:lang="en">searing</rdfs:label>
    </owl:Class>
    


    <!-- http://purl.obolibrary.org/obo/FOODON_03450046 -->

    <owl:Class rdf:about="http://purl.obolibrary.org/obo/FOODON_03450046">
        <rdfs:subClassOf rdf:resource="http://purl.obolibrary.org/obo/FOODON_03450005"/>
        <oboInOwl:hasDbXref rdf:datatype="http://www.w3.org/2001/XMLSchema#string">http://www.langual.org/langual_thesaurus.asp?termid=G0046</oboInOwl:hasDbXref>
        <rdfs:comment xml:lang="en">LanguaL curation note: Use when a pie crust or other pastry is baked without the filling.</rdfs:comment>
        <rdfs:label xml:lang="en">blind baking</rdfs:label>
    </owl:Class>
    


    <!-- http://purl.obolibrary.org/obo/FOODON_03450047 -->

    <owl:Class rdf:about="http://purl.obolibrary.org/obo/FOODON_03450047">
        <rdfs:subClassOf rdf:resource="http://purl.obolibrary.org/obo/FOODON_03450025"/>
        <oboInOwl:hasDbXref rdf:datatype="http://www.w3.org/2001/XMLSchema#string">http://www.langual.org/langual_thesaurus.asp?termid=G0047</oboInOwl:hasDbXref>
        <oboInOwl:hasExactSynonym xml:lang="en">pressure frying</oboInOwl:hasExactSynonym>
        <rdfs:comment xml:lang="en">LanguaL curation note: Use when e.g. meat and cooking oil are brought to high temperatures while pressure is held high enough that the water within is prevented from boiling off.</rdfs:comment>
        <rdfs:label xml:lang="en">pressure frying process</rdfs:label>
    </owl:Class>
    


    <!-- http://purl.obolibrary.org/obo/FOODON_03460101 -->

    <owl:Class rdf:about="http://purl.obolibrary.org/obo/FOODON_03460101">
        <rdfs:subClassOf rdf:resource="http://purl.obolibrary.org/obo/FOODON_03460256"/>
        <oboInOwl:hasDbXref rdf:datatype="http://www.w3.org/2001/XMLSchema#string">http://www.langual.org/langual_thesaurus.asp?termid=H0101</oboInOwl:hasDbXref>
        <oboInOwl:hasSynonym xml:lang="en">cultured|pickled by fermentation</oboInOwl:hasSynonym>
        <rdfs:label xml:lang="en">lactic acid fermentation</rdfs:label>
    </owl:Class>
    


    <!-- http://purl.obolibrary.org/obo/FOODON_03460102 -->

    <owl:Class rdf:about="http://purl.obolibrary.org/obo/FOODON_03460102">
        <rdfs:subClassOf rdf:resource="http://purl.obolibrary.org/obo/FOODON_03460230"/>
        <oboInOwl:hasDbXref rdf:datatype="http://www.w3.org/2001/XMLSchema#string">http://www.langual.org/langual_thesaurus.asp?termid=H0102</oboInOwl:hasDbXref>
        <rdfs:label xml:lang="en">proteolytic fermentation</rdfs:label>
    </owl:Class>
    


    <!-- http://purl.obolibrary.org/obo/FOODON_03460103 -->

    <owl:Class rdf:about="http://purl.obolibrary.org/obo/FOODON_03460103">
        <rdfs:subClassOf rdf:resource="http://purl.obolibrary.org/obo/FOODON_03460111"/>
        <oboInOwl:hasDbXref rdf:datatype="http://www.w3.org/2001/XMLSchema#string">http://www.langual.org/langual_thesaurus.asp?termid=H0103</oboInOwl:hasDbXref>
        <rdfs:comment xml:lang="en">LanguaL curation note: Use the appropriate narrower term for a food product that was prepared from a natural food product by removing an endogeneous component and adding a component of the same class. Index the specific component added under *INGREDIENT ADDED*, regardless of its level.</rdfs:comment>
        <rdfs:label xml:lang="en">component substitution process</rdfs:label>
    </owl:Class>
    


    <!-- http://purl.obolibrary.org/obo/FOODON_03460106 -->

    <owl:Class rdf:about="http://purl.obolibrary.org/obo/FOODON_03460106">
        <rdfs:subClassOf rdf:resource="http://purl.obolibrary.org/obo/FOODON_03460150"/>
        <oboInOwl:hasDbXref rdf:datatype="http://www.w3.org/2001/XMLSchema#string">http://www.langual.org/langual_thesaurus.asp?termid=H0106</oboInOwl:hasDbXref>
        <rdfs:comment xml:lang="en">LanguaL curation note: Used when a color is added that is exempt from certification and considered safe for use.</rdfs:comment>
        <rdfs:label xml:lang="en">food noncertified color addition process</rdfs:label>
    </owl:Class>
    


    <!-- http://purl.obolibrary.org/obo/FOODON_03460107 -->

    <owl:Class rdf:about="http://purl.obolibrary.org/obo/FOODON_03460107">
        <rdfs:subClassOf rdf:resource="http://purl.obolibrary.org/obo/FOODON_03460128"/>
        <oboInOwl:hasDbXref rdf:datatype="http://www.w3.org/2001/XMLSchema#string">http://www.langual.org/langual_thesaurus.asp?termid=H0107</oboInOwl:hasDbXref>
        <rdfs:label xml:lang="en">lactic acid-other agent fermentation</rdfs:label>
    </owl:Class>
    


    <!-- http://purl.obolibrary.org/obo/FOODON_03460109 -->

    <owl:Class rdf:about="http://purl.obolibrary.org/obo/FOODON_03460109">
        <rdfs:subClassOf rdf:resource="http://purl.obolibrary.org/obo/FOODON_03460175"/>
        <oboInOwl:hasDbXref rdf:datatype="http://www.w3.org/2001/XMLSchema#string">http://www.langual.org/langual_thesaurus.asp?termid=H0109</oboInOwl:hasDbXref>
        <rdfs:comment xml:lang="en">LanguaL curation note: Used when carbon dioxide has been added to a food product at any level. Damion Dooley&apos;s note: converted to a process</rdfs:comment>
        <rdfs:label xml:lang="en">artificial carbonation process</rdfs:label>
    </owl:Class>
    


    <!-- http://purl.obolibrary.org/obo/FOODON_03460111 -->

    <owl:Class rdf:about="http://purl.obolibrary.org/obo/FOODON_03460111">
        <rdfs:subClassOf rdf:resource="http://purl.obolibrary.org/obo/FOODON_00002451"/>
        <obo:IAO_0000115 xml:lang="en">Used to specifically characterize a food product based on the treatment or processes applied to the product or any indexed ingredient. The processes include adding, substituting or removing components or modifying the food or component, e.g., through fermentation.</obo:IAO_0000115>
        <oboInOwl:hasDbXref rdf:datatype="http://www.w3.org/2001/XMLSchema#string">http://www.langual.org/langual_thesaurus.asp?termid=H0111</oboInOwl:hasDbXref>
        <rdfs:comment xml:lang="en">LanguaL curation note: This term is for CLASSIFICATION ONLY; DO NOT USE term in indexing. Use a more precise narrower term.</rdfs:comment>
        <rdfs:label xml:lang="en">food treatment process</rdfs:label>
    </owl:Class>
    


    <!-- http://purl.obolibrary.org/obo/FOODON_03460112 -->

    <owl:Class rdf:about="http://purl.obolibrary.org/obo/FOODON_03460112">
        <rdfs:subClassOf rdf:resource="http://purl.obolibrary.org/obo/FOODON_03460138"/>
        <oboInOwl:hasDbXref rdf:datatype="http://www.w3.org/2001/XMLSchema#string">http://www.langual.org/langual_thesaurus.asp?termid=H0112</oboInOwl:hasDbXref>
        <oboInOwl:hasSynonym xml:lang="en">concentrated, 40 degrees brix or higher</oboInOwl:hasSynonym>
        <rdfs:label xml:lang="en">water removal to reconstitution ratio 3 plus 1 or higher</rdfs:label>
    </owl:Class>
    


    <!-- http://purl.obolibrary.org/obo/FOODON_03460113 -->

    <owl:Class rdf:about="http://purl.obolibrary.org/obo/FOODON_03460113">
        <rdfs:subClassOf rdf:resource="http://purl.obolibrary.org/obo/FOODON_03460138"/>
        <oboInOwl:hasDbXref rdf:datatype="http://www.w3.org/2001/XMLSchema#string">http://www.langual.org/langual_thesaurus.asp?termid=H0113</oboInOwl:hasDbXref>
        <oboInOwl:hasSynonym xml:lang="en">concentrated, 20-40 degrees brix</oboInOwl:hasSynonym>
        <rdfs:label xml:lang="en">water removal to reconstitution ratio 2 plus 1</rdfs:label>
    </owl:Class>
    


    <!-- http://purl.obolibrary.org/obo/FOODON_03460114 -->

    <owl:Class rdf:about="http://purl.obolibrary.org/obo/FOODON_03460114">
        <rdfs:subClassOf rdf:resource="http://purl.obolibrary.org/obo/FOODON_03460138"/>
        <oboInOwl:hasDbXref rdf:datatype="http://www.w3.org/2001/XMLSchema#string">http://www.langual.org/langual_thesaurus.asp?termid=H0114</oboInOwl:hasDbXref>
        <oboInOwl:hasSynonym xml:lang="en">condensed</oboInOwl:hasSynonym>
        <rdfs:label xml:lang="en">water removal to reconstitution ratio 1 plus 1</rdfs:label>
    </owl:Class>
    


    <!-- http://purl.obolibrary.org/obo/FOODON_03460119 -->

    <owl:Class rdf:about="http://purl.obolibrary.org/obo/FOODON_03460119">
        <rdfs:subClassOf rdf:resource="http://purl.obolibrary.org/obo/FOODON_03460141"/>
        <obo:IAO_0000115 xml:lang="en">A food modification process by microbial or enzymatic action which results in molecular changes in any food component.</obo:IAO_0000115>
        <oboInOwl:hasDbXref rdf:datatype="http://www.w3.org/2001/XMLSchema#string">http://www.langual.org/langual_thesaurus.asp?termid=H0119</oboInOwl:hasDbXref>
        <oboInOwl:hasSynonym xml:lang="en">fermented, unspecified</oboInOwl:hasSynonym>
        <rdfs:comment xml:lang="en">LanguaL curation note: If salt, sugar or other food additive is used to aid in the modification process, index it by the appropriate term under *INGREDIENT ADDED*.</rdfs:comment>
        <rdfs:label xml:lang="en">microbial/enzymatic modification process</rdfs:label>
    </owl:Class>
    


    <!-- http://purl.obolibrary.org/obo/FOODON_03460121 -->

    <owl:Class rdf:about="http://purl.obolibrary.org/obo/FOODON_03460121">
        <rdfs:subClassOf rdf:resource="http://purl.obolibrary.org/obo/FOODON_03460130"/>
        <obo:IAO_0000115 xml:lang="en">A physical/chemical modification process in which a food product or component is irradiated for any purpose.</obo:IAO_0000115>
        <oboInOwl:hasDbXref rdf:datatype="http://www.w3.org/2001/XMLSchema#string">http://www.langual.org/langual_thesaurus.asp?termid=H0121</oboInOwl:hasDbXref>
        <oboInOwl:hasSynonym xml:lang="en">picowaved</oboInOwl:hasSynonym>
        <rdfs:label xml:lang="en">food irradiation process</rdfs:label>
    </owl:Class>
    


    <!-- http://purl.obolibrary.org/obo/FOODON_03460123 -->

    <owl:Class rdf:about="http://purl.obolibrary.org/obo/FOODON_03460123">
        <rdfs:subClassOf rdf:resource="http://purl.obolibrary.org/obo/FOODON_03460256"/>
        <oboInOwl:hasDbXref rdf:datatype="http://www.w3.org/2001/XMLSchema#string">http://www.langual.org/langual_thesaurus.asp?termid=H0123</oboInOwl:hasDbXref>
        <rdfs:label xml:lang="en">alcohol-acetic acid fermentation</rdfs:label>
    </owl:Class>
    


    <!-- http://purl.obolibrary.org/obo/FOODON_03460127 -->

    <owl:Class rdf:about="http://purl.obolibrary.org/obo/FOODON_03460127">
        <rdfs:subClassOf rdf:resource="http://purl.obolibrary.org/obo/FOODON_03460230"/>
        <oboInOwl:hasDbXref rdf:datatype="http://www.w3.org/2001/XMLSchema#string">http://www.langual.org/langual_thesaurus.asp?termid=H0127</oboInOwl:hasDbXref>
        <rdfs:label xml:lang="en">lipolytic fermentation</rdfs:label>
    </owl:Class>
    


    <!-- http://purl.obolibrary.org/obo/FOODON_03460128 -->

    <owl:Class rdf:about="http://purl.obolibrary.org/obo/FOODON_03460128">
        <rdfs:subClassOf rdf:resource="http://purl.obolibrary.org/obo/FOODON_00001304"/>
        <obo:IAO_0000115 xml:lang="en">A food fermentation process in which significant amounts of two or more components (i.e. carbohydrate and protein, carbohydrate and fat, protein and fat, or all three) are modified through microbial processes. Enzymatic or other biological processes may also be involved.</obo:IAO_0000115>
        <oboInOwl:hasDbXref rdf:datatype="http://www.w3.org/2001/XMLSchema#string">http://www.langual.org/langual_thesaurus.asp?termid=H0128</oboInOwl:hasDbXref>
        <oboInOwl:hasSynonym xml:lang="en">ripened (cured)</oboInOwl:hasSynonym>
        <rdfs:label xml:lang="en">multi-component food fermentation</rdfs:label>
    </owl:Class>
    


    <!-- http://purl.obolibrary.org/obo/FOODON_03460130 -->

    <owl:Class rdf:about="http://purl.obolibrary.org/obo/FOODON_03460130">
        <rdfs:subClassOf rdf:resource="http://purl.obolibrary.org/obo/FOODON_03460141"/>
        <obo:IAO_0000115 xml:lang="en">A food modification process where physical or chemical changes are effected in any food ingredient through a physical or non-enzymatic chemical process.</obo:IAO_0000115>
        <oboInOwl:hasDbXref rdf:datatype="http://www.w3.org/2001/XMLSchema#string">http://www.langual.org/langual_thesaurus.asp?termid=H0130</oboInOwl:hasDbXref>
        <rdfs:label xml:lang="en">physical/chemical modification process</rdfs:label>
    </owl:Class>
    


    <!-- http://purl.obolibrary.org/obo/FOODON_03460133 -->

    <owl:Class rdf:about="http://purl.obolibrary.org/obo/FOODON_03460133">
        <rdfs:subClassOf rdf:resource="http://purl.obolibrary.org/obo/FOODON_03460150"/>
        <obo:IAO_0000115 xml:lang="en">A food color addition process in which color that must be certified by batch as safe to use is added at any level.</obo:IAO_0000115>
        <oboInOwl:hasDbXref rdf:datatype="http://www.w3.org/2001/XMLSchema#string">http://www.langual.org/langual_thesaurus.asp?termid=H0133</oboInOwl:hasDbXref>
        <rdfs:label xml:lang="en">food certified color addition process</rdfs:label>
    </owl:Class>
    


    <!-- http://purl.obolibrary.org/obo/FOODON_03460134 -->

    <owl:Class rdf:about="http://purl.obolibrary.org/obo/FOODON_03460134">
        <rdfs:subClassOf rdf:resource="http://purl.obolibrary.org/obo/FOODON_03460238"/>
        <oboInOwl:hasDbXref rdf:datatype="http://www.w3.org/2001/XMLSchema#string">http://www.langual.org/langual_thesaurus.asp?termid=H0134</oboInOwl:hasDbXref>
        <rdfs:label xml:lang="en">protein removal process</rdfs:label>
    </owl:Class>
    


    <!-- http://purl.obolibrary.org/obo/FOODON_03460135 -->

    <owl:Class rdf:about="http://purl.obolibrary.org/obo/FOODON_03460135">
        <rdfs:subClassOf rdf:resource="http://purl.obolibrary.org/obo/FOODON_03460238"/>
        <oboInOwl:hasDbXref rdf:datatype="http://www.w3.org/2001/XMLSchema#string">http://www.langual.org/langual_thesaurus.asp?termid=H0135</oboInOwl:hasDbXref>
        <oboInOwl:hasSynonym xml:lang="en">dealkaloidized|purine removed</oboInOwl:hasSynonym>
        <rdfs:label xml:lang="en">alkaloid or purine removal process</rdfs:label>
    </owl:Class>
    


    <!-- http://purl.obolibrary.org/obo/FOODON_03460137 -->

    <owl:Class rdf:about="http://purl.obolibrary.org/obo/FOODON_03460137">
        <rdfs:subClassOf rdf:resource="http://purl.obolibrary.org/obo/FOODON_03460238"/>
        <oboInOwl:hasDbXref rdf:datatype="http://www.w3.org/2001/XMLSchema#string">http://www.langual.org/langual_thesaurus.asp?termid=H0137</oboInOwl:hasDbXref>
        <oboInOwl:hasSynonym xml:lang="en">calcium removed|minerals removed</oboInOwl:hasSynonym>
        <rdfs:comment xml:lang="en">LanguaL curation note: Used when one or more naturally present minerals have been fully or partially removed.</rdfs:comment>
        <rdfs:label xml:lang="en">demineralizing process</rdfs:label>
    </owl:Class>
    


    <!-- http://purl.obolibrary.org/obo/FOODON_03460138 -->

    <owl:Class rdf:about="http://purl.obolibrary.org/obo/FOODON_03460138">
        <rdfs:subClassOf rdf:resource="http://purl.obolibrary.org/obo/FOODON_03460238"/>
        <oboInOwl:hasDbXref rdf:datatype="http://www.w3.org/2001/XMLSchema#string">http://www.langual.org/langual_thesaurus.asp?termid=H0138</oboInOwl:hasDbXref>
        <rdfs:comment xml:lang="en">LanguaL curation note: Used for a liquid or solid product from which a significant amount of water (25% or more of the original weight of the water) has been removed. If dehydration is the primary preservation method, also index *DEHYDRATED OR DRIED*. For soups that require the addition of water, use the appropriate narrower term regardless of whether water was removed or not. Do not use for products that have been rehydrated.</rdfs:comment>
        <rdfs:label xml:lang="en">water removal process</rdfs:label>
    </owl:Class>
    


    <!-- http://purl.obolibrary.org/obo/FOODON_03460140 -->

    <owl:Class rdf:about="http://purl.obolibrary.org/obo/FOODON_03460140">
        <rdfs:subClassOf rdf:resource="http://purl.obolibrary.org/obo/FOODON_03460135"/>
        <oboInOwl:hasDbXref rdf:datatype="http://www.w3.org/2001/XMLSchema#string">http://www.langual.org/langual_thesaurus.asp?termid=H0140</oboInOwl:hasDbXref>
        <rdfs:label xml:lang="en">decaffeination process</rdfs:label>
    </owl:Class>
    


    <!-- http://purl.obolibrary.org/obo/FOODON_03460141 -->

    <owl:Class rdf:about="http://purl.obolibrary.org/obo/FOODON_03460141">
        <rdfs:subClassOf rdf:resource="http://purl.obolibrary.org/obo/FOODON_03460111"/>
        <oboInOwl:hasDbXref rdf:datatype="http://www.w3.org/2001/XMLSchema#string">http://www.langual.org/langual_thesaurus.asp?termid=H0141</oboInOwl:hasDbXref>
        <rdfs:comment xml:lang="en">LanguaL curation note: Used when the food product underwent mechanical, chemical or enzymatic modification that has affected the texture, flavor or other characteristic of the product.</rdfs:comment>
        <rdfs:label xml:lang="en">food modification process</rdfs:label>
    </owl:Class>
    


    <!-- http://purl.obolibrary.org/obo/FOODON_03460148 -->

    <owl:Class rdf:about="http://purl.obolibrary.org/obo/FOODON_03460148">
        <rdfs:subClassOf rdf:resource="http://purl.obolibrary.org/obo/FOODON_03460225"/>
        <rdfs:subClassOf rdf:resource="http://purl.obolibrary.org/obo/FOODON_03460254"/>
        <oboInOwl:hasDbXref rdf:datatype="http://www.w3.org/2001/XMLSchema#string">http://www.langual.org/langual_thesaurus.asp?termid=H0148</oboInOwl:hasDbXref>
        <oboInOwl:hasSynonym xml:lang="en">diluted</oboInOwl:hasSynonym>
        <rdfs:comment xml:lang="en">LanguaL curation note: Used for a liquid or solid product to which water was added beyond its natural water level. If a single-strength standard for the product exists, use the appropriate narrower term under *WATER ADDED*.</rdfs:comment>
        <rdfs:label xml:lang="en">water addition process</rdfs:label>
    </owl:Class>
    


    <!-- http://purl.obolibrary.org/obo/FOODON_03460150 -->

    <owl:Class rdf:about="http://purl.obolibrary.org/obo/FOODON_03460150">
        <rdfs:subClassOf rdf:resource="http://purl.obolibrary.org/obo/FOODON_03460225"/>
        <oboInOwl:hasDbXref rdf:datatype="http://www.w3.org/2001/XMLSchema#string">http://www.langual.org/langual_thesaurus.asp?termid=H0150</oboInOwl:hasDbXref>
        <rdfs:comment xml:lang="en">LanguaL curation note: Used when a color substance is added to a food at any level.</rdfs:comment>
        <rdfs:label xml:lang="en">food color addition process</rdfs:label>
    </owl:Class>
    


    <!-- http://purl.obolibrary.org/obo/FOODON_03460160 -->

    <owl:Class rdf:about="http://purl.obolibrary.org/obo/FOODON_03460160">
        <rdfs:subClassOf rdf:resource="http://purl.obolibrary.org/obo/FOODON_03460225"/>
        <oboInOwl:hasDbXref rdf:datatype="http://www.w3.org/2001/XMLSchema#string">http://www.langual.org/langual_thesaurus.asp?termid=H0160</oboInOwl:hasDbXref>
        <oboInOwl:hasSynonym xml:lang="en">brandied</oboInOwl:hasSynonym>
        <rdfs:comment xml:lang="en">LanguaL curation note: Used when alcohol is added for flavor or taste, for example, brandied peaches or cold-pack cheese food with port wine.</rdfs:comment>
        <rdfs:label xml:lang="en">alcoholization process</rdfs:label>
    </owl:Class>
    


    <!-- http://purl.obolibrary.org/obo/FOODON_03460161 -->

    <owl:Class rdf:about="http://purl.obolibrary.org/obo/FOODON_03460161">
        <rdfs:subClassOf rdf:resource="http://purl.obolibrary.org/obo/FOODON_03460238"/>
        <oboInOwl:hasDbXref rdf:datatype="http://www.w3.org/2001/XMLSchema#string">http://www.langual.org/langual_thesaurus.asp?termid=H0161</oboInOwl:hasDbXref>
        <oboInOwl:hasSynonym xml:lang="en">cholesterol removed|defatted</oboInOwl:hasSynonym>
        <rdfs:comment xml:lang="en">LanguaL curation note: Used for products that contain less than 60% of the fat naturally present in the food source (more precisely, the part of the food source.) more specific fat levels, which vary from one product type to another, are specified in the extended scope notes for *FAT PARTIALLY REMOVED* and *FAT FULLY REMOVED* in the manual.</rdfs:comment>
        <rdfs:label xml:lang="en">fat removal process</rdfs:label>
    </owl:Class>
    


    <!-- http://purl.obolibrary.org/obo/FOODON_03460169 -->

    <owl:Class rdf:about="http://purl.obolibrary.org/obo/FOODON_03460169">
        <rdfs:subClassOf rdf:resource="http://purl.obolibrary.org/obo/FOODON_03460141"/>
        <oboInOwl:hasDbXref rdf:datatype="http://www.w3.org/2001/XMLSchema#string">http://www.langual.org/langual_thesaurus.asp?termid=H0169</oboInOwl:hasDbXref>
        <oboInOwl:hasSynonym xml:lang="en">agglomerated|converted (grain)</oboInOwl:hasSynonym>
        <rdfs:comment xml:lang="en">LanguaL curation note: Used for food products modified to reduce cooking time or to enhance dispersion characteristics of powdered or granulated products.</rdfs:comment>
        <rdfs:label xml:lang="en">food instantizing</rdfs:label>
    </owl:Class>
    


    <!-- http://purl.obolibrary.org/obo/FOODON_03460174 -->

    <owl:Class rdf:about="http://purl.obolibrary.org/obo/FOODON_03460174">
        <rdfs:subClassOf rdf:resource="http://purl.obolibrary.org/obo/FOODON_03460130"/>
        <obo:IAO_0000115 xml:lang="en">The saturating or hardening of a vegetable oil to which hydrogen has been chemically added to convert it to a fat.</obo:IAO_0000115>
        <oboInOwl:hasDbXref rdf:datatype="http://www.w3.org/2001/XMLSchema#string">http://www.langual.org/langual_thesaurus.asp?termid=H0174</oboInOwl:hasDbXref>
        <rdfs:label xml:lang="en">food hydrogenation process</rdfs:label>
    </owl:Class>
    


    <!-- http://purl.obolibrary.org/obo/FOODON_03460175 -->

    <owl:Class rdf:about="http://purl.obolibrary.org/obo/FOODON_03460175">
        <rdfs:subClassOf rdf:resource="http://purl.obolibrary.org/obo/FOODON_03460225"/>
        <oboInOwl:hasDbXref rdf:datatype="http://www.w3.org/2001/XMLSchema#string">http://www.langual.org/langual_thesaurus.asp?termid=H0175</oboInOwl:hasDbXref>
        <oboInOwl:hasSynonym xml:lang="en">carbon dioxide added</oboInOwl:hasSynonym>
        <rdfs:comment xml:lang="en">LanguaL curation note: Used when carbon dioxide is added or introduced by processing. Excludes naturally carbonated water, which is indexed under food source *MINERAL WATER*.  Damion Dooley&apos;s note: converted to a process</rdfs:comment>
        <rdfs:label xml:lang="en">carbonation process</rdfs:label>
    </owl:Class>
    


    <!-- http://purl.obolibrary.org/obo/FOODON_03460178 -->

    <owl:Class rdf:about="http://purl.obolibrary.org/obo/FOODON_03460178">
        <rdfs:subClassOf rdf:resource="http://purl.obolibrary.org/obo/FOODON_03460130"/>
        <oboInOwl:hasDbXref rdf:datatype="http://www.w3.org/2001/XMLSchema#string">http://www.langual.org/langual_thesaurus.asp?termid=H0178</oboInOwl:hasDbXref>
        <rdfs:comment xml:lang="en">LanguaL curation note: Used for products with which a substantial amount of air has been mixed through mechanical action. Do not use when air was introduced primarily through chemical action or through fermentation.</rdfs:comment>
        <rdfs:label xml:lang="en">food aeration process</rdfs:label>
    </owl:Class>
    


    <!-- http://purl.obolibrary.org/obo/FOODON_03460179 -->

    <owl:Class rdf:about="http://purl.obolibrary.org/obo/FOODON_03460179">
        <rdfs:subClassOf rdf:resource="http://purl.obolibrary.org/obo/FOODON_03460121"/>
        <oboInOwl:hasDbXref rdf:datatype="http://www.w3.org/2001/XMLSchema#string">http://www.langual.org/langual_thesaurus.asp?termid=H0179</oboInOwl:hasDbXref>
        <rdfs:label xml:lang="en">food ionizing irradiation process</rdfs:label>
    </owl:Class>
    


    <!-- http://purl.obolibrary.org/obo/FOODON_03460182 -->

    <owl:Class rdf:about="http://purl.obolibrary.org/obo/FOODON_03460182">
        <rdfs:subClassOf rdf:resource="http://purl.obolibrary.org/obo/FOODON_03460130"/>
        <oboInOwl:hasDbXref rdf:datatype="http://www.w3.org/2001/XMLSchema#string">http://www.langual.org/langual_thesaurus.asp?termid=H0182</oboInOwl:hasDbXref>
        <rdfs:comment xml:lang="en">LanguaL curation note: Used for whole fruit or pieces of fruit are permeated by sugar to result in a product with sugar solids over 70% (e.g., candied citrus peel or candied cherry). Not used for sugar-coated products or for such products as candied sweet potatoes or glazed carrots, which are merely sweetened by cooking in syrup.</rdfs:comment>
        <rdfs:label xml:lang="en">candying process</rdfs:label>
    </owl:Class>
    


    <!-- http://purl.obolibrary.org/obo/FOODON_03460190 -->

    <owl:Class rdf:about="http://purl.obolibrary.org/obo/FOODON_03460190">
        <rdfs:subClassOf rdf:resource="http://purl.obolibrary.org/obo/FOODON_03460119"/>
        <obo:IAO_0000115 xml:lang="en">Treated with acid that may be produced by fermentation or added and/or with salt brine, often in the presence of spices or herbs, producing changes in flavor and texture.</obo:IAO_0000115>
        <oboInOwl:hasDbXref rdf:datatype="http://www.w3.org/2001/XMLSchema#string">http://www.langual.org/langual_thesaurus.asp?termid=H0190</oboInOwl:hasDbXref>
        <rdfs:comment xml:lang="en">LanguaL curation note: Also index by other applicable terms from *MICROBIALLY/ ENZYMATICALLY MODIFIED*.</rdfs:comment>
        <rdfs:label xml:lang="en">pickling</rdfs:label>
    </owl:Class>
    


    <!-- http://purl.obolibrary.org/obo/FOODON_03460192 -->

    <owl:Class rdf:about="http://purl.obolibrary.org/obo/FOODON_03460192">
        <rdfs:subClassOf rdf:resource="http://purl.obolibrary.org/obo/FOODON_00002409"/>
        <obo:IAO_0000115 xml:lang="en">Modified through physical and/or chemical treatment to promote or affect the tactile quality and appearance of a food product.</obo:IAO_0000115>
        <oboInOwl:hasDbXref rdf:datatype="http://www.w3.org/2001/XMLSchema#string">http://www.langual.org/langual_thesaurus.asp?termid=H0192</oboInOwl:hasDbXref>
        <rdfs:label xml:lang="en">food texturing process</rdfs:label>
    </owl:Class>
    


    <!-- http://purl.obolibrary.org/obo/FOODON_03460194 -->

    <owl:Class rdf:about="http://purl.obolibrary.org/obo/FOODON_03460194">
        <rdfs:subClassOf rdf:resource="http://purl.obolibrary.org/obo/FOODON_03460225"/>
        <obo:IAO_0000115 xml:lang="en">A food is &apos;enriched&apos; when nutrients are added to it to replace those that are lost in processing; a food is &apos;fortified&apos; when nutrients that were never present are added to it.</obo:IAO_0000115>
        <oboInOwl:hasDbXref rdf:datatype="http://www.w3.org/2001/XMLSchema#string">http://www.langual.org/langual_thesaurus.asp?termid=H0194</oboInOwl:hasDbXref>
        <oboInOwl:hasSynonym xml:lang="en">enriched|fortified|restored</oboInOwl:hasSynonym>
        <rdfs:comment xml:lang="en">LanguaL curation note: Used when a chemical constituent is added for nutrient supplementation. Not used when the constituent is added to improve the functional properties of the food product. If the purpose of the constituent is not known, use the appropriate index term.</rdfs:comment>
        <rdfs:label xml:lang="en">nutrient or dietary substance addition process</rdfs:label>
    </owl:Class>
    


    <!-- http://purl.obolibrary.org/obo/FOODON_03460197 -->

    <owl:Class rdf:about="http://purl.obolibrary.org/obo/FOODON_03460197">
        <rdfs:subClassOf rdf:resource="http://purl.obolibrary.org/obo/FOODON_03460130"/>
        <obo:IAO_0000115 xml:lang="en">Treated with chemicals to reduce color, primarily to whiten, e.g., bleached flour.</obo:IAO_0000115>
        <oboInOwl:hasDbXref rdf:datatype="http://www.w3.org/2001/XMLSchema#string">http://www.langual.org/langual_thesaurus.asp?termid=H0197</oboInOwl:hasDbXref>
        <rdfs:label xml:lang="en">food bleaching process</rdfs:label>
    </owl:Class>
    


    <!-- http://purl.obolibrary.org/obo/FOODON_03460198 -->

    <owl:Class rdf:about="http://purl.obolibrary.org/obo/FOODON_03460198">
        <rdfs:subClassOf rdf:resource="http://purl.obolibrary.org/obo/FOODON_03460238"/>
        <oboInOwl:hasDbXref rdf:datatype="http://www.w3.org/2001/XMLSchema#string">http://www.langual.org/langual_thesaurus.asp?termid=H0198</oboInOwl:hasDbXref>
        <rdfs:label xml:lang="en">debittering process</rdfs:label>
    </owl:Class>
    


    <!-- http://purl.obolibrary.org/obo/FOODON_03460200 -->

    <owl:Class rdf:about="http://purl.obolibrary.org/obo/FOODON_03460200">
        <rdfs:subClassOf rdf:resource="http://purl.obolibrary.org/obo/FOODON_03460225"/>
        <oboInOwl:hasDbXref rdf:datatype="http://www.w3.org/2001/XMLSchema#string">http://www.langual.org/langual_thesaurus.asp?termid=H0200</oboInOwl:hasDbXref>
        <oboInOwl:hasSynonym xml:lang="en">pickled by acidification</oboInOwl:hasSynonym>
        <rdfs:comment xml:lang="en">LanguaL curation note: Used  when acid is added to a food product at any level.</rdfs:comment>
        <rdfs:label xml:lang="en">acidification process</rdfs:label>
    </owl:Class>
    


    <!-- http://purl.obolibrary.org/obo/FOODON_03460203 -->

    <owl:Class rdf:about="http://purl.obolibrary.org/obo/FOODON_03460203">
        <rdfs:subClassOf rdf:resource="http://purl.obolibrary.org/obo/FOODON_03460252"/>
        <oboInOwl:hasDbXref rdf:datatype="http://www.w3.org/2001/XMLSchema#string">http://www.langual.org/langual_thesaurus.asp?termid=H0203</oboInOwl:hasDbXref>
        <oboInOwl:hasSynonym xml:lang="en">converted (lactose)|delactosed</oboInOwl:hasSynonym>
        <rdfs:comment xml:lang="en">LanguaL curation note: Used when all or part of the lactose in milk is converted to glucose and galactose through enzymatic action.</rdfs:comment>
        <rdfs:label xml:lang="en">lactose conversion process</rdfs:label>
    </owl:Class>
    


    <!-- http://purl.obolibrary.org/obo/FOODON_03460206 -->

    <owl:Class rdf:about="http://purl.obolibrary.org/obo/FOODON_03460206">
        <rdfs:subClassOf rdf:resource="http://purl.obolibrary.org/obo/FOODON_03460130"/>
        <obo:IAO_0000115 xml:lang="en">Treated with a solution of alkali (primarily potassium or sodium carbonate). In cacao, alkalization neutralizes acids and leads to changes in flavor and color. In fats and oils, treatment with alkali leads to saponification of free fatty acids; soap and alkali are then removed.</obo:IAO_0000115>
        <oboInOwl:hasDbXref rdf:datatype="http://www.w3.org/2001/XMLSchema#string">http://www.langual.org/langual_thesaurus.asp?termid=H0206</oboInOwl:hasDbXref>
        <oboInOwl:hasSynonym xml:lang="en">alkalinized|dutch processed</oboInOwl:hasSynonym>
        <rdfs:label xml:lang="en">food alkalization process</rdfs:label>
    </owl:Class>
    


    <!-- http://purl.obolibrary.org/obo/FOODON_03460207 -->

    <owl:Class rdf:about="http://purl.obolibrary.org/obo/FOODON_03460207">
        <rdfs:subClassOf rdf:resource="http://purl.obolibrary.org/obo/FOODON_03460130"/>
        <rdfs:subClassOf>
            <owl:Restriction>
                <owl:onProperty rdf:resource="http://purl.obolibrary.org/obo/RO_0002233"/>
                <owl:someValuesFrom rdf:resource="http://purl.obolibrary.org/obo/FOODON_00001868"/>
            </owl:Restriction>
        </rdfs:subClassOf>
        <oboInOwl:hasDbXref rdf:datatype="http://www.w3.org/2001/XMLSchema#string">http://www.langual.org/langual_thesaurus.asp?termid=H0207</oboInOwl:hasDbXref>
        <oboInOwl:hasSynonym xml:lang="en">stuffing process</oboInOwl:hasSynonym>
        <rdfs:comment xml:lang="en">LanguaL curation note: Applies to all filled or stuffed products, including pies and sandwiches.</rdfs:comment>
        <rdfs:label xml:lang="en">food filling process</rdfs:label>
    </owl:Class>
    


    <!-- http://purl.obolibrary.org/obo/FOODON_03460208 -->

    <owl:Class rdf:about="http://purl.obolibrary.org/obo/FOODON_03460208">
        <rdfs:subClassOf rdf:resource="http://purl.obolibrary.org/obo/FOODON_03460103"/>
        <obo:IAO_0000115 xml:lang="en">Food product prepared from a natural food product by removing endogenous fat and adding fat from a different source, e.g., egg substitute, in which egg fat is replaced by vegetable oil.</obo:IAO_0000115>
        <oboInOwl:hasDbXref rdf:datatype="http://www.w3.org/2001/XMLSchema#string">http://www.langual.org/langual_thesaurus.asp?termid=H0208</oboInOwl:hasDbXref>
        <rdfs:label xml:lang="en">fat substitution process</rdfs:label>
    </owl:Class>
    


    <!-- http://purl.obolibrary.org/obo/FOODON_03460220 -->

    <owl:Class rdf:about="http://purl.obolibrary.org/obo/FOODON_03460220">
        <rdfs:subClassOf rdf:resource="http://purl.obolibrary.org/obo/FOODON_03450012"/>
        <rdfs:subClassOf rdf:resource="http://purl.obolibrary.org/obo/FOODON_03460130"/>
        <obo:IAO_0000115 xml:lang="en">Treated with moist heat to soften the grain and to transfer nutrients from the bran to the endosperm.</obo:IAO_0000115>
        <oboInOwl:hasDbXref rdf:datatype="http://www.w3.org/2001/XMLSchema#string">http://www.langual.org/langual_thesaurus.asp?termid=H0220</oboInOwl:hasDbXref>
        <oboInOwl:hasSynonym xml:lang="en">parboiled (rice)</oboInOwl:hasSynonym>
        <rdfs:label xml:lang="en">food parboiling process (grain)</rdfs:label>
    </owl:Class>
    


    <!-- http://purl.obolibrary.org/obo/FOODON_03460225 -->

    <owl:Class rdf:about="http://purl.obolibrary.org/obo/FOODON_03460225">
        <rdfs:subClassOf rdf:resource="http://purl.obolibrary.org/obo/FOODON_03460111"/>
        <obo:IAO_0000117 rdf:datatype="http://www.w3.org/2001/XMLSchema#string">Damion Dooley</obo:IAO_0000117>
        <oboInOwl:hasDbXref rdf:datatype="http://www.w3.org/2001/XMLSchema#string">http://www.langual.org/langual_thesaurus.asp?termid=H0225</oboInOwl:hasDbXref>
        <rdfs:comment xml:lang="en">LanguaL curation note: A food product is characterized by its main ingredient (food source and part); the addition of secondary ingredients is considered a treatment applied to the product. Secondary ingredients are indexed according to rules that are based on the order of predominance by weight (not counting water) as seen from the label statement, formulation or recipe and/or from the amount of the ingredient as percentage of total product weight. The general rule is:  an ingredient is always indexed if it is the second ingredient in order of predominance, if it is used as a filling, or if it is part of the product name(e.g., raisin bread). Specific rules are given in the scope note for the individual ingredient added; these rules specify more exhaustive indexing. For example, *MUSHROOM ADDED* is indexed regardless of ingredient position. another specific rule is given in the scope note for *SALTED*:  Use if the level of salt is more than 4%. Such a rule is used only when the percentage level can be inferred from the list of ingredients.</rdfs:comment>
        <rdfs:label xml:lang="en">food component addition process</rdfs:label>
    </owl:Class>
    


    <!-- http://purl.obolibrary.org/obo/FOODON_03460230 -->

    <owl:Class rdf:about="http://purl.obolibrary.org/obo/FOODON_03460230">
        <rdfs:subClassOf rdf:resource="http://purl.obolibrary.org/obo/FOODON_00001304"/>
        <oboInOwl:hasDbXref rdf:datatype="http://www.w3.org/2001/XMLSchema#string">http://www.langual.org/langual_thesaurus.asp?termid=H0230</oboInOwl:hasDbXref>
        <rdfs:comment xml:lang="en">LanguaL curation note: Used for products in which either carbohydrates, proteins or fats were modified through microbial processes. Enzymatic or other biological processes may also be involved. If two or more of these components are modified in significant amounts, index under *FERMENTED/MODIFIED, MULTIPLE COMPONENT*.</rdfs:comment>
        <rdfs:label xml:lang="en">single component food fermentation</rdfs:label>
    </owl:Class>
    


    <!-- http://purl.obolibrary.org/obo/FOODON_03460232 -->

    <owl:Class rdf:about="http://purl.obolibrary.org/obo/FOODON_03460232">
        <rdfs:subClassOf rdf:resource="http://purl.obolibrary.org/obo/FOODON_03460256"/>
        <oboInOwl:hasDbXref rdf:datatype="http://www.w3.org/2001/XMLSchema#string">http://www.langual.org/langual_thesaurus.asp?termid=H0232</oboInOwl:hasDbXref>
        <rdfs:label xml:lang="en">alcohol fermentation</rdfs:label>
    </owl:Class>
    


    <!-- http://purl.obolibrary.org/obo/FOODON_03460234 -->

    <owl:Class rdf:about="http://purl.obolibrary.org/obo/FOODON_03460234">
        <rdfs:subClassOf rdf:resource="http://purl.obolibrary.org/obo/FOODON_03460148"/>
        <oboInOwl:hasDbXref rdf:datatype="http://www.w3.org/2001/XMLSchema#string">http://www.langual.org/langual_thesaurus.asp?termid=H0234</oboInOwl:hasDbXref>
        <rdfs:label xml:lang="en">dilution process to 15-49% of single strength</rdfs:label>
    </owl:Class>
    


    <!-- http://purl.obolibrary.org/obo/FOODON_03460236 -->

    <owl:Class rdf:about="http://purl.obolibrary.org/obo/FOODON_03460236">
        <rdfs:subClassOf rdf:resource="http://purl.obolibrary.org/obo/FOODON_03460137"/>
        <oboInOwl:hasDbXref rdf:datatype="http://www.w3.org/2001/XMLSchema#string">http://www.langual.org/langual_thesaurus.asp?termid=H0236</oboInOwl:hasDbXref>
        <rdfs:comment xml:lang="en">LanguaL curation note: Used when naturally present sodium has been fully or partially removed. Index also by the appropriate term under *SALT OR SODIUM SPECIAL CLAIM OR USE*.</rdfs:comment>
        <rdfs:label xml:lang="en">sodium removal process</rdfs:label>
    </owl:Class>
    


    <!-- http://purl.obolibrary.org/obo/FOODON_03460237 -->

    <owl:Class rdf:about="http://purl.obolibrary.org/obo/FOODON_03460237">
        <rdfs:subClassOf rdf:resource="http://purl.obolibrary.org/obo/FOODON_03460148"/>
        <oboInOwl:hasDbXref rdf:datatype="http://www.w3.org/2001/XMLSchema#string">http://www.langual.org/langual_thesaurus.asp?termid=H0237</oboInOwl:hasDbXref>
        <rdfs:label xml:lang="en">dilution process to 50-99% of single strength</rdfs:label>
    </owl:Class>
    


    <!-- http://purl.obolibrary.org/obo/FOODON_03460238 -->

    <owl:Class rdf:about="http://purl.obolibrary.org/obo/FOODON_03460238">
        <rdfs:subClassOf rdf:resource="http://purl.obolibrary.org/obo/FOODON_03460111"/>
        <obo:IAO_0000115 xml:lang="en">A component separation process at the very least removes one component from an initial entity.  The removed component may be captured as a process output for reuse if not destroyed in the process of removal.</obo:IAO_0000115>
        <obo:IAO_0000117 rdf:datatype="http://www.w3.org/2001/XMLSchema#string">Damion Dooley</obo:IAO_0000117>
        <oboInOwl:hasDbXref rdf:datatype="http://www.w3.org/2001/XMLSchema#string">http://www.langual.org/langual_thesaurus.asp?termid=H0238</oboInOwl:hasDbXref>
        <rdfs:comment xml:lang="en">LanguaL curation note: Use the appropriate term under *COMPONENT REMOVED* to indicate the permanent full or partial removal of a nutritional/chemical component naturally present in the part of plant or animal used.</rdfs:comment>
        <rdfs:label xml:lang="en">component separation process</rdfs:label>
    </owl:Class>
    


    <!-- http://purl.obolibrary.org/obo/FOODON_03460239 -->

    <owl:Class rdf:about="http://purl.obolibrary.org/obo/FOODON_03460239">
        <rdfs:subClassOf rdf:resource="http://purl.obolibrary.org/obo/FOODON_00002409"/>
        <oboInOwl:hasDbXref rdf:datatype="http://www.w3.org/2001/XMLSchema#string">http://www.langual.org/langual_thesaurus.asp?termid=H0239</oboInOwl:hasDbXref>
        <rdfs:comment xml:lang="en">LanguaL curation note: Used for a grain in which the kernels have been physically compressed between heated rollers.</rdfs:comment>
        <rdfs:label xml:lang="en">food rolling process</rdfs:label>
    </owl:Class>
    


    <!-- http://purl.obolibrary.org/obo/FOODON_03460241 -->

    <owl:Class rdf:about="http://purl.obolibrary.org/obo/FOODON_03460241">
        <rdfs:subClassOf rdf:resource="http://purl.obolibrary.org/obo/FOODON_03460130"/>
        <oboInOwl:hasDbXref rdf:datatype="http://www.w3.org/2001/XMLSchema#string">http://www.langual.org/langual_thesaurus.asp?termid=H0241</oboInOwl:hasDbXref>
        <oboInOwl:hasSynonym xml:lang="en">frozen previously</oboInOwl:hasSynonym>
        <rdfs:comment xml:lang="en">LanguaL curation note: Used when the product or any indexed ingredient was frozen and then thawed. Excludes freeze-dried products and freeze-flo products.</rdfs:comment>
        <rdfs:label xml:lang="en">food thawing process</rdfs:label>
    </owl:Class>
    


    <!-- http://purl.obolibrary.org/obo/FOODON_03460246 -->

    <owl:Class rdf:about="http://purl.obolibrary.org/obo/FOODON_03460246">
        <rdfs:subClassOf rdf:resource="http://purl.obolibrary.org/obo/FOODON_03460175"/>
        <oboInOwl:hasDbXref rdf:datatype="http://www.w3.org/2001/XMLSchema#string">http://www.langual.org/langual_thesaurus.asp?termid=H0246</oboInOwl:hasDbXref>
        <rdfs:comment xml:lang="en">LanguaL curation note: Used when carbon dioxide produced by fermentation remains noticeable in the food product. Damion Dooley&apos;s note: converted to a process</rdfs:comment>
        <rdfs:label xml:lang="en">carbonation by fermentation</rdfs:label>
    </owl:Class>
    


    <!-- http://purl.obolibrary.org/obo/FOODON_03460247 -->

    <owl:Class rdf:about="http://purl.obolibrary.org/obo/FOODON_03460247">
        <rdfs:subClassOf rdf:resource="http://purl.obolibrary.org/obo/FOODON_03460161"/>
        <oboInOwl:hasDbXref rdf:datatype="http://www.w3.org/2001/XMLSchema#string">http://www.langual.org/langual_thesaurus.asp?termid=H0247</oboInOwl:hasDbXref>
        <oboInOwl:hasSynonym xml:lang="en">dry roasted</oboInOwl:hasSynonym>
        <rdfs:comment xml:lang="en">LanguaL curation note: Used for products that contain between 10-20% and 60% of the fat naturally present in the food source. Examples are breakfast cocoa, low fat milk and low-fat cottage cheese.</rdfs:comment>
        <rdfs:label xml:lang="en">partial fat removal process</rdfs:label>
    </owl:Class>
    


    <!-- http://purl.obolibrary.org/obo/FOODON_03460248 -->

    <owl:Class rdf:about="http://purl.obolibrary.org/obo/FOODON_03460248">
        <rdfs:subClassOf rdf:resource="http://purl.obolibrary.org/obo/FOODON_03460161"/>
        <oboInOwl:hasDbXref rdf:datatype="http://www.w3.org/2001/XMLSchema#string">http://www.langual.org/langual_thesaurus.asp?termid=H0248</oboInOwl:hasDbXref>
        <rdfs:comment xml:lang="en">LanguaL curation note: Used for products that contain less than 10-20% of the fat naturally present in the food source. Examples are skim milk, low-fat cocoa and dry-curd cottage cheese.</rdfs:comment>
        <rdfs:label xml:lang="en">full fat removal process</rdfs:label>
    </owl:Class>
    


    <!-- http://purl.obolibrary.org/obo/FOODON_03460250 -->

    <owl:Class rdf:about="http://purl.obolibrary.org/obo/FOODON_03460250">
        <rdfs:subClassOf rdf:resource="http://purl.obolibrary.org/obo/FOODON_03460103"/>
        <oboInOwl:hasDbXref rdf:datatype="http://www.w3.org/2001/XMLSchema#string">http://www.langual.org/langual_thesaurus.asp?termid=H0250</oboInOwl:hasDbXref>
        <rdfs:label xml:lang="en">protein substitution process</rdfs:label>
    </owl:Class>
    


    <!-- http://purl.obolibrary.org/obo/FOODON_03460252 -->

    <owl:Class rdf:about="http://purl.obolibrary.org/obo/FOODON_03460252">
        <rdfs:subClassOf rdf:resource="http://purl.obolibrary.org/obo/FOODON_03460119"/>
        <oboInOwl:hasDbXref rdf:datatype="http://www.w3.org/2001/XMLSchema#string">http://www.langual.org/langual_thesaurus.asp?termid=H0252</oboInOwl:hasDbXref>
        <rdfs:comment xml:lang="en">LanguaL curation note: Used for products in which one or more components were converted through the addition of enzymes or through activation of endogenous enzymes.</rdfs:comment>
        <rdfs:label xml:lang="en">enzymatic modification process</rdfs:label>
    </owl:Class>
    


    <!-- http://purl.obolibrary.org/obo/FOODON_03460253 -->

    <owl:Class rdf:about="http://purl.obolibrary.org/obo/FOODON_03460253">
        <rdfs:subClassOf rdf:resource="http://purl.obolibrary.org/obo/FOODON_03460128"/>
        <obo:IAO_0000115 xml:lang="en">Modified through complex enzymatic or microbial processes resulting in physicochemical changes in particular with respect to texture, flavor, color or shelf life of the food product. Such changes may be induced by the introduction of certain chemicals, such as sodium sulfite, salt, sugar, or other substances, such as phenolics, in dry or liquid form and often aided by smoke. Cheese should always be indexed by the appropriate narrower term under *LACTIC ACID-OTHER AGENT FERMENTED*.</obo:IAO_0000115>
        <oboInOwl:hasDbXref rdf:datatype="http://www.w3.org/2001/XMLSchema#string">http://www.langual.org/langual_thesaurus.asp?termid=H0253</oboInOwl:hasDbXref>
        <oboInOwl:hasSynonym xml:lang="en">aged</oboInOwl:hasSynonym>
        <rdfs:label xml:lang="en">curing or aging</rdfs:label>
    </owl:Class>
    


    <!-- http://purl.obolibrary.org/obo/FOODON_03460254 -->

    <owl:Class rdf:about="http://purl.obolibrary.org/obo/FOODON_03460254">
        <owl:equivalentClass>
            <owl:Class>
                <owl:unionOf rdf:parseType="Collection">
                    <rdf:Description rdf:about="http://purl.obolibrary.org/obo/FOODON_03460138"/>
                    <rdf:Description rdf:about="http://purl.obolibrary.org/obo/FOODON_03460148"/>
                </owl:unionOf>
            </owl:Class>
        </owl:equivalentClass>
        <rdfs:subClassOf rdf:resource="http://purl.obolibrary.org/obo/FOODON_03460111"/>
        <oboInOwl:hasDbXref rdf:datatype="http://www.w3.org/2001/XMLSchema#string">http://www.langual.org/langual_thesaurus.asp?termid=H0254</oboInOwl:hasDbXref>
        <rdfs:comment xml:lang="en">LanguaL curation note: Used when water is added or removed in order to change the total solids-to-liquids ratio of a food product.</rdfs:comment>
        <rdfs:label xml:lang="en">water addition or removal process</rdfs:label>
    </owl:Class>
    


    <!-- http://purl.obolibrary.org/obo/FOODON_03460256 -->

    <owl:Class rdf:about="http://purl.obolibrary.org/obo/FOODON_03460256">
        <rdfs:subClassOf rdf:resource="http://purl.obolibrary.org/obo/FOODON_03460230"/>
        <rdfs:subClassOf>
            <owl:Restriction>
                <owl:onProperty rdf:resource="http://purl.obolibrary.org/obo/RO_0002233"/>
                <owl:someValuesFrom rdf:resource="http://purl.obolibrary.org/obo/FOODON_03411345"/>
            </owl:Restriction>
        </rdfs:subClassOf>
        <oboInOwl:hasDbXref rdf:datatype="http://www.w3.org/2001/XMLSchema#string">http://www.langual.org/langual_thesaurus.asp?termid=H0256</oboInOwl:hasDbXref>
        <oboInOwl:hasSynonym xml:lang="en">yeast leavened</oboInOwl:hasSynonym>
        <rdfs:label xml:lang="en">carbohydrate fermentation</rdfs:label>
    </owl:Class>
    


    <!-- http://purl.obolibrary.org/obo/FOODON_03460259 -->

    <owl:Class rdf:about="http://purl.obolibrary.org/obo/FOODON_03460259">
        <rdfs:subClassOf rdf:resource="http://purl.obolibrary.org/obo/FOODON_03460148"/>
        <rdfs:subClassOf rdf:resource="http://purl.obolibrary.org/obo/FOODON_03460225"/>
        <oboInOwl:hasDbXref rdf:datatype="http://www.w3.org/2001/XMLSchema#string">http://www.langual.org/langual_thesaurus.asp?termid=H0259</oboInOwl:hasDbXref>
        <oboInOwl:hasSynonym xml:lang="en">made from concentrate|moistened|previously concentrated|reconstituted to liquid|soaked</oboInOwl:hasSynonym>
        <rdfs:comment xml:lang="en">LanguaL curation note: Used for a product that is prepared by adding water or a water-based liquid (milk, juice, broth) to a dehydrated or concentrated product or to a product that contains an indexed dehydrated ingredient plus water to rehydrate that ingredient. Examples:  juice or juice drink from concentrate; milk reconstituted from dry or concentrated milk; soaked dried beans or stewed fruit; biscuit dough (prepared by rehydrating flour); soup made from dehydrated ingredients; cooked noodles or boiled rice. If the resulting product contains water beyond its natural water level, also index *WATER ADDED*.</rdfs:comment>
        <rdfs:label xml:lang="en">rehydration process</rdfs:label>
    </owl:Class>
    


    <!-- http://purl.obolibrary.org/obo/FOODON_03460261 -->

    <owl:Class rdf:about="http://purl.obolibrary.org/obo/FOODON_03460261">
        <rdfs:subClassOf rdf:resource="http://purl.obolibrary.org/obo/FOODON_03460121"/>
        <oboInOwl:hasDbXref rdf:datatype="http://www.w3.org/2001/XMLSchema#string">http://www.langual.org/langual_thesaurus.asp?termid=H0261</oboInOwl:hasDbXref>
        <rdfs:label xml:lang="en">food ultraviolet radiation process</rdfs:label>
    </owl:Class>
    


    <!-- http://purl.obolibrary.org/obo/FOODON_03460266 -->

    <owl:Class rdf:about="http://purl.obolibrary.org/obo/FOODON_03460266">
        <rdfs:subClassOf rdf:resource="http://purl.obolibrary.org/obo/FOODON_03460238"/>
        <oboInOwl:hasDbXref rdf:datatype="http://www.w3.org/2001/XMLSchema#string">http://www.langual.org/langual_thesaurus.asp?termid=H0266</oboInOwl:hasDbXref>
        <rdfs:label xml:lang="en">carbohydrate removal process</rdfs:label>
    </owl:Class>
    


    <!-- http://purl.obolibrary.org/obo/FOODON_03460268 -->

    <owl:Class rdf:about="http://purl.obolibrary.org/obo/FOODON_03460268">
        <rdfs:subClassOf rdf:resource="http://purl.obolibrary.org/obo/FOODON_03460130"/>
        <oboInOwl:hasDbXref rdf:datatype="http://www.w3.org/2001/XMLSchema#string">http://www.langual.org/langual_thesaurus.asp?termid=H0268</oboInOwl:hasDbXref>
        <rdfs:label xml:lang="en">food puffing process</rdfs:label>
    </owl:Class>
    


    <!-- http://purl.obolibrary.org/obo/FOODON_03460270 -->

    <owl:Class rdf:about="http://purl.obolibrary.org/obo/FOODON_03460270">
        <rdfs:subClassOf rdf:resource="http://purl.obolibrary.org/obo/FOODON_03460130"/>
        <oboInOwl:hasDbXref rdf:datatype="http://www.w3.org/2001/XMLSchema#string">http://www.langual.org/langual_thesaurus.asp?termid=H0270</oboInOwl:hasDbXref>
        <rdfs:label xml:lang="en">food distillation process</rdfs:label>
    </owl:Class>
    


    <!-- http://purl.obolibrary.org/obo/FOODON_03460274 -->

    <owl:Class rdf:about="http://purl.obolibrary.org/obo/FOODON_03460274">
        <rdfs:subClassOf rdf:resource="http://purl.obolibrary.org/obo/FOODON_00002409"/>
        <oboInOwl:hasDbXref rdf:datatype="http://www.w3.org/2001/XMLSchema#string">http://www.langual.org/langual_thesaurus.asp?termid=H0274</oboInOwl:hasDbXref>
        <rdfs:comment xml:lang="en">LanguaL curation note: Used only for breakfast cereals made by forcing cooked particles of grain or tiny pellets of dough between very heavy rollers that convert each piece into a single flake.</rdfs:comment>
        <rdfs:label xml:lang="en">food flaking process</rdfs:label>
    </owl:Class>
    


    <!-- http://purl.obolibrary.org/obo/FOODON_03460275 -->

    <owl:Class rdf:about="http://purl.obolibrary.org/obo/FOODON_03460275">
        <rdfs:subClassOf rdf:resource="http://purl.obolibrary.org/obo/FOODON_03460130"/>
        <oboInOwl:hasDbXref rdf:datatype="http://www.w3.org/2001/XMLSchema#string">http://www.langual.org/langual_thesaurus.asp?termid=H0275</oboInOwl:hasDbXref>
        <oboInOwl:hasSynonym xml:lang="en">enhanced|prebasted</oboInOwl:hasSynonym>
        <rdfs:comment xml:lang="en">LanguaL curation note: Used when liquid is injected into a meat or poultry is prebasted. Do not confuse with *WATER ADDED*.</rdfs:comment>
        <rdfs:label xml:lang="en">food meat liquid injection process</rdfs:label>
    </owl:Class>
    


    <!-- http://purl.obolibrary.org/obo/FOODON_03460276 -->

    <owl:Class rdf:about="http://purl.obolibrary.org/obo/FOODON_03460276">
        <rdfs:subClassOf rdf:resource="http://purl.obolibrary.org/obo/FOODON_03460130"/>
        <oboInOwl:hasDbXref rdf:datatype="http://www.w3.org/2001/XMLSchema#string">http://www.langual.org/langual_thesaurus.asp?termid=H0276</oboInOwl:hasDbXref>
        <rdfs:label xml:lang="en">food bromination process</rdfs:label>
    </owl:Class>
    


    <!-- http://purl.obolibrary.org/obo/FOODON_03460277 -->

    <owl:Class rdf:about="http://purl.obolibrary.org/obo/FOODON_03460277">
        <rdfs:subClassOf rdf:resource="http://purl.obolibrary.org/obo/FOODON_03460130"/>
        <oboInOwl:hasDbXref rdf:datatype="http://www.w3.org/2001/XMLSchema#string">http://www.langual.org/langual_thesaurus.asp?termid=H0277</oboInOwl:hasDbXref>
        <rdfs:label xml:lang="en">food hydrolyzation process</rdfs:label>
    </owl:Class>
    


    <!-- http://purl.obolibrary.org/obo/FOODON_03460278 -->

    <owl:Class rdf:about="http://purl.obolibrary.org/obo/FOODON_03460278">
        <rdfs:subClassOf rdf:resource="http://purl.obolibrary.org/obo/FOODON_03460130"/>
        <oboInOwl:hasDbXref rdf:datatype="http://www.w3.org/2001/XMLSchema#string">http://www.langual.org/langual_thesaurus.asp?termid=H0278</oboInOwl:hasDbXref>
        <rdfs:label xml:lang="en">food phosphating process</rdfs:label>
    </owl:Class>
    


    <!-- http://purl.obolibrary.org/obo/FOODON_03460285 -->

    <owl:Class rdf:about="http://purl.obolibrary.org/obo/FOODON_03460285">
        <rdfs:subClassOf rdf:resource="http://purl.obolibrary.org/obo/FOODON_03460238"/>
        <oboInOwl:hasDbXref rdf:datatype="http://www.w3.org/2001/XMLSchema#string">http://www.langual.org/langual_thesaurus.asp?termid=H0285</oboInOwl:hasDbXref>
        <rdfs:comment xml:lang="en">LanguaL curation note: Used for products from which alcohol has been removed.</rdfs:comment>
        <rdfs:label xml:lang="en">alcohol removal process</rdfs:label>
    </owl:Class>
    


    <!-- http://purl.obolibrary.org/obo/FOODON_03460286 -->

    <owl:Class rdf:about="http://purl.obolibrary.org/obo/FOODON_03460286">
        <rdfs:subClassOf rdf:resource="http://purl.obolibrary.org/obo/FOODON_03460285"/>
        <oboInOwl:hasDbXref rdf:datatype="http://www.w3.org/2001/XMLSchema#string">http://www.langual.org/langual_thesaurus.asp?termid=H0286</oboInOwl:hasDbXref>
        <rdfs:comment xml:lang="en">LanguaL curation note: Used for products from which alcohol has been removed to less than 0.5% alcohol by volume.</rdfs:comment>
        <rdfs:label xml:lang="en">full alcohol removal process</rdfs:label>
    </owl:Class>
    


    <!-- http://purl.obolibrary.org/obo/FOODON_03460287 -->

    <owl:Class rdf:about="http://purl.obolibrary.org/obo/FOODON_03460287">
        <rdfs:subClassOf rdf:resource="http://purl.obolibrary.org/obo/FOODON_03460285"/>
        <oboInOwl:hasDbXref rdf:datatype="http://www.w3.org/2001/XMLSchema#string">http://www.langual.org/langual_thesaurus.asp?termid=H0287</oboInOwl:hasDbXref>
        <rdfs:comment xml:lang="en">LanguaL curation note: Used for products from which alcohol has been removed to 0.5% or more alcohol by volume.</rdfs:comment>
        <rdfs:label xml:lang="en">partial alcohol removal process</rdfs:label>
    </owl:Class>
    


    <!-- http://purl.obolibrary.org/obo/FOODON_03460288 -->

    <owl:Class rdf:about="http://purl.obolibrary.org/obo/FOODON_03460288">
        <rdfs:subClassOf rdf:resource="http://purl.obolibrary.org/obo/FOODON_03460253"/>
        <oboInOwl:hasDbXref rdf:datatype="http://www.w3.org/2001/XMLSchema#string">http://www.langual.org/langual_thesaurus.asp?termid=H0288</oboInOwl:hasDbXref>
        <rdfs:label xml:lang="en">curing or aging &lt; 2 weeks</rdfs:label>
    </owl:Class>
    


    <!-- http://purl.obolibrary.org/obo/FOODON_03460289 -->

    <owl:Class rdf:about="http://purl.obolibrary.org/obo/FOODON_03460289">
        <rdfs:subClassOf rdf:resource="http://purl.obolibrary.org/obo/FOODON_03460253"/>
        <oboInOwl:hasDbXref rdf:datatype="http://www.w3.org/2001/XMLSchema#string">http://www.langual.org/langual_thesaurus.asp?termid=H0289</oboInOwl:hasDbXref>
        <rdfs:label xml:lang="en">curing or aging 2 weeks to 1 month</rdfs:label>
    </owl:Class>
    


    <!-- http://purl.obolibrary.org/obo/FOODON_03460290 -->

    <owl:Class rdf:about="http://purl.obolibrary.org/obo/FOODON_03460290">
        <rdfs:subClassOf rdf:resource="http://purl.obolibrary.org/obo/FOODON_03460253"/>
        <oboInOwl:hasDbXref rdf:datatype="http://www.w3.org/2001/XMLSchema#string">http://www.langual.org/langual_thesaurus.asp?termid=H0290</oboInOwl:hasDbXref>
        <rdfs:label xml:lang="en">curing or aging 1 to 2 months</rdfs:label>
    </owl:Class>
    


    <!-- http://purl.obolibrary.org/obo/FOODON_03460291 -->

    <owl:Class rdf:about="http://purl.obolibrary.org/obo/FOODON_03460291">
        <rdfs:subClassOf rdf:resource="http://purl.obolibrary.org/obo/FOODON_03460253"/>
        <oboInOwl:hasDbXref rdf:datatype="http://www.w3.org/2001/XMLSchema#string">http://www.langual.org/langual_thesaurus.asp?termid=H0291</oboInOwl:hasDbXref>
        <rdfs:label xml:lang="en">curing or aging 2 to 4 months</rdfs:label>
    </owl:Class>
    


    <!-- http://purl.obolibrary.org/obo/FOODON_03460292 -->

    <owl:Class rdf:about="http://purl.obolibrary.org/obo/FOODON_03460292">
        <rdfs:subClassOf rdf:resource="http://purl.obolibrary.org/obo/FOODON_03460253"/>
        <oboInOwl:hasDbXref rdf:datatype="http://www.w3.org/2001/XMLSchema#string">http://www.langual.org/langual_thesaurus.asp?termid=H0292</oboInOwl:hasDbXref>
        <rdfs:label xml:lang="en">curing or aging 4 to 6 months</rdfs:label>
    </owl:Class>
    


    <!-- http://purl.obolibrary.org/obo/FOODON_03460293 -->

    <owl:Class rdf:about="http://purl.obolibrary.org/obo/FOODON_03460293">
        <rdfs:subClassOf rdf:resource="http://purl.obolibrary.org/obo/FOODON_03460253"/>
        <oboInOwl:hasDbXref rdf:datatype="http://www.w3.org/2001/XMLSchema#string">http://www.langual.org/langual_thesaurus.asp?termid=H0293</oboInOwl:hasDbXref>
        <rdfs:label xml:lang="en">curing or aging 6 to 12 months</rdfs:label>
    </owl:Class>
    


    <!-- http://purl.obolibrary.org/obo/FOODON_03460294 -->

    <owl:Class rdf:about="http://purl.obolibrary.org/obo/FOODON_03460294">
        <rdfs:subClassOf rdf:resource="http://purl.obolibrary.org/obo/FOODON_03460253"/>
        <oboInOwl:hasDbXref rdf:datatype="http://www.w3.org/2001/XMLSchema#string">http://www.langual.org/langual_thesaurus.asp?termid=H0294</oboInOwl:hasDbXref>
        <rdfs:label xml:lang="en">curing or aging 12 months or over</rdfs:label>
    </owl:Class>
    


    <!-- http://purl.obolibrary.org/obo/FOODON_03460295 -->

    <owl:Class rdf:about="http://purl.obolibrary.org/obo/FOODON_03460295">
        <rdfs:subClassOf rdf:resource="http://purl.obolibrary.org/obo/FOODON_03460266"/>
        <oboInOwl:hasDbXref rdf:datatype="http://www.w3.org/2001/XMLSchema#string">http://www.langual.org/langual_thesaurus.asp?termid=H0295</oboInOwl:hasDbXref>
        <rdfs:comment xml:lang="en">LanguaL curation note: Used when lactose is removed from the food product as when washing curd for cheese preparation. When lactose content is reduced by enzymatic conversion of lactose, use *LACTOSE CONVERTED*.</rdfs:comment>
        <rdfs:label xml:lang="en">lactose removal process</rdfs:label>
    </owl:Class>
    


    <!-- http://purl.obolibrary.org/obo/FOODON_03460298 -->

    <owl:Class rdf:about="http://purl.obolibrary.org/obo/FOODON_03460298">
        <rdfs:subClassOf rdf:resource="http://purl.obolibrary.org/obo/FOODON_03460252"/>
        <oboInOwl:hasDbXref rdf:datatype="http://www.w3.org/2001/XMLSchema#string">http://www.langual.org/langual_thesaurus.asp?termid=H0298</oboInOwl:hasDbXref>
        <oboInOwl:hasExactSynonym xml:lang="en">rennin (rennet) coagulation</oboInOwl:hasExactSynonym>
        <rdfs:comment xml:lang="en">LanguaL curation note: Used when a clotting enzyme is added to a food product at any level.</rdfs:comment>
        <rdfs:label xml:lang="en">clotting enzyme addition process</rdfs:label>
    </owl:Class>
    


    <!-- http://purl.obolibrary.org/obo/FOODON_03460300 -->

    <owl:Class rdf:about="http://purl.obolibrary.org/obo/FOODON_03460300">
        <rdfs:subClassOf rdf:resource="http://purl.obolibrary.org/obo/FOODON_03460256"/>
        <oboInOwl:hasDbXref rdf:datatype="http://www.w3.org/2001/XMLSchema#string">http://www.langual.org/langual_thesaurus.asp?termid=H0300</oboInOwl:hasDbXref>
        <rdfs:label xml:lang="en">acetic acid fermentation</rdfs:label>
    </owl:Class>
    


    <!-- http://purl.obolibrary.org/obo/FOODON_03460306 -->

    <owl:Class rdf:about="http://purl.obolibrary.org/obo/FOODON_03460306">
        <rdfs:subClassOf rdf:resource="http://purl.obolibrary.org/obo/FOODON_03460130"/>
        <oboInOwl:hasDbXref rdf:datatype="http://www.w3.org/2001/XMLSchema#string">http://www.langual.org/langual_thesaurus.asp?termid=H0306</oboInOwl:hasDbXref>
        <oboInOwl:hasExactSynonym xml:lang="en">emulsification | homogenization</oboInOwl:hasExactSynonym>
        <rdfs:comment xml:lang="en">LanguaL curation note: Used for products in which two or more phases are mixed very finely but not at the molecular level. A very fine dispersion of a solid in a liquid is called a suspension. A very fine dispersion of one liquid in another immiscible liquid is called an emulsion.</rdfs:comment>
        <rdfs:label xml:lang="en">food homogenization or emulsification process</rdfs:label>
    </owl:Class>
    


    <!-- http://purl.obolibrary.org/obo/FOODON_03460324 -->

    <owl:Class rdf:about="http://purl.obolibrary.org/obo/FOODON_03460324">
        <rdfs:subClassOf rdf:resource="http://purl.obolibrary.org/obo/FOODON_03460247"/>
        <oboInOwl:hasDbXref rdf:datatype="http://www.w3.org/2001/XMLSchema#string">http://www.langual.org/langual_thesaurus.asp?termid=H0324</oboInOwl:hasDbXref>
        <rdfs:comment xml:lang="en">LanguaL curation note: Used for food products that have had fat partially removed to leave more than 50% fat from a full fat product. An example would 2% milk where full fat milk is 4%.</rdfs:comment>
        <rdfs:label xml:lang="en">partial fat removal process, 50% or more remaining</rdfs:label>
    </owl:Class>
    


    <!-- http://purl.obolibrary.org/obo/FOODON_03460325 -->

    <owl:Class rdf:about="http://purl.obolibrary.org/obo/FOODON_03460325">
        <rdfs:subClassOf rdf:resource="http://purl.obolibrary.org/obo/FOODON_03460247"/>
        <oboInOwl:hasDbXref rdf:datatype="http://www.w3.org/2001/XMLSchema#string">http://www.langual.org/langual_thesaurus.asp?termid=H0325</oboInOwl:hasDbXref>
        <rdfs:comment xml:lang="en">LanguaL curation note: Used for food products that have had fat removed to leave less than 50% fat from a full fat product. Examples would be 1% milk or 1/2% milk, where full fat milk is 4%.</rdfs:comment>
        <rdfs:label xml:lang="en">partial fat removal process, less than 50% remaining</rdfs:label>
    </owl:Class>
    


    <!-- http://purl.obolibrary.org/obo/FOODON_03460326 -->

    <owl:Class rdf:about="http://purl.obolibrary.org/obo/FOODON_03460326">
        <rdfs:subClassOf rdf:resource="http://purl.obolibrary.org/obo/FOODON_03460107"/>
        <oboInOwl:hasDbXref rdf:datatype="http://www.w3.org/2001/XMLSchema#string">http://www.langual.org/langual_thesaurus.asp?termid=H0326</oboInOwl:hasDbXref>
        <rdfs:label xml:lang="en">bacterial food-curing process</rdfs:label>
    </owl:Class>
    


    <!-- http://purl.obolibrary.org/obo/FOODON_03460327 -->

    <owl:Class rdf:about="http://purl.obolibrary.org/obo/FOODON_03460327">
        <rdfs:subClassOf rdf:resource="http://purl.obolibrary.org/obo/FOODON_03460326"/>
        <oboInOwl:hasDbXref rdf:datatype="http://www.w3.org/2001/XMLSchema#string">http://www.langual.org/langual_thesaurus.asp?termid=H0327</oboInOwl:hasDbXref>
        <rdfs:label xml:lang="en">food surface bacterial curing</rdfs:label>
    </owl:Class>
    


    <!-- http://purl.obolibrary.org/obo/FOODON_03460328 -->

    <owl:Class rdf:about="http://purl.obolibrary.org/obo/FOODON_03460328">
        <rdfs:subClassOf rdf:resource="http://purl.obolibrary.org/obo/FOODON_03460326"/>
        <oboInOwl:hasDbXref rdf:datatype="http://www.w3.org/2001/XMLSchema#string">http://www.langual.org/langual_thesaurus.asp?termid=H0328</oboInOwl:hasDbXref>
        <rdfs:label xml:lang="en">food interior bacterial curing</rdfs:label>
    </owl:Class>
    


    <!-- http://purl.obolibrary.org/obo/FOODON_03460329 -->

    <owl:Class rdf:about="http://purl.obolibrary.org/obo/FOODON_03460329">
        <rdfs:subClassOf rdf:resource="http://purl.obolibrary.org/obo/FOODON_03460107"/>
        <oboInOwl:hasDbXref rdf:datatype="http://www.w3.org/2001/XMLSchema#string">http://www.langual.org/langual_thesaurus.asp?termid=H0329</oboInOwl:hasDbXref>
        <rdfs:label xml:lang="en">mold food-curing process</rdfs:label>
    </owl:Class>
    


    <!-- http://purl.obolibrary.org/obo/FOODON_03460330 -->

    <owl:Class rdf:about="http://purl.obolibrary.org/obo/FOODON_03460330">
        <rdfs:subClassOf rdf:resource="http://purl.obolibrary.org/obo/FOODON_03460329"/>
        <oboInOwl:hasDbXref rdf:datatype="http://www.w3.org/2001/XMLSchema#string">http://www.langual.org/langual_thesaurus.asp?termid=H0330</oboInOwl:hasDbXref>
        <rdfs:label xml:lang="en">food surface mold curing</rdfs:label>
    </owl:Class>
    


    <!-- http://purl.obolibrary.org/obo/FOODON_03460331 -->

    <owl:Class rdf:about="http://purl.obolibrary.org/obo/FOODON_03460331">
        <rdfs:subClassOf rdf:resource="http://purl.obolibrary.org/obo/FOODON_03460329"/>
        <oboInOwl:hasDbXref rdf:datatype="http://www.w3.org/2001/XMLSchema#string">http://www.langual.org/langual_thesaurus.asp?termid=H0331</oboInOwl:hasDbXref>
        <rdfs:label xml:lang="en">food interior mold curing</rdfs:label>
    </owl:Class>
    


    <!-- http://purl.obolibrary.org/obo/FOODON_03460351 -->

    <owl:Class rdf:about="http://purl.obolibrary.org/obo/FOODON_03460351">
        <rdfs:subClassOf rdf:resource="http://purl.obolibrary.org/obo/FOODON_03460751"/>
        <oboInOwl:hasDbXref rdf:datatype="http://www.w3.org/2001/XMLSchema#string">http://www.langual.org/langual_thesaurus.asp?termid=H0351</oboInOwl:hasDbXref>
        <oboInOwl:hasExactSynonym xml:lang="en">baking powder addition | baking soda addition</oboInOwl:hasExactSynonym>
        <rdfs:label xml:lang="en">chemical leavening agent addition process</rdfs:label>
    </owl:Class>
    


    <!-- http://purl.obolibrary.org/obo/FOODON_03460352 -->

    <owl:Class rdf:about="http://purl.obolibrary.org/obo/FOODON_03460352">
        <rdfs:subClassOf rdf:resource="http://purl.obolibrary.org/obo/FOODON_00002409"/>
        <obo:IAO_0000115 xml:lang="en">Modified through a physical or chemical procedure by forcing a food mixture through a die to achieve a particular shape.</obo:IAO_0000115>
        <oboInOwl:hasDbXref rdf:datatype="http://www.w3.org/2001/XMLSchema#string">http://www.langual.org/langual_thesaurus.asp?termid=H0352</oboInOwl:hasDbXref>
        <rdfs:label xml:lang="en">food extrusion</rdfs:label>
    </owl:Class>
    


    <!-- http://purl.obolibrary.org/obo/FOODON_03460353 -->

    <owl:Class rdf:about="http://purl.obolibrary.org/obo/FOODON_03460353">
        <rdfs:subClassOf rdf:resource="http://purl.obolibrary.org/obo/FOODON_03460130"/>
        <oboInOwl:hasDbXref rdf:datatype="http://www.w3.org/2001/XMLSchema#string">http://www.langual.org/langual_thesaurus.asp?termid=H0353</oboInOwl:hasDbXref>
        <oboInOwl:hasExactSynonym xml:lang="en">glazing process | food covering process | food coating process</oboInOwl:hasExactSynonym>
        <rdfs:label xml:lang="en">food coating or covering process</rdfs:label>
    </owl:Class>
    


    <!-- http://purl.obolibrary.org/obo/FOODON_03460354 -->

    <owl:Class rdf:about="http://purl.obolibrary.org/obo/FOODON_03460354">
        <rdfs:subClassOf rdf:resource="http://purl.obolibrary.org/obo/FOODON_03460353"/>
        <oboInOwl:hasDbXref rdf:datatype="http://www.w3.org/2001/XMLSchema#string">http://www.langual.org/langual_thesaurus.asp?termid=H0354</oboInOwl:hasDbXref>
        <oboInOwl:hasExactSynonym xml:lang="en">sugar coating | sugar covering</oboInOwl:hasExactSynonym>
        <rdfs:label xml:lang="en">sugar coating or covering process</rdfs:label>
    </owl:Class>
    


    <!-- http://purl.obolibrary.org/obo/FOODON_03460355 -->

    <owl:Class rdf:about="http://purl.obolibrary.org/obo/FOODON_03460355">
        <rdfs:subClassOf rdf:resource="http://purl.obolibrary.org/obo/FOODON_03460353"/>
        <oboInOwl:hasDbXref rdf:datatype="http://www.w3.org/2001/XMLSchema#string">http://www.langual.org/langual_thesaurus.asp?termid=H0355</oboInOwl:hasDbXref>
        <oboInOwl:hasExactSynonym xml:lang="en">chocolate coating | chocolate covering</oboInOwl:hasExactSynonym>
        <rdfs:comment xml:lang="en">LanguaL curation note: Includes chocolate coatings for such products as candy and ice cream products as well as icings and frostings for such products as cakes and doughnuts.</rdfs:comment>
        <rdfs:label xml:lang="en">chocolate coating or covering process</rdfs:label>
    </owl:Class>
    


    <!-- http://purl.obolibrary.org/obo/FOODON_03460357 -->

    <owl:Class rdf:about="http://purl.obolibrary.org/obo/FOODON_03460357">
        <rdfs:subClassOf rdf:resource="http://purl.obolibrary.org/obo/FOODON_03460353"/>
        <oboInOwl:hasDbXref rdf:datatype="http://www.w3.org/2001/XMLSchema#string">http://www.langual.org/langual_thesaurus.asp?termid=H0357</oboInOwl:hasDbXref>
        <oboInOwl:hasExactSynonym xml:lang="en">carob coating | carob covering</oboInOwl:hasExactSynonym>
        <rdfs:comment xml:lang="en">LanguaL curation note: Used for foods that have a coating or icing made from carob.</rdfs:comment>
        <rdfs:label xml:lang="en">carob coating or covering process</rdfs:label>
    </owl:Class>
    


    <!-- http://purl.obolibrary.org/obo/FOODON_03460358 -->

    <owl:Class rdf:about="http://purl.obolibrary.org/obo/FOODON_03460358">
        <rdfs:subClassOf rdf:resource="http://purl.obolibrary.org/obo/FOODON_03460178"/>
        <oboInOwl:hasDbXref rdf:datatype="http://www.w3.org/2001/XMLSchema#string">http://www.langual.org/langual_thesaurus.asp?termid=H0358</oboInOwl:hasDbXref>
        <oboInOwl:hasExactSynonym xml:lang="en">beating | whipping</oboInOwl:hasExactSynonym>
        <rdfs:comment xml:lang="en">LanguaL curation note: Used when foods or liquids (or a combination) are aerated by vigorously mixing them using a whip, whisk, spoon, spatula, rotary beater or electric mixer.</rdfs:comment>
        <rdfs:label xml:lang="en">food aeration by whipping</rdfs:label>
    </owl:Class>
    


    <!-- http://purl.obolibrary.org/obo/FOODON_03460359 -->

    <owl:Class rdf:about="http://purl.obolibrary.org/obo/FOODON_03460359">
        <rdfs:subClassOf rdf:resource="http://purl.obolibrary.org/obo/FOODON_03460178"/>
        <oboInOwl:hasDbXref rdf:datatype="http://www.w3.org/2001/XMLSchema#string">http://www.langual.org/langual_thesaurus.asp?termid=H0359</oboInOwl:hasDbXref>
        <oboInOwl:hasExactSynonym xml:lang="en">creaming</oboInOwl:hasExactSynonym>
        <rdfs:comment xml:lang="en">LanguaL curation note: Used when a solid fat (butter, margarine, shortening) is aerated to a creamy appearance, often with the addition of sugar.</rdfs:comment>
        <rdfs:label xml:lang="en">food aeration by creaming</rdfs:label>
    </owl:Class>
    


    <!-- http://purl.obolibrary.org/obo/FOODON_03460366 -->

    <owl:Class rdf:about="http://purl.obolibrary.org/obo/FOODON_03460366">
        <rdfs:subClassOf rdf:resource="http://purl.obolibrary.org/obo/FOODON_00002409"/>
        <oboInOwl:hasDbXref rdf:datatype="http://www.w3.org/2001/XMLSchema#string">http://www.langual.org/langual_thesaurus.asp?termid=H0366</oboInOwl:hasDbXref>
        <rdfs:comment xml:lang="en">LanguaL curation note: Used for any process such as rolling or pounding that is applied to dough, paste or meat (veal, chicken breast) in order to flatten the appearance.</rdfs:comment>
        <rdfs:label xml:lang="en">food flattening process</rdfs:label>
    </owl:Class>
    


    <!-- http://purl.obolibrary.org/obo/FOODON_03460391 -->

    <owl:Class rdf:about="http://purl.obolibrary.org/obo/FOODON_03460391">
        <rdfs:subClassOf rdf:resource="http://purl.obolibrary.org/obo/FOODON_03450005"/>
        <oboInOwl:hasDbXref rdf:datatype="http://www.w3.org/2001/XMLSchema#string">http://www.langual.org/langual_thesaurus.asp?termid=H0391</oboInOwl:hasDbXref>
        <rdfs:comment xml:lang="en">LanguaL curation note: Used primarily for processing of seeds, such as coffee, spices, nuts, and cacao beans.</rdfs:comment>
        <rdfs:label xml:lang="en">seed roasting</rdfs:label>
    </owl:Class>
    


    <!-- http://purl.obolibrary.org/obo/FOODON_03460393 -->

    <owl:Class rdf:about="http://purl.obolibrary.org/obo/FOODON_03460393">
        <rdfs:subClassOf rdf:resource="http://purl.obolibrary.org/obo/FOODON_03460238"/>
        <oboInOwl:hasDbXref rdf:datatype="http://www.w3.org/2001/XMLSchema#string">http://www.langual.org/langual_thesaurus.asp?termid=H0393</oboInOwl:hasDbXref>
        <rdfs:comment xml:lang="en">LanguaL curation note: Used when a juice, typically orange, has undergone a process specified in 21 CFR 146.148 to reduce the adicity of the food.</rdfs:comment>
        <rdfs:label xml:lang="en">acid reduction process</rdfs:label>
    </owl:Class>
    


    <!-- http://purl.obolibrary.org/obo/FOODON_03460396 -->

    <owl:Class rdf:about="http://purl.obolibrary.org/obo/FOODON_03460396">
        <rdfs:subClassOf rdf:resource="http://purl.obolibrary.org/obo/FOODON_03460123"/>
        <rdfs:subClassOf rdf:resource="http://purl.obolibrary.org/obo/FOODON_03460200"/>
        <oboInOwl:hasDbXref rdf:datatype="http://www.w3.org/2001/XMLSchema#string">http://www.langual.org/langual_thesaurus.asp?termid=H0396</oboInOwl:hasDbXref>
        <rdfs:comment xml:lang="en">LanguaL curation note: Used when a food such as meat, fish or vegetables are soaked in a seasoned liquid in order to absorb flavor and, in some instances, to be tenderized. Most marinades contain an acid (lemon juice, vinegar, wine) and herbs or spices; the acid ingredient serves as the tenderizer.</rdfs:comment>
        <rdfs:label xml:lang="en">marinading</rdfs:label>
    </owl:Class>
    


    <!-- http://purl.obolibrary.org/obo/FOODON_03460398 -->

    <owl:Class rdf:about="http://purl.obolibrary.org/obo/FOODON_03460398">
        <rdfs:subClassOf rdf:resource="http://purl.obolibrary.org/obo/FOODON_03460238"/>
        <oboInOwl:hasDbXref rdf:datatype="http://www.w3.org/2001/XMLSchema#string">http://www.langual.org/langual_thesaurus.asp?termid=H0398</oboInOwl:hasDbXref>
        <rdfs:comment xml:lang="en">LanguaL curation note: Used for food products (typically fruit, cheese or meat) that have had the rind removed.</rdfs:comment>
        <rdfs:label xml:lang="en">rind removal process</rdfs:label>
    </owl:Class>
    


    <!-- http://purl.obolibrary.org/obo/FOODON_03460750 -->

    <owl:Class rdf:about="http://purl.obolibrary.org/obo/FOODON_03460750">
        <rdfs:subClassOf rdf:resource="http://purl.obolibrary.org/obo/FOODON_03460134"/>
        <oboInOwl:hasDbXref rdf:datatype="http://www.w3.org/2001/XMLSchema#string">http://www.langual.org/langual_thesaurus.asp?termid=H0750</oboInOwl:hasDbXref>
        <rdfs:label xml:lang="en">gluten removal process</rdfs:label>
    </owl:Class>
    


    <!-- http://purl.obolibrary.org/obo/FOODON_03460751 -->

    <owl:Class rdf:about="http://purl.obolibrary.org/obo/FOODON_03460751">
        <rdfs:subClassOf rdf:resource="http://purl.obolibrary.org/obo/FOODON_03460225"/>
        <oboInOwl:hasDbXref rdf:datatype="http://www.w3.org/2001/XMLSchema#string">http://www.langual.org/langual_thesaurus.asp?termid=H0751</oboInOwl:hasDbXref>
        <rdfs:label xml:lang="en">leavening agent addition process</rdfs:label>
    </owl:Class>
    


    <!-- http://purl.obolibrary.org/obo/FOODON_03460752 -->

    <owl:Class rdf:about="http://purl.obolibrary.org/obo/FOODON_03460752">
        <rdfs:subClassOf rdf:resource="http://purl.obolibrary.org/obo/FOODON_03460751"/>
        <oboInOwl:hasDbXref rdf:datatype="http://www.w3.org/2001/XMLSchema#string">http://www.langual.org/langual_thesaurus.asp?termid=H0752</oboInOwl:hasDbXref>
        <rdfs:comment xml:lang="en">LanguaL curation note: If wheat sourdough was added use also *WHEAT ADDED [H0319]*. If rye sourdough was added use also *RYE ADDED [H0337]*.</rdfs:comment>
        <rdfs:label xml:lang="en">sourdough addition process</rdfs:label>
    </owl:Class>
    


    <!-- http://purl.obolibrary.org/obo/FOODON_03460753 -->

    <owl:Class rdf:about="http://purl.obolibrary.org/obo/FOODON_03460753">
        <rdfs:subClassOf rdf:resource="http://purl.obolibrary.org/obo/FOODON_03460751"/>
        <oboInOwl:hasDbXref rdf:datatype="http://www.w3.org/2001/XMLSchema#string">http://www.langual.org/langual_thesaurus.asp?termid=H0753</oboInOwl:hasDbXref>
        <rdfs:label xml:lang="en">yeast addition process</rdfs:label>
    </owl:Class>
    


    <!-- http://purl.obolibrary.org/obo/FOODON_03460760 -->

    <owl:Class rdf:about="http://purl.obolibrary.org/obo/FOODON_03460760">
        <rdfs:subClassOf rdf:resource="http://purl.obolibrary.org/obo/FOODON_03460141"/>
        <obo:IAO_0000115 xml:lang="en">Rendering is a process that converts waste animal tissue into stable, value-added materials. Rendering can refer to any processing of animal byproducts into more useful materials, or more narrowly to the rendering of whole animal fatty tissue into purified fats like lard or tallow. Rendering can be carried out on an industrial, farm, or kitchen scale.</obo:IAO_0000115>
        <oboInOwl:hasDbXref rdf:datatype="http://www.w3.org/2001/XMLSchema#string">http://www.langual.org/langual_thesaurus.asp?termid=H0760</oboInOwl:hasDbXref>
        <rdfs:label xml:lang="en">food animal rendering</rdfs:label>
    </owl:Class>
    


    <!-- http://purl.obolibrary.org/obo/FOODON_03460781 -->

    <owl:Class rdf:about="http://purl.obolibrary.org/obo/FOODON_03460781">
        <rdfs:subClassOf rdf:resource="http://purl.obolibrary.org/obo/FOODON_03460130"/>
        <obo:IAO_0000115 xml:lang="en">Micro-encapsulation is a process in which tiny particles or droplets are surrounded by a coating to give small capsules many useful properties. In a relatively simplistic form, a microcapsule is a small sphere with a uniform wall around it.</obo:IAO_0000115>
        <oboInOwl:hasDbXref rdf:datatype="http://www.w3.org/2001/XMLSchema#string">http://www.langual.org/langual_thesaurus.asp?termid=H0781</oboInOwl:hasDbXref>
        <oboInOwl:hasExactSynonym xml:lang="en">coating process | covering process | micro-encapsulation process</oboInOwl:hasExactSynonym>
        <rdfs:comment xml:lang="en">The material inside the microcapsule is referred to as the core, internal phase, or fill, whereas the wall is sometimes called a shell, coating, or membrane. Most microcapsules have diameters between a few micrometers and a few millimeters. The definition has been expanded, and includes most foods. Every class of food ingredient has been encapsulated; flavors are the most common. The technique of microencapsulation depends on the physical and chemical properties of the material to be encapsulated.[http://en.wikipedia.org/wiki/Micro-encapsulation]  LanguaL curation note: Used for the coating of microscopic particles with another material.</rdfs:comment>
        <rdfs:label xml:lang="en">food micro-encapsulation process</rdfs:label>
    </owl:Class>
    


    <!-- http://purl.obolibrary.org/obo/FOODON_03470100 -->

    <owl:Class rdf:about="http://purl.obolibrary.org/obo/FOODON_03470100">
        <rdfs:subClassOf rdf:resource="http://purl.obolibrary.org/obo/FOODON_03470109"/>
        <obo:IAO_0000115 xml:lang="en">Preservation by adding chemical preservatives (e.g., sorbic acid, sodium benzoate, BHT, calcium proprionate) to suppress or inhibit undesirable microorganisms or enzyme activity.</obo:IAO_0000115>
        <oboInOwl:hasDbXref rdf:datatype="http://www.w3.org/2001/XMLSchema#string">http://www.langual.org/langual_thesaurus.asp?termid=J0100</oboInOwl:hasDbXref>
        <rdfs:label xml:lang="en">preservation by adding chemicals</rdfs:label>
    </owl:Class>
    


    <!-- http://purl.obolibrary.org/obo/FOODON_03470102 -->

    <owl:Class rdf:about="http://purl.obolibrary.org/obo/FOODON_03470102">
        <rdfs:subClassOf rdf:resource="http://purl.obolibrary.org/obo/FOODON_03470123"/>
        <oboInOwl:hasDbXref rdf:datatype="http://www.w3.org/2001/XMLSchema#string">http://www.langual.org/langual_thesaurus.asp?termid=J0102</oboInOwl:hasDbXref>
        <rdfs:comment xml:lang="en">LanguaL curation note: Used when a food product is sterilized by holding at a high temperature before filling; the container may be sterilized before or after filling.</rdfs:comment>
        <rdfs:label xml:lang="en">food sterilization before filling</rdfs:label>
    </owl:Class>
    


    <!-- http://purl.obolibrary.org/obo/FOODON_03470103 -->

    <owl:Class rdf:about="http://purl.obolibrary.org/obo/FOODON_03470103">
        <rdfs:subClassOf rdf:resource="http://purl.obolibrary.org/obo/FOODON_03460130"/>
        <rdfs:subClassOf rdf:resource="http://purl.obolibrary.org/obo/FOODON_03470145"/>
        <rdfs:subClassOf rdf:resource="http://purl.obolibrary.org/obo/FOODON_03470154"/>
        <oboInOwl:hasDbXref rdf:datatype="http://www.w3.org/2001/XMLSchema#string">http://www.langual.org/langual_thesaurus.asp?termid=J0103</oboInOwl:hasDbXref>
        <rdfs:comment xml:lang="en">LanguaL curation note: Used when salting is used for preservation. The salt content of the food is generally 8% or higher (e.g. salted fish, etc.).</rdfs:comment>
        <rdfs:label xml:lang="en">food salting</rdfs:label>
    </owl:Class>
    


    <!-- http://purl.obolibrary.org/obo/FOODON_03470106 -->

    <owl:Class rdf:about="http://purl.obolibrary.org/obo/FOODON_03470106">
        <rdfs:subClassOf rdf:resource="http://purl.obolibrary.org/obo/FOODON_03460141"/>
        <rdfs:subClassOf rdf:resource="http://purl.obolibrary.org/obo/FOODON_03470145"/>
        <obo:IAO_0000115 xml:lang="en">Smoking is the process of flavoring, browning, cooking, or preserving food by exposing it to smoke from burning or smoldering material, most often wood.</obo:IAO_0000115>
        <obo:IAO_0000117 rdf:datatype="http://www.w3.org/2001/XMLSchema#string">Damion Dooley</obo:IAO_0000117>
        <oboInOwl:hasDbXref rdf:datatype="http://www.w3.org/2001/XMLSchema#string">http://www.langual.org/langual_thesaurus.asp?termid=J0106</oboInOwl:hasDbXref>
        <rdfs:comment xml:lang="en">In the past, smoking was a useful preservation tool, in combination with other techniques, most commonly salt-curing or drying. For some long-smoked foods, the smoking time also served to dry the food. Drying, curing, or other techniques can render the interior of foods inhospitable to bacterial life, while the smoking gives the vulnerable exterior surfaces an extra layer of protection. [Wikipedia]|LanguaL curation note: Used when smoking is used for preservation.</rdfs:comment>
        <rdfs:label xml:lang="en">food smoking</rdfs:label>
    </owl:Class>
    


    <!-- http://purl.obolibrary.org/obo/FOODON_03470107 -->

    <owl:Class rdf:about="http://purl.obolibrary.org/obo/FOODON_03470107">
        <rdfs:subClassOf rdf:resource="http://purl.obolibrary.org/obo/FOODON_00002451"/>
        <obo:IAO_0000115 xml:lang="en">The methods contributing to the prevention or retardation of microbial, enzymatic or oxidative spoilage and thus to the extension of shelf life. Index all methods for which information is available, even if a corresponding descriptor has already been used in *H. TREATMENT APPLIED*. Preservation descriptors refer to the finished food as a whole with these exceptions: (1) if the components of a multi-component food, such as cream pie, are preservation by different methods, index all methods; (2)  if chemical preservatives are declared on the label, always index them even if it is known that the preservative was introduced through or is only present in a component or ingredient of the food; and (3) if the preservation method for an ingredient is declared on the label (such as brie cheese made from pasteurized milk) index it. Also use *INGREDIENT preservation by THERMAL PROCESSING* or *INGREDIENT preservation by IRRADIATION* when ingredients have been pasteurized, ultrapasteurized, sterilized or irradiated.</obo:IAO_0000115>
        <oboInOwl:hasDbXref rdf:datatype="http://www.w3.org/2001/XMLSchema#string">http://www.langual.org/langual_thesaurus.asp?termid=J0107</oboInOwl:hasDbXref>
        <rdfs:comment xml:lang="en">LanguaL curation note: This term is for CLASSIFICATION ONLY; DO NOT USE term in indexing. Use a more precise narrower term.</rdfs:comment>
        <rdfs:label xml:lang="en">food preservation process</rdfs:label>
    </owl:Class>
    


    <!-- http://purl.obolibrary.org/obo/FOODON_03470108 -->

    <owl:Class rdf:about="http://purl.obolibrary.org/obo/FOODON_03470108">
        <rdfs:subClassOf rdf:resource="http://purl.obolibrary.org/obo/FOODON_03470109"/>
        <obo:IAO_0000115 xml:lang="en">Preservation by immersing in or spraying with liquids (e.g., sulfite solutions) or surrounding with gases (e.g., ethylene oxide, propylene oxide or sulfur dioxide) to destroy undesirable microorganisms or inactivate enzymes. Diffusion and chemical reaction may create a residue in the food product that contributes to continuing preservation.</obo:IAO_0000115>
        <oboInOwl:hasDbXref rdf:datatype="http://www.w3.org/2001/XMLSchema#string">http://www.langual.org/langual_thesaurus.asp?termid=J0108</oboInOwl:hasDbXref>
        <rdfs:label xml:lang="en">preservation by treatment with chemicals</rdfs:label>
    </owl:Class>
    


    <!-- http://purl.obolibrary.org/obo/FOODON_03470109 -->

    <owl:Class rdf:about="http://purl.obolibrary.org/obo/FOODON_03470109">
        <rdfs:subClassOf rdf:resource="http://purl.obolibrary.org/obo/FOODON_03470107"/>
        <obo:IAO_0000115 xml:lang="en">Preservation by use of chemical to destroy, suppress or inhibit undesirable microorganisms or enzyme activity.</obo:IAO_0000115>
        <oboInOwl:hasDbXref rdf:datatype="http://www.w3.org/2001/XMLSchema#string">http://www.langual.org/langual_thesaurus.asp?termid=J0109</oboInOwl:hasDbXref>
        <rdfs:label xml:lang="en">chemical food preservation process</rdfs:label>
    </owl:Class>
    


    <!-- http://purl.obolibrary.org/obo/FOODON_03470110 -->

    <owl:Class rdf:about="http://purl.obolibrary.org/obo/FOODON_03470110">
        <rdfs:subClassOf rdf:resource="http://purl.obolibrary.org/obo/FOODON_03470123"/>
        <oboInOwl:hasDbXref rdf:datatype="http://www.w3.org/2001/XMLSchema#string">http://www.langual.org/langual_thesaurus.asp?termid=J0110</oboInOwl:hasDbXref>
        <rdfs:comment xml:lang="en">LanguaL curation note: Used when a food product was sterilized by holding at a high temperature after filling.</rdfs:comment>
        <rdfs:label xml:lang="en">food sterilization after filling</rdfs:label>
    </owl:Class>
    


    <!-- http://purl.obolibrary.org/obo/FOODON_03470111 -->

    <owl:Class rdf:about="http://purl.obolibrary.org/obo/FOODON_03470111">
        <rdfs:subClassOf rdf:resource="http://purl.obolibrary.org/obo/FOODON_03470107"/>
        <obo:IAO_0000115 xml:lang="en">Preservation by storage in an atmosphere in which the concentrations of oxygen and carbon dioxide are different from those in air. This reduces microbial and enzymatic activity; often used commercially in conjunction with refrigeration (e.g., refrigerated rail cars) for fresh meat and produce.</obo:IAO_0000115>
        <oboInOwl:hasDbXref rdf:datatype="http://www.w3.org/2001/XMLSchema#string">http://www.langual.org/langual_thesaurus.asp?termid=J0111</oboInOwl:hasDbXref>
        <rdfs:label xml:lang="en">preservation by storage in modified atmosphere</rdfs:label>
    </owl:Class>
    


    <!-- http://purl.obolibrary.org/obo/FOODON_03470112 -->

    <owl:Class rdf:about="http://purl.obolibrary.org/obo/FOODON_03470112">
        <rdfs:subClassOf rdf:resource="http://purl.obolibrary.org/obo/FOODON_03470144"/>
        <oboInOwl:hasDbXref rdf:datatype="http://www.w3.org/2001/XMLSchema#string">http://www.langual.org/langual_thesaurus.asp?termid=J0112</oboInOwl:hasDbXref>
        <rdfs:comment xml:lang="en">LanguaL curation note: Used when the pressure is reduced to increase the efficiency of water removal.</rdfs:comment>
        <rdfs:label xml:lang="en">drying under reduced pressure</rdfs:label>
    </owl:Class>
    


    <!-- http://purl.obolibrary.org/obo/FOODON_03470113 -->

    <owl:Class rdf:about="http://purl.obolibrary.org/obo/FOODON_03470113">
        <rdfs:subClassOf rdf:resource="http://purl.obolibrary.org/obo/FOODON_03470122"/>
        <oboInOwl:hasDbXref rdf:datatype="http://www.w3.org/2001/XMLSchema#string">http://www.langual.org/langual_thesaurus.asp?termid=J0113</oboInOwl:hasDbXref>
        <rdfs:comment xml:lang="en">LanguaL curation note: Used for a food product that has been packed in a hermetically sealed container and rendered commercially sterile by ionizing radiation (e.g. 24-28 kGy).</rdfs:comment>
        <rdfs:label xml:lang="en">sterilization by irradiation</rdfs:label>
    </owl:Class>
    


    <!-- http://purl.obolibrary.org/obo/FOODON_03470114 -->

    <owl:Class rdf:about="http://purl.obolibrary.org/obo/FOODON_03470114">
        <rdfs:subClassOf rdf:resource="http://purl.obolibrary.org/obo/FOODON_03470102"/>
        <oboInOwl:hasDbXref rdf:datatype="http://www.w3.org/2001/XMLSchema#string">http://www.langual.org/langual_thesaurus.asp?termid=J0114</oboInOwl:hasDbXref>
        <rdfs:comment xml:lang="en">LanguaL curation note: Used when a sterile product is filled into a container at approximately 212 degrees F and cooled promptly after sealing.</rdfs:comment>
        <rdfs:label xml:lang="en">food sterilization by hot filling and cooling</rdfs:label>
    </owl:Class>
    


    <!-- http://purl.obolibrary.org/obo/FOODON_03470115 -->

    <owl:Class rdf:about="http://purl.obolibrary.org/obo/FOODON_03470115">
        <rdfs:subClassOf rdf:resource="http://purl.obolibrary.org/obo/FOODON_03470138"/>
        <oboInOwl:hasDbXref rdf:datatype="http://www.w3.org/2001/XMLSchema#string">http://www.langual.org/langual_thesaurus.asp?termid=J0115</oboInOwl:hasDbXref>
        <rdfs:comment xml:lang="en">LanguaL curation note: Used when sufficient ultraviolet radiation is applied to destroy most pathogenic and spoilage organisms present on the surface or to inhibit sprouting of stored agricultural produce and destroy storage pests. When followed by refrigeration, also index *preservation by CHILLING*.</rdfs:comment>
        <rdfs:label xml:lang="en">surface pasteurization or disinfection by ultraviolet irradiation</rdfs:label>
    </owl:Class>
    


    <!-- http://purl.obolibrary.org/obo/FOODON_03470116 -->

    <owl:Class rdf:about="http://purl.obolibrary.org/obo/FOODON_03470116">
        <rdfs:subClassOf rdf:resource="http://purl.obolibrary.org/obo/FOODON_00002419"/>
        <rdfs:subClassOf rdf:resource="http://purl.obolibrary.org/obo/FOODON_03470145"/>
        <oboInOwl:hasDbXref rdf:datatype="http://www.w3.org/2001/XMLSchema#string">http://www.langual.org/langual_thesaurus.asp?termid=J0116</oboInOwl:hasDbXref>
        <oboInOwl:hasExactSynonym xml:lang="en">dehydration | drying</oboInOwl:hasExactSynonym>
        <rdfs:comment xml:lang="en">LanguaL curation note: Used when the water activity has been lowered enough to achieve preservation. Also index *WATER REMOVED* in *H. TREATMENT APPLIED*.</rdfs:comment>
        <rdfs:label xml:lang="en">dehydration or drying</rdfs:label>
    </owl:Class>
    


    <!-- http://purl.obolibrary.org/obo/FOODON_03470117 -->

    <owl:Class rdf:about="http://purl.obolibrary.org/obo/FOODON_03470117">
        <rdfs:subClassOf rdf:resource="http://purl.obolibrary.org/obo/FOODON_03470116"/>
        <obo:IAO_0000115 xml:lang="en">Drying by heat.</obo:IAO_0000115>
        <oboInOwl:hasDbXref rdf:datatype="http://www.w3.org/2001/XMLSchema#string">http://www.langual.org/langual_thesaurus.asp?termid=J0117</oboInOwl:hasDbXref>
        <rdfs:label xml:lang="en">heat drying process</rdfs:label>
    </owl:Class>
    


    <!-- http://purl.obolibrary.org/obo/FOODON_03470119 -->

    <owl:Class rdf:about="http://purl.obolibrary.org/obo/FOODON_03470119">
        <rdfs:subClassOf rdf:resource="http://purl.obolibrary.org/obo/FOODON_03470122"/>
        <oboInOwl:hasDbXref rdf:datatype="http://www.w3.org/2001/XMLSchema#string">http://www.langual.org/langual_thesaurus.asp?termid=J0119</oboInOwl:hasDbXref>
        <rdfs:comment xml:lang="en">LanguaL curation note: Used when sufficient radiation (e.g. 10 kGy) is applied to destroy most patho-genic and food spoilage organisms. Also index *preservation by CHILLING*.</rdfs:comment>
        <rdfs:label xml:lang="en">pasteurization by irradiation</rdfs:label>
    </owl:Class>
    


    <!-- http://purl.obolibrary.org/obo/FOODON_03470120 -->

    <owl:Class rdf:about="http://purl.obolibrary.org/obo/FOODON_03470120">
        <rdfs:subClassOf rdf:resource="http://purl.obolibrary.org/obo/FOODON_03470107"/>
        <obo:IAO_0000115 xml:lang="en">Preservation by the use of high temperature for a time sufficient to reduce or destroy undesirable microorganisms and enzyme activity. [FDA CFSAN 1995]</obo:IAO_0000115>
        <oboInOwl:hasDbXref rdf:datatype="http://www.w3.org/2001/XMLSchema#string">http://www.langual.org/langual_thesaurus.asp?termid=J0120</oboInOwl:hasDbXref>
        <rdfs:label xml:lang="en">heat treatment food preservation</rdfs:label>
    </owl:Class>
    


    <!-- http://purl.obolibrary.org/obo/FOODON_03470121 -->

    <owl:Class rdf:about="http://purl.obolibrary.org/obo/FOODON_03470121">
        <rdfs:subClassOf rdf:resource="http://purl.obolibrary.org/obo/FOODON_03460238"/>
        <rdfs:subClassOf rdf:resource="http://purl.obolibrary.org/obo/FOODON_03470107"/>
        <obo:IAO_0000115 xml:lang="en">Preservation by filtering out yeasts and molds, generally followed by aseptic packaging. FDA CFSAN 1995</obo:IAO_0000115>
        <oboInOwl:hasDbXref rdf:datatype="http://www.w3.org/2001/XMLSchema#string">http://www.langual.org/langual_thesaurus.asp?termid=J0121</oboInOwl:hasDbXref>
        <rdfs:label xml:lang="en">food filtration</rdfs:label>
    </owl:Class>
    


    <!-- http://purl.obolibrary.org/obo/FOODON_03470122 -->

    <owl:Class rdf:about="http://purl.obolibrary.org/obo/FOODON_03470122">
        <rdfs:subClassOf rdf:resource="http://purl.obolibrary.org/obo/FOODON_03470138"/>
        <obo:IAO_0000115 xml:lang="en">Preservation by irradiation, primarily by gamma radiation.</obo:IAO_0000115>
        <oboInOwl:hasDbXref rdf:datatype="http://www.w3.org/2001/XMLSchema#string">http://www.langual.org/langual_thesaurus.asp?termid=J0122</oboInOwl:hasDbXref>
        <rdfs:label xml:lang="en">preservation by ionizing radiation</rdfs:label>
    </owl:Class>
    


    <!-- http://purl.obolibrary.org/obo/FOODON_03470123 -->

    <owl:Class rdf:about="http://purl.obolibrary.org/obo/FOODON_03470123">
        <rdfs:subClassOf rdf:resource="http://purl.obolibrary.org/obo/FOODON_03470120"/>
        <oboInOwl:hasDbXref rdf:datatype="http://www.w3.org/2001/XMLSchema#string">http://www.langual.org/langual_thesaurus.asp?termid=J0123</oboInOwl:hasDbXref>
        <oboInOwl:hasExactSynonym xml:lang="en">canning (sterilized and hermetically packed) | preservation by canning</oboInOwl:hasExactSynonym>
        <rdfs:comment xml:lang="en">LanguaL curation note: Used when the product is rendered commercially sterile by holding at high temperature before or after it is packed in a hermetically sealed container.</rdfs:comment>
        <rdfs:label xml:lang="en">food sterilization by heating</rdfs:label>
    </owl:Class>
    


    <!-- http://purl.obolibrary.org/obo/FOODON_03470124 -->

    <owl:Class rdf:about="http://purl.obolibrary.org/obo/FOODON_03470124">
        <rdfs:subClassOf rdf:resource="http://purl.obolibrary.org/obo/FOODON_03470116"/>
        <obo:IAO_0000115 xml:lang="en">Reduction of water in the product by osmosis.</obo:IAO_0000115>
        <oboInOwl:hasDbXref rdf:datatype="http://www.w3.org/2001/XMLSchema#string">http://www.langual.org/langual_thesaurus.asp?termid=J0124</oboInOwl:hasDbXref>
        <rdfs:label xml:lang="en">osmotic dehydration</rdfs:label>
    </owl:Class>
    


    <!-- http://purl.obolibrary.org/obo/FOODON_03470126 -->

    <owl:Class rdf:about="http://purl.obolibrary.org/obo/FOODON_03470126">
        <rdfs:subClassOf rdf:resource="http://purl.obolibrary.org/obo/FOODON_03470102"/>
        <oboInOwl:hasDbXref rdf:datatype="http://www.w3.org/2001/XMLSchema#string">http://www.langual.org/langual_thesaurus.asp?termid=J0126</oboInOwl:hasDbXref>
        <rdfs:comment xml:lang="en">LanguaL curation note: Used when a sterile product is filled in a sterile atmosphere into a sterile container. For further detail see 21 CFR 113.3(a).</rdfs:comment>
        <rdfs:label xml:lang="en">aseptic filling and sealing of food</rdfs:label>
    </owl:Class>
    


    <!-- http://purl.obolibrary.org/obo/FOODON_03470128 -->

    <owl:Class rdf:about="http://purl.obolibrary.org/obo/FOODON_03470128">
        <rdfs:subClassOf rdf:resource="http://purl.obolibrary.org/obo/FOODON_03470136"/>
        <oboInOwl:hasDbXref rdf:datatype="http://www.w3.org/2001/XMLSchema#string">http://www.langual.org/langual_thesaurus.asp?termid=J0128</oboInOwl:hasDbXref>
        <oboInOwl:hasExactSynonym xml:lang="en">quiescent freezing | sharp freezing | slush freezing</oboInOwl:hasExactSynonym>
        <rdfs:label xml:lang="en">food slow freezing</rdfs:label>
    </owl:Class>
    


    <!-- http://purl.obolibrary.org/obo/FOODON_03470129 -->

    <owl:Class rdf:about="http://purl.obolibrary.org/obo/FOODON_03470129">
        <rdfs:subClassOf rdf:resource="http://purl.obolibrary.org/obo/FOODON_03470102"/>
        <oboInOwl:hasDbXref rdf:datatype="http://www.w3.org/2001/XMLSchema#string">http://www.langual.org/langual_thesaurus.asp?termid=J0129</oboInOwl:hasDbXref>
        <rdfs:comment xml:lang="en">LanguaL curation note: Used when a sterile product is filled into a container at approximately 212 degrees F., sealed, and held hot temporarily to complete processing before cooling.</rdfs:comment>
        <rdfs:label xml:lang="en">food sterilization by hot filling, held hot and cooling</rdfs:label>
    </owl:Class>
    


    <!-- http://purl.obolibrary.org/obo/FOODON_03470130 -->

    <owl:Class rdf:about="http://purl.obolibrary.org/obo/FOODON_03470130">
        <rdfs:subClassOf rdf:resource="http://purl.obolibrary.org/obo/FOODON_03470112"/>
        <obo:IAO_0000115 xml:lang="en">Dehydration by sublimation under reduced pressure while frozen. Usually the product is not stored frozen.</obo:IAO_0000115>
        <oboInOwl:hasDbXref rdf:datatype="http://www.w3.org/2001/XMLSchema#string">http://www.langual.org/langual_thesaurus.asp?termid=J0130</oboInOwl:hasDbXref>
        <rdfs:label xml:lang="en">freeze-drying</rdfs:label>
    </owl:Class>
    


    <!-- http://purl.obolibrary.org/obo/FOODON_03470131 -->

    <owl:Class rdf:about="http://purl.obolibrary.org/obo/FOODON_03470131">
        <rdfs:subClassOf rdf:resource="http://purl.obolibrary.org/obo/FOODON_03470107"/>
        <obo:IAO_0000115 xml:lang="en">Cooling and keeping at a temperature between 30°F and 45°F (-1°C and 7°C). Regarding food preservation regulations, the temperature range depends on national legislation.</obo:IAO_0000115>
        <oboInOwl:hasDbXref rdf:datatype="http://www.w3.org/2001/XMLSchema#string">http://www.langual.org/langual_thesaurus.asp?termid=J0131</oboInOwl:hasDbXref>
        <oboInOwl:hasExactSynonym xml:lang="en">preservation by storage in refrigeration | refrigeration</oboInOwl:hasExactSynonym>
        <rdfs:comment xml:lang="en">LanguaL curation note: Preservation methods that imply subsequent chilling are: *PASTEURIZED BY IRRADIATION*, *PASTEURIZED BY HEAT*, *preservation by CHEMICALS *, *preservation by FERMENTATION*, *SURFACE PASTEURIZED BY ULTRAVIOLET*, *preservation by STORAGE IN MODIFIED ATMOSPHERE*, *preservation by FILTRATION*.</rdfs:comment>
        <rdfs:label xml:lang="en">food chilling</rdfs:label>
    </owl:Class>
    


    <!-- http://purl.obolibrary.org/obo/FOODON_03470132 -->

    <owl:Class rdf:about="http://purl.obolibrary.org/obo/FOODON_03470132">
        <rdfs:subClassOf rdf:resource="http://purl.obolibrary.org/obo/FOODON_03470136"/>
        <oboInOwl:hasDbXref rdf:datatype="http://www.w3.org/2001/XMLSchema#string">http://www.langual.org/langual_thesaurus.asp?termid=J0132</oboInOwl:hasDbXref>
        <rdfs:label xml:lang="en">food quick freezing</rdfs:label>
    </owl:Class>
    


    <!-- http://purl.obolibrary.org/obo/FOODON_03470133 -->

    <owl:Class rdf:about="http://purl.obolibrary.org/obo/FOODON_03470133">
        <rdfs:subClassOf rdf:resource="http://purl.obolibrary.org/obo/FOODON_03470144"/>
        <oboInOwl:hasDbXref rdf:datatype="http://www.w3.org/2001/XMLSchema#string">http://www.langual.org/langual_thesaurus.asp?termid=J0133</oboInOwl:hasDbXref>
        <rdfs:comment xml:lang="en">LanguaL curation note: Used when liquids and low-viscosity pastes or purees are dried by atomisation. Example: milk.</rdfs:comment>
        <rdfs:label xml:lang="en">spray-drying</rdfs:label>
    </owl:Class>
    


    <!-- http://purl.obolibrary.org/obo/FOODON_03470134 -->

    <owl:Class rdf:about="http://purl.obolibrary.org/obo/FOODON_03470134">
        <rdfs:subClassOf rdf:resource="http://purl.obolibrary.org/obo/FOODON_03470143"/>
        <oboInOwl:hasDbXref rdf:datatype="http://www.w3.org/2001/XMLSchema#string">http://www.langual.org/langual_thesaurus.asp?termid=J0134</oboInOwl:hasDbXref>
        <rdfs:comment xml:lang="en">LanguaL curation note: Used when water is removed from products placed in trays on shelves under atmospheric pressure. Example: vegetables, fruits.</rdfs:comment>
        <rdfs:label xml:lang="en">shelf-drying under normal pressure</rdfs:label>
    </owl:Class>
    


    <!-- http://purl.obolibrary.org/obo/FOODON_03470135 -->

    <owl:Class rdf:about="http://purl.obolibrary.org/obo/FOODON_03470135">
        <rdfs:subClassOf rdf:resource="http://purl.obolibrary.org/obo/FOODON_03470120"/>
        <oboInOwl:hasDbXref rdf:datatype="http://www.w3.org/2001/XMLSchema#string">http://www.langual.org/langual_thesaurus.asp?termid=J0135</oboInOwl:hasDbXref>
        <rdfs:comment xml:lang="en">LanguaL curation note: Used when the product is held at a temperature of 60-150 °C (140-300 °F) for a time sufficient to destroy most pathogenic and food spoilage organisms. When followed by refrigeration, also index *preservation by CHILLING*.</rdfs:comment>
        <rdfs:label xml:lang="en">pasteurization by heating</rdfs:label>
    </owl:Class>
    


    <!-- http://purl.obolibrary.org/obo/FOODON_03470136 -->

    <owl:Class rdf:about="http://purl.obolibrary.org/obo/FOODON_03470136">
        <rdfs:subClassOf rdf:resource="http://purl.obolibrary.org/obo/FOODON_03470107"/>
        <obo:IAO_0000115 xml:lang="en">Preservation by freezing a food product and keeping it at a temperature below the freezing point (20-30 degrees F) without regard to the product&apos;s physical state.</obo:IAO_0000115>
        <oboInOwl:hasDbXref rdf:datatype="http://www.w3.org/2001/XMLSchema#string">http://www.langual.org/langual_thesaurus.asp?termid=J0136</oboInOwl:hasDbXref>
        <oboInOwl:hasExactSynonym xml:lang="en">freezing</oboInOwl:hasExactSynonym>
        <rdfs:label xml:lang="en">food freezing</rdfs:label>
    </owl:Class>
    


    <!-- http://purl.obolibrary.org/obo/FOODON_03470137 -->

    <owl:Class rdf:about="http://purl.obolibrary.org/obo/FOODON_03470137">
        <rdfs:subClassOf rdf:resource="http://purl.obolibrary.org/obo/FOODON_03470103"/>
        <obo:IAO_0000115 xml:lang="en">Immersed in a salt brine strong enough to suppress enzyme activity and growth of undesirable organisms.</obo:IAO_0000115>
        <obo:IAO_0000119 rdf:datatype="http://www.w3.org/2001/XMLSchema#string">https://en.wikipedia.org/wiki/Brining</obo:IAO_0000119>
        <oboInOwl:hasDbXref rdf:datatype="http://www.w3.org/2001/XMLSchema#string">http://www.langual.org/langual_thesaurus.asp?termid=J0137</oboInOwl:hasDbXref>
        <oboInOwl:hasExactSynonym xml:lang="en">brining | corning</oboInOwl:hasExactSynonym>
        <rdfs:label xml:lang="en">food brining</rdfs:label>
    </owl:Class>
    


    <!-- http://purl.obolibrary.org/obo/FOODON_03470138 -->

    <owl:Class rdf:about="http://purl.obolibrary.org/obo/FOODON_03470138">
        <rdfs:subClassOf rdf:resource="http://purl.obolibrary.org/obo/FOODON_03470107"/>
        <obo:IAO_0000115 xml:lang="en">Preservation by the use of radiation to destroy or suppress undesirable microorganisms or enzyme activity.</obo:IAO_0000115>
        <oboInOwl:hasDbXref rdf:datatype="http://www.w3.org/2001/XMLSchema#string">http://www.langual.org/langual_thesaurus.asp?termid=J0138</oboInOwl:hasDbXref>
        <rdfs:label xml:lang="en">preservation by irradiation</rdfs:label>
    </owl:Class>
    


    <!-- http://purl.obolibrary.org/obo/FOODON_03470139 -->

    <owl:Class rdf:about="http://purl.obolibrary.org/obo/FOODON_03470139">
        <rdfs:subClassOf rdf:resource="http://purl.obolibrary.org/obo/FOODON_03470103"/>
        <obo:IAO_0000115 xml:lang="en">Packed in dry salt in sufficient quantity to suppress enzyme activity or growth of undesirable organisms.</obo:IAO_0000115>
        <oboInOwl:hasDbXref rdf:datatype="http://www.w3.org/2001/XMLSchema#string">http://www.langual.org/langual_thesaurus.asp?termid=J0139</oboInOwl:hasDbXref>
        <oboInOwl:hasExactSynonym xml:lang="en">dry salted</oboInOwl:hasExactSynonym>
        <rdfs:label xml:lang="en">food dry salting</rdfs:label>
    </owl:Class>
    


    <!-- http://purl.obolibrary.org/obo/FOODON_03470140 -->

    <owl:Class rdf:about="http://purl.obolibrary.org/obo/FOODON_03470140">
        <rdfs:subClassOf rdf:resource="http://purl.obolibrary.org/obo/FOODON_03470143"/>
        <oboInOwl:hasDbXref rdf:datatype="http://www.w3.org/2001/XMLSchema#string">http://www.langual.org/langual_thesaurus.asp?termid=J0140</oboInOwl:hasDbXref>
        <rdfs:label xml:lang="en">drum-drying</rdfs:label>
    </owl:Class>
    


    <!-- http://purl.obolibrary.org/obo/FOODON_03470141 -->

    <owl:Class rdf:about="http://purl.obolibrary.org/obo/FOODON_03470141">
        <rdfs:subClassOf rdf:resource="http://purl.obolibrary.org/obo/FOODON_03470117"/>
        <obo:IAO_0000115 xml:lang="en">Dried by natural heat, usually through exposure to the sun. Includes field-dried products such as grains and dry beans. These products are included also if they have been artificially dried to return them to normal dry state, e.g. grain that has been artificially dried after harvest.</obo:IAO_0000115>
        <oboInOwl:hasDbXref rdf:datatype="http://www.w3.org/2001/XMLSchema#string">http://www.langual.org/langual_thesaurus.asp?termid=J0141</oboInOwl:hasDbXref>
        <oboInOwl:hasExactSynonym xml:lang="en">field drying | sun drying</oboInOwl:hasExactSynonym>
        <rdfs:label xml:lang="en">natural heat drying</rdfs:label>
    </owl:Class>
    


    <!-- http://purl.obolibrary.org/obo/FOODON_03470142 -->

    <owl:Class rdf:about="http://purl.obolibrary.org/obo/FOODON_03470142">
        <owl:equivalentClass>
            <owl:Class>
                <owl:unionOf rdf:parseType="Collection">
                    <rdf:Description rdf:about="http://purl.obolibrary.org/obo/FOODON_03470131"/>
                    <rdf:Description rdf:about="http://purl.obolibrary.org/obo/FOODON_03470136"/>
                </owl:unionOf>
            </owl:Class>
        </owl:equivalentClass>
        <rdfs:subClassOf rdf:resource="http://purl.obolibrary.org/obo/FOODON_03470107"/>
        <obo:IAO_0000115 xml:lang="en">Preservation by cooling and storage at low temperature (chilling at around 0-5°C (32 to 41°F), freezing at -18°C (0°F))  to prevent or retard microbial or enzymatic spoilage.</obo:IAO_0000115>
        <oboInOwl:hasDbXref rdf:datatype="http://www.w3.org/2001/XMLSchema#string">http://www.langual.org/langual_thesaurus.asp?termid=J0142</oboInOwl:hasDbXref>
        <oboInOwl:hasExactSynonym xml:lang="en">preservation by refrigeration</oboInOwl:hasExactSynonym>
        <rdfs:comment xml:lang="en">LanguaL curation note: In order to comply with labelling requirements, it must be specified if it is chilling or freezing.</rdfs:comment>
        <rdfs:label xml:lang="en">chilling or freezing</rdfs:label>
    </owl:Class>
    


    <!-- http://purl.obolibrary.org/obo/FOODON_03470143 -->

    <owl:Class rdf:about="http://purl.obolibrary.org/obo/FOODON_03470143">
        <rdfs:subClassOf rdf:resource="http://purl.obolibrary.org/obo/FOODON_03470144"/>
        <oboInOwl:hasDbXref rdf:datatype="http://www.w3.org/2001/XMLSchema#string">http://www.langual.org/langual_thesaurus.asp?termid=J0143</oboInOwl:hasDbXref>
        <rdfs:label xml:lang="en">drying under normal pressure</rdfs:label>
    </owl:Class>
    


    <!-- http://purl.obolibrary.org/obo/FOODON_03470144 -->

    <owl:Class rdf:about="http://purl.obolibrary.org/obo/FOODON_03470144">
        <rdfs:subClassOf rdf:resource="http://purl.obolibrary.org/obo/FOODON_03470117"/>
        <obo:IAO_0000115 xml:lang="en">Drying by the application of artificial heat.</obo:IAO_0000115>
        <oboInOwl:hasDbXref rdf:datatype="http://www.w3.org/2001/XMLSchema#string">http://www.langual.org/langual_thesaurus.asp?termid=J0144</oboInOwl:hasDbXref>
        <rdfs:label xml:lang="en">artificial heat drying</rdfs:label>
    </owl:Class>
    


    <!-- http://purl.obolibrary.org/obo/FOODON_03470145 -->

    <owl:Class rdf:about="http://purl.obolibrary.org/obo/FOODON_03470145">
        <rdfs:subClassOf rdf:resource="http://purl.obolibrary.org/obo/FOODON_03470107"/>
        <obo:IAO_0000115 xml:lang="en">Preservation method that lowers the water activity (relative humidity) of a food product. This is accomplished by using mechanical dehydration equipment, by natural drying, by adding salt, sugar or other agents to the food or by surface drying during a refrigeration or freezing operation. This method of preservation may be used in conjunction with other preservation methods such as preservation by thermal processing.</obo:IAO_0000115>
        <oboInOwl:hasDbXref rdf:datatype="http://www.w3.org/2001/XMLSchema#string">http://www.langual.org/langual_thesaurus.asp?termid=J0145</oboInOwl:hasDbXref>
        <rdfs:label xml:lang="en">preservation by reducing water activity</rdfs:label>
    </owl:Class>
    


    <!-- http://purl.obolibrary.org/obo/FOODON_03470146 -->

    <owl:Class rdf:about="http://purl.obolibrary.org/obo/FOODON_03470146">
        <rdfs:subClassOf rdf:resource="http://purl.obolibrary.org/obo/FOODON_03470145"/>
        <obo:IAO_0000115 xml:lang="en">Preservation by adding sugar, sugar syrup or by partial inversion of disaccharides until the sugar concentration is high enough to prevent growth of microorganisms.</obo:IAO_0000115>
        <oboInOwl:hasDbXref rdf:datatype="http://www.w3.org/2001/XMLSchema#string">http://www.langual.org/langual_thesaurus.asp?termid=J0146</oboInOwl:hasDbXref>
        <rdfs:label xml:lang="en">preservation by adding sugar</rdfs:label>
    </owl:Class>
    


    <!-- http://purl.obolibrary.org/obo/FOODON_03470147 -->

    <owl:Class rdf:about="http://purl.obolibrary.org/obo/FOODON_03470147">
        <rdfs:subClassOf rdf:resource="http://purl.obolibrary.org/obo/FOODON_03470126"/>
        <oboInOwl:hasDbXref rdf:datatype="http://www.w3.org/2001/XMLSchema#string">http://www.langual.org/langual_thesaurus.asp?termid=J0147</oboInOwl:hasDbXref>
        <oboInOwl:hasExactSynonym xml:lang="en">UHT sterilized</oboInOwl:hasExactSynonym>
        <rdfs:label xml:lang="en">food sterilization at ultra high temperature (UHT)</rdfs:label>
    </owl:Class>
    


    <!-- http://purl.obolibrary.org/obo/FOODON_03470148 -->

    <owl:Class rdf:about="http://purl.obolibrary.org/obo/FOODON_03470148">
        <rdfs:subClassOf rdf:resource="http://purl.obolibrary.org/obo/FOODON_03470135"/>
        <obo:IAO_0000115 xml:lang="en">When used to describe a dairy product, means that such product shall have been thermally processed at or above 138° C (280° C) for at least 2 seconds, either before or after packaging so as to produce a product that has extended shelf life under refrigerated conditions (21 CFR 131.3 (c)). Used to describe liquid egg products that also have been thermally processed, but at a different temperature than for milk products.  The egg product will have an extended shelf life under refrigerated conditions.</obo:IAO_0000115>
        <oboInOwl:hasDbXref rdf:datatype="http://www.w3.org/2001/XMLSchema#string">http://www.langual.org/langual_thesaurus.asp?termid=J0148</oboInOwl:hasDbXref>
        <rdfs:label xml:lang="en">ultra pasteurization (UP) by heat</rdfs:label>
    </owl:Class>
    


    <!-- http://purl.obolibrary.org/obo/FOODON_03470149 -->

    <owl:Class rdf:about="http://purl.obolibrary.org/obo/FOODON_03470149">
        <rdfs:subClassOf rdf:resource="http://purl.obolibrary.org/obo/FOODON_03470100"/>
        <oboInOwl:hasDbXref rdf:datatype="http://www.w3.org/2001/XMLSchema#string">http://www.langual.org/langual_thesaurus.asp?termid=J0149</oboInOwl:hasDbXref>
        <rdfs:label xml:lang="en">preservation by adding acid</rdfs:label>
    </owl:Class>
    


    <!-- http://purl.obolibrary.org/obo/FOODON_03470150 -->

    <owl:Class rdf:about="http://purl.obolibrary.org/obo/FOODON_03470150">
        <rdfs:subClassOf rdf:resource="http://purl.obolibrary.org/obo/FOODON_03450002"/>
        <obo:IAO_0000115 xml:lang="en">Sous-vide, French for &quot;under vacuum&quot;, is a method of cooking that is intended to maintain the integrity of ingredients by heating them for an extended period of time in vacuum sealed plastic pouches at relatively low temperatures. Food is cooked for a long time, sometimes well over 24 hours. Unlike cooking in a slow cooker, sous-vide cooking uses airtight plastic bags placed in hot water well below boiling point (usually around 60°C or 140°F).</obo:IAO_0000115>
        <oboInOwl:hasDbXref rdf:datatype="http://www.w3.org/2001/XMLSchema#string">http://www.langual.org/langual_thesaurus.asp?termid=J0150</oboInOwl:hasDbXref>
        <oboInOwl:hasExactSynonym xml:lang="en">sous vide</oboInOwl:hasExactSynonym>
        <rdfs:label xml:lang="en">sous vide cooking</rdfs:label>
    </owl:Class>
    


    <!-- http://purl.obolibrary.org/obo/FOODON_03470151 -->

    <owl:Class rdf:about="http://purl.obolibrary.org/obo/FOODON_03470151">
        <rdfs:subClassOf rdf:resource="http://purl.obolibrary.org/obo/FOODON_03470120"/>
        <oboInOwl:hasDbXref rdf:datatype="http://www.w3.org/2001/XMLSchema#string">http://www.langual.org/langual_thesaurus.asp?termid=J0151</oboInOwl:hasDbXref>
        <rdfs:comment xml:lang="en">LanguaL curation note: Used when an ingredient or a component of a food has been subjected to preservation by pasteurization, ultrapasteurization or sterilization.</rdfs:comment>
        <rdfs:label xml:lang="en">preservation of food component by heat treatment</rdfs:label>
    </owl:Class>
    


    <!-- http://purl.obolibrary.org/obo/FOODON_03470152 -->

    <owl:Class rdf:about="http://purl.obolibrary.org/obo/FOODON_03470152">
        <rdfs:subClassOf rdf:resource="http://purl.obolibrary.org/obo/FOODON_03470138"/>
        <oboInOwl:hasDbXref rdf:datatype="http://www.w3.org/2001/XMLSchema#string">http://www.langual.org/langual_thesaurus.asp?termid=J0152</oboInOwl:hasDbXref>
        <rdfs:comment xml:lang="en">LanguaL curation note: Used when an ingredient or a component of a food has been preservation by irradiation.</rdfs:comment>
        <rdfs:label xml:lang="en">ingredient preservation by irradiation</rdfs:label>
    </owl:Class>
    


    <!-- http://purl.obolibrary.org/obo/FOODON_03470153 -->

    <owl:Class rdf:about="http://purl.obolibrary.org/obo/FOODON_03470153">
        <rdfs:subClassOf rdf:resource="http://purl.obolibrary.org/obo/FOODON_03470107"/>
        <obo:IAO_0000115 xml:lang="en">Preservation by adding spices or extracts (e.g. garlic, onion, horseradish, paprika) to suppress or inhibit undesirable micro-organisms, enzyme activity, or oxidative changes.</obo:IAO_0000115>
        <oboInOwl:hasDbXref rdf:datatype="http://www.w3.org/2001/XMLSchema#string">http://www.langual.org/langual_thesaurus.asp?termid=J0153</oboInOwl:hasDbXref>
        <rdfs:label xml:lang="en">preservation by adding spices or extracts</rdfs:label>
    </owl:Class>
    


    <!-- http://purl.obolibrary.org/obo/FOODON_03470154 -->

    <owl:Class rdf:about="http://purl.obolibrary.org/obo/FOODON_03470154">
        <rdfs:subClassOf rdf:resource="http://purl.obolibrary.org/obo/FOODON_03470149"/>
        <obo:IAO_0000115 xml:lang="en">Preservation by adding inorganic acids or salts (e.g. SO2, H2SO4, KNO4, NaNO3) to suppress or inhibit undesirable micro-organisms or enzyme activity.</obo:IAO_0000115>
        <oboInOwl:hasDbXref rdf:datatype="http://www.w3.org/2001/XMLSchema#string">http://www.langual.org/langual_thesaurus.asp?termid=J0154</oboInOwl:hasDbXref>
        <rdfs:label xml:lang="en">preservation by adding inorganic acids or salts</rdfs:label>
    </owl:Class>
    


    <!-- http://purl.obolibrary.org/obo/FOODON_03470155 -->

    <owl:Class rdf:about="http://purl.obolibrary.org/obo/FOODON_03470155">
        <rdfs:subClassOf rdf:resource="http://purl.obolibrary.org/obo/FOODON_03470149"/>
        <obo:IAO_0000115 xml:lang="en">Preservation by adding organic acids or salts (e.g. lactic acid, acetic acid, salicylic acid) to suppress or inhibit undesirable micro organisms or enzyme activity.</obo:IAO_0000115>
        <oboInOwl:hasDbXref rdf:datatype="http://www.w3.org/2001/XMLSchema#string">http://www.langual.org/langual_thesaurus.asp?termid=J0155</oboInOwl:hasDbXref>
        <rdfs:label xml:lang="en">preservation by adding organic acids or salts</rdfs:label>
    </owl:Class>
    


    <!-- http://purl.obolibrary.org/obo/FOODON_03470156 -->

    <owl:Class rdf:about="http://purl.obolibrary.org/obo/FOODON_03470156">
        <rdfs:subClassOf rdf:resource="http://purl.obolibrary.org/obo/FOODON_03470100"/>
        <obo:IAO_0000115 xml:lang="en">Preservation by adding antibiotics (e.g. nisin, tylosine, subtlin, bacitracin, chlorotetracyclin, oxytetracyclin) to kill micro organisms or stop their growth.</obo:IAO_0000115>
        <oboInOwl:hasDbXref rdf:datatype="http://www.w3.org/2001/XMLSchema#string">http://www.langual.org/langual_thesaurus.asp?termid=J0156</oboInOwl:hasDbXref>
        <rdfs:label xml:lang="en">preservation by adding antibiotics</rdfs:label>
    </owl:Class>
    


    <!-- http://purl.obolibrary.org/obo/FOODON_03470157 -->

    <owl:Class rdf:about="http://purl.obolibrary.org/obo/FOODON_03470157">
        <rdfs:subClassOf rdf:resource="http://purl.obolibrary.org/obo/FOODON_03470121"/>
        <obo:IAO_0000115 xml:lang="en">Separation of colloidal or very fine solid materials by filtration through microporous or semipermeable mediums. Membranes have pores in the range 2-20 nm diameter.</obo:IAO_0000115>
        <oboInOwl:hasDbXref rdf:datatype="http://www.w3.org/2001/XMLSchema#string">http://www.langual.org/langual_thesaurus.asp?termid=J0157</oboInOwl:hasDbXref>
        <rdfs:comment xml:lang="en">Some dairy product are ultrafiltrated in order to obtain a higher protein concentration and hereby, a thicker consistency or textture. LanguaL curation note: Used when a product is preservation by the use of ultra-filtration to remove undesirable micro organisms and molecules. Example: beer.</rdfs:comment>
        <rdfs:label xml:lang="en">food ultra-filtration</rdfs:label>
    </owl:Class>
    


    <!-- http://purl.obolibrary.org/obo/FOODON_03470158 -->

    <owl:Class rdf:about="http://purl.obolibrary.org/obo/FOODON_03470158">
        <rdfs:subClassOf rdf:resource="http://purl.obolibrary.org/obo/FOODON_03470181"/>
        <oboInOwl:hasDbXref rdf:datatype="http://www.w3.org/2001/XMLSchema#string">http://www.langual.org/langual_thesaurus.asp?termid=J0158</oboInOwl:hasDbXref>
        <rdfs:label xml:lang="en">pasteurization by heat after filling</rdfs:label>
    </owl:Class>
    


    <!-- http://purl.obolibrary.org/obo/FOODON_03470159 -->

    <owl:Class rdf:about="http://purl.obolibrary.org/obo/FOODON_03470159">
        <rdfs:subClassOf rdf:resource="http://purl.obolibrary.org/obo/FOODON_03470181"/>
        <oboInOwl:hasDbXref rdf:datatype="http://www.w3.org/2001/XMLSchema#string">http://www.langual.org/langual_thesaurus.asp?termid=J0159</oboInOwl:hasDbXref>
        <rdfs:label xml:lang="en">pasteurization by heat before filling</rdfs:label>
    </owl:Class>
    


    <!-- http://purl.obolibrary.org/obo/FOODON_03470160 -->

    <owl:Class rdf:about="http://purl.obolibrary.org/obo/FOODON_03470160">
        <rdfs:subClassOf rdf:resource="http://purl.obolibrary.org/obo/FOODON_03470107"/>
        <obo:IAO_0000115 xml:lang="en">The process of holding food at a high pressure, normally greater than 1000 bar, which leads to sterilization. Example: Fruit juice, jam.</obo:IAO_0000115>
        <obo:IAO_0000117 rdf:datatype="http://www.w3.org/2001/XMLSchema#string">Damion Dooley</obo:IAO_0000117>
        <oboInOwl:hasDbXref rdf:datatype="http://www.w3.org/2001/XMLSchema#string">http://www.langual.org/langual_thesaurus.asp?termid=J0160</oboInOwl:hasDbXref>
        <rdfs:label xml:lang="en">ultra high pressure sterilization</rdfs:label>
    </owl:Class>
    


    <!-- http://purl.obolibrary.org/obo/FOODON_03470161 -->

    <owl:Class rdf:about="http://purl.obolibrary.org/obo/FOODON_03470161">
        <rdfs:subClassOf rdf:resource="http://purl.obolibrary.org/obo/FOODON_03470138"/>
        <obo:IAO_0000115 xml:lang="en">Treated by electron accelerator radiation, for example to kill insects in cereals.</obo:IAO_0000115>
        <oboInOwl:hasDbXref rdf:datatype="http://www.w3.org/2001/XMLSchema#string">http://www.langual.org/langual_thesaurus.asp?termid=J0161</oboInOwl:hasDbXref>
        <rdfs:label xml:lang="en">preservation by electron accelerator radiation</rdfs:label>
    </owl:Class>
    


    <!-- http://purl.obolibrary.org/obo/FOODON_03470162 -->

    <owl:Class rdf:about="http://purl.obolibrary.org/obo/FOODON_03470162">
        <rdfs:subClassOf rdf:resource="http://purl.obolibrary.org/obo/FOODON_03470122"/>
        <oboInOwl:hasDbXref rdf:datatype="http://www.w3.org/2001/XMLSchema#string">http://www.langual.org/langual_thesaurus.asp?termid=J0162</oboInOwl:hasDbXref>
        <rdfs:comment xml:lang="en">LanguaL curation note: Used when sufficient radiation (e.g. 1-5 k gy) is applied to destroy pathogenic and food spoilage organisms. Example: spices. Radurised food should be stored in a cool and dry place.</rdfs:comment>
        <rdfs:label xml:lang="en">disinfection by irradiation</rdfs:label>
    </owl:Class>
    


    <!-- http://purl.obolibrary.org/obo/FOODON_03470163 -->

    <owl:Class rdf:about="http://purl.obolibrary.org/obo/FOODON_03470163">
        <rdfs:subClassOf rdf:resource="http://purl.obolibrary.org/obo/FOODON_03470116"/>
        <oboInOwl:hasDbXref rdf:datatype="http://www.w3.org/2001/XMLSchema#string">http://www.langual.org/langual_thesaurus.asp?termid=J0163</oboInOwl:hasDbXref>
        <rdfs:comment xml:lang="en">LanguaL curation note: Used when the water activity is lowered enough by high frequency heating in order to achieve preservation.</rdfs:comment>
        <rdfs:label xml:lang="en">drying by radiation</rdfs:label>
    </owl:Class>
    


    <!-- http://purl.obolibrary.org/obo/FOODON_03470165 -->

    <owl:Class rdf:about="http://purl.obolibrary.org/obo/FOODON_03470165">
        <rdfs:subClassOf rdf:resource="http://purl.obolibrary.org/obo/FOODON_03470163"/>
        <oboInOwl:hasDbXref rdf:datatype="http://www.w3.org/2001/XMLSchema#string">http://www.langual.org/langual_thesaurus.asp?termid=J0165</oboInOwl:hasDbXref>
        <rdfs:comment xml:lang="en">LanguaL curation note: Used when the water activity is lowered enough by microwave radiation in order to achieve preservation. Also index *WATER REMOVED* in facet H - Treatment applied. Example: tea.</rdfs:comment>
        <rdfs:label xml:lang="en">drying by microwave radiation</rdfs:label>
    </owl:Class>
    


    <!-- http://purl.obolibrary.org/obo/FOODON_03470166 -->

    <owl:Class rdf:about="http://purl.obolibrary.org/obo/FOODON_03470166">
        <rdfs:subClassOf rdf:resource="http://purl.obolibrary.org/obo/FOODON_03470143"/>
        <oboInOwl:hasDbXref rdf:datatype="http://www.w3.org/2001/XMLSchema#string">http://www.langual.org/langual_thesaurus.asp?termid=J0166</oboInOwl:hasDbXref>
        <rdfs:comment xml:lang="en">LanguaL curation note: Used when susceptible materials are dried by electromagnetic radiation with wave-lengths between 0.76um and 1 mm.</rdfs:comment>
        <rdfs:label xml:lang="en">drying by infrared heat radiation</rdfs:label>
    </owl:Class>
    


    <!-- http://purl.obolibrary.org/obo/FOODON_03470168 -->

    <owl:Class rdf:about="http://purl.obolibrary.org/obo/FOODON_03470168">
        <rdfs:subClassOf rdf:resource="http://purl.obolibrary.org/obo/FOODON_03470144"/>
        <oboInOwl:hasDbXref rdf:datatype="http://www.w3.org/2001/XMLSchema#string">http://www.langual.org/langual_thesaurus.asp?termid=J0168</oboInOwl:hasDbXref>
        <rdfs:comment xml:lang="en">LanguaL curation note: Used when a product is dehydrated under pressure. Example: vegetable or fruit juices, milk.</rdfs:comment>
        <rdfs:label xml:lang="en">drying under increased pressure</rdfs:label>
    </owl:Class>
    


    <!-- http://purl.obolibrary.org/obo/FOODON_03470169 -->

    <owl:Class rdf:about="http://purl.obolibrary.org/obo/FOODON_03470169">
        <rdfs:subClassOf rdf:resource="http://purl.obolibrary.org/obo/FOODON_03470112"/>
        <oboInOwl:hasDbXref rdf:datatype="http://www.w3.org/2001/XMLSchema#string">http://www.langual.org/langual_thesaurus.asp?termid=J0169</oboInOwl:hasDbXref>
        <rdfs:comment xml:lang="en">LanguaL curation note: Used when the water content of a product is reduced by reverse osmosis. Typically used for concentrating fluids, e.g. milk, fruit juices.</rdfs:comment>
        <rdfs:label xml:lang="en">concentration by reverse osmosis</rdfs:label>
    </owl:Class>
    


    <!-- http://purl.obolibrary.org/obo/FOODON_03470170 -->

    <owl:Class rdf:about="http://purl.obolibrary.org/obo/FOODON_03470170">
        <rdfs:subClassOf rdf:resource="http://purl.obolibrary.org/obo/FOODON_03470141"/>
        <obo:IAO_0000115 xml:lang="en">Drying by exposure to the sun. Example: cereals, spices, vegetables.</obo:IAO_0000115>
        <oboInOwl:hasDbXref rdf:datatype="http://www.w3.org/2001/XMLSchema#string">http://www.langual.org/langual_thesaurus.asp?termid=J0170</oboInOwl:hasDbXref>
        <rdfs:label xml:lang="en">sun drying</rdfs:label>
    </owl:Class>
    


    <!-- http://purl.obolibrary.org/obo/FOODON_03470171 -->

    <owl:Class rdf:about="http://purl.obolibrary.org/obo/FOODON_03470171">
        <rdfs:subClassOf rdf:resource="http://purl.obolibrary.org/obo/FOODON_03470132"/>
        <obo:IAO_0000115 xml:lang="en">Frozen very rapidly by means of refrigerating agents such as liquid nitrogen or carbon dioxide. Example: lobster frozen in liquid nitrogen.</obo:IAO_0000115>
        <oboInOwl:hasDbXref rdf:datatype="http://www.w3.org/2001/XMLSchema#string">http://www.langual.org/langual_thesaurus.asp?termid=J0171</oboInOwl:hasDbXref>
        <oboInOwl:hasExactSynonym xml:lang="en">frozen by refrigerating agent</oboInOwl:hasExactSynonym>
        <rdfs:label xml:lang="en">food cryogenic freezing</rdfs:label>
    </owl:Class>
    


    <!-- http://purl.obolibrary.org/obo/FOODON_03470172 -->

    <owl:Class rdf:about="http://purl.obolibrary.org/obo/FOODON_03470172">
        <rdfs:subClassOf rdf:resource="http://purl.obolibrary.org/obo/FOODON_03470131"/>
        <obo:IAO_0000115 xml:lang="en">The process of food storage involving an accompanying refrigerating agent.</obo:IAO_0000115>
        <obo:IAO_0000117 rdf:datatype="http://www.w3.org/2001/XMLSchema#string">Damion Dooley</obo:IAO_0000117>
        <oboInOwl:hasDbXref rdf:datatype="http://www.w3.org/2001/XMLSchema#string">http://www.langual.org/langual_thesaurus.asp?termid=J0172</oboInOwl:hasDbXref>
        <rdfs:label xml:lang="en">food storage with refrigerating agent process</rdfs:label>
    </owl:Class>
    


    <!-- http://purl.obolibrary.org/obo/FOODON_03470173 -->

    <owl:Class rdf:about="http://purl.obolibrary.org/obo/FOODON_03470173">
        <rdfs:subClassOf rdf:resource="http://purl.obolibrary.org/obo/FOODON_03470111"/>
        <obo:IAO_0000115 xml:lang="en">Preservation by storage in inert gases (e.g. nitrogen) to suppress or inhibit undesirable micro-organism growth, oxidation activity, etc.</obo:IAO_0000115>
        <oboInOwl:hasDbXref rdf:datatype="http://www.w3.org/2001/XMLSchema#string">http://www.langual.org/langual_thesaurus.asp?termid=J0173</oboInOwl:hasDbXref>
        <rdfs:label xml:lang="en">inert atmosphere storage process</rdfs:label>
    </owl:Class>
    


    <!-- http://purl.obolibrary.org/obo/FOODON_03470174 -->

    <owl:Class rdf:about="http://purl.obolibrary.org/obo/FOODON_03470174">
        <rdfs:subClassOf rdf:resource="http://purl.obolibrary.org/obo/FOODON_03470111"/>
        <obo:IAO_0000115 xml:lang="en">Storing under reduced pressure (e.g. 1.3-2 kPa) in order to suppress or inhibit undesirable micro organism growth, oxidation activity, etc.</obo:IAO_0000115>
        <oboInOwl:hasDbXref rdf:datatype="http://www.w3.org/2001/XMLSchema#string">http://www.langual.org/langual_thesaurus.asp?termid=J0174</oboInOwl:hasDbXref>
        <rdfs:label xml:lang="en">vaccume storage process</rdfs:label>
    </owl:Class>
    


    <!-- http://purl.obolibrary.org/obo/FOODON_03470175 -->

    <owl:Class rdf:about="http://purl.obolibrary.org/obo/FOODON_03470175">
        <rdfs:subClassOf rdf:resource="http://purl.obolibrary.org/obo/FOODON_03450002"/>
        <rdfs:subClassOf rdf:resource="http://purl.obolibrary.org/obo/FOODON_03460130"/>
        <rdfs:subClassOf rdf:resource="http://purl.obolibrary.org/obo/FOODON_03470120"/>
        <obo:IAO_0000115 xml:lang="en">Blanching is a cooking process wherein a food, usually a vegetable or fruit, is scalded in boiling water, removed after a brief, timed interval, and finally plunged into iced water or placed under cold running water (shocking or refreshing) to halt the cooking process. Blanching foods helps reduce quality loss over time. People often use blanching as a pre-treatment prior to freezing, drying, or canning—heating vegetables or fruits to inactivate enzymes, modify texture, remove the peel, and wilt tissue. Blanching is also utilized to preserve color, flavor, and nutritional value. The process has three stages: preheating, blanching, and cooling. The most common blanching methods for vegetables/fruits are hot water and steam, while cooling is either done using cold water or cool air.</obo:IAO_0000115>
        <obo:IAO_0000117 rdf:datatype="http://www.w3.org/2001/XMLSchema#string">Damion Dooley</obo:IAO_0000117>
        <oboInOwl:hasDbXref rdf:datatype="http://www.w3.org/2001/XMLSchema#string">http://www.langual.org/langual_thesaurus.asp?termid=J0175</oboInOwl:hasDbXref>
        <oboInOwl:hasExactSynonym xml:lang="en">blanching</oboInOwl:hasExactSynonym>
        <rdfs:comment xml:lang="en">LanguaL definition: &quot;Short time scalding; this can be used to stop emzymatic activity for vegetables being prepared for freezing.</rdfs:comment>
        <rdfs:label xml:lang="en">food blanching</rdfs:label>
    </owl:Class>
    


    <!-- http://purl.obolibrary.org/obo/FOODON_03470176 -->

    <owl:Class rdf:about="http://purl.obolibrary.org/obo/FOODON_03470176">
        <rdfs:subClassOf rdf:resource="http://purl.obolibrary.org/obo/FOODON_03470111"/>
        <obo:IAO_0000115 xml:lang="en">Storage of fruits and vegetables in an atmosphere in which the concentrations of oxygen, carbon dioxide (and often nitrogen) are different from those in air and at a low temperature. All three (four) factors are controlled at the desired levels in order to suppress the fruits&apos; and vegetables&apos; natural respiration.</obo:IAO_0000115>
        <oboInOwl:hasDbXref rdf:datatype="http://www.w3.org/2001/XMLSchema#string">http://www.langual.org/langual_thesaurus.asp?termid=J0176</oboInOwl:hasDbXref>
        <oboInOwl:hasExactSynonym xml:lang="en">CA | CA storage</oboInOwl:hasExactSynonym>
        <rdfs:label xml:lang="en">controlled atmosphere storage process</rdfs:label>
    </owl:Class>
    


    <!-- http://purl.obolibrary.org/obo/FOODON_03470177 -->

    <owl:Class rdf:about="http://purl.obolibrary.org/obo/FOODON_03470177">
        <rdfs:subClassOf rdf:resource="http://purl.obolibrary.org/obo/FOODON_03470121"/>
        <obo:IAO_0000115 xml:lang="en">Microfiltration is used to remove undesirable micro-organisms and molecules. The membranes have pore diameters from 10 to 10000 nm. Micro-filtration is often used instead of pateurisation, e.g. in the brewing industry.</obo:IAO_0000115>
        <oboInOwl:hasDbXref rdf:datatype="http://www.w3.org/2001/XMLSchema#string">http://www.langual.org/langual_thesaurus.asp?termid=J0177</oboInOwl:hasDbXref>
        <rdfs:label xml:lang="en">food micro-filtration</rdfs:label>
    </owl:Class>
    


    <!-- http://purl.obolibrary.org/obo/FOODON_03470178 -->

    <owl:Class rdf:about="http://purl.obolibrary.org/obo/FOODON_03470178">
        <rdfs:subClassOf rdf:resource="http://purl.obolibrary.org/obo/FOODON_03470135"/>
        <obo:IAO_0000115 xml:lang="en">High Temperature Short Time (HTST) pasteurization is one of the most common methods of pasteurization , which uses metal plates and hot water to raise milk temperatures to at least 72° C (161° F) for not less than 15 seconds, followed by rapid cooling.</obo:IAO_0000115>
        <oboInOwl:hasDbXref rdf:datatype="http://www.w3.org/2001/XMLSchema#string">http://www.langual.org/langual_thesaurus.asp?termid=J0178</oboInOwl:hasDbXref>
        <oboInOwl:hasExactSynonym xml:lang="en">HTST</oboInOwl:hasExactSynonym>
        <rdfs:label xml:lang="en">high temperature short time (HTST) pasteurization</rdfs:label>
    </owl:Class>
    


    <!-- http://purl.obolibrary.org/obo/FOODON_03470179 -->

    <owl:Class rdf:about="http://purl.obolibrary.org/obo/FOODON_03470179">
        <rdfs:subClassOf rdf:resource="http://purl.obolibrary.org/obo/FOODON_03470135"/>
        <obo:IAO_0000115 xml:lang="en">Higher Heat Shorter Time (HHST) is a process similar to HTST pasteurization, but it uses slightly different equipment and higher temperatures (83 - 127° C) for a shorter time.</obo:IAO_0000115>
        <oboInOwl:hasDbXref rdf:datatype="http://www.w3.org/2001/XMLSchema#string">http://www.langual.org/langual_thesaurus.asp?termid=J0179</oboInOwl:hasDbXref>
        <oboInOwl:hasExactSynonym xml:lang="en">HHST</oboInOwl:hasExactSynonym>
        <rdfs:label xml:lang="en">higher heat shorter time (HHST) pasteurization</rdfs:label>
    </owl:Class>
    


    <!-- http://purl.obolibrary.org/obo/FOODON_03470180 -->

    <owl:Class rdf:about="http://purl.obolibrary.org/obo/FOODON_03470180">
        <rdfs:subClassOf rdf:resource="http://purl.obolibrary.org/obo/FOODON_03470135"/>
        <obo:IAO_0000115 xml:lang="en">Typically involves heating milk or cream to 135° to 150° C (275° to 302° F) for 1 or 2 seconds. The milk is then packaged in sterile, hermetically-sealed (airtight) containers (aspetic filling) and can be stored without refrigeration for up to 90 days. After opening, spoilage times for UHT products are similar to those of conventionally pasteurized products.</obo:IAO_0000115>
        <oboInOwl:hasDbXref rdf:datatype="http://www.w3.org/2001/XMLSchema#string">http://www.langual.org/langual_thesaurus.asp?termid=J0180</oboInOwl:hasDbXref>
        <oboInOwl:hasExactSynonym xml:lang="en">UHT</oboInOwl:hasExactSynonym>
        <rdfs:label xml:lang="en">ultra high temperature (UHT) pasteurization</rdfs:label>
    </owl:Class>
    


    <!-- http://purl.obolibrary.org/obo/FOODON_03470181 -->

    <owl:Class rdf:about="http://purl.obolibrary.org/obo/FOODON_03470181">
        <rdfs:subClassOf rdf:resource="http://purl.obolibrary.org/obo/FOODON_03470135"/>
        <oboInOwl:hasDbXref rdf:datatype="http://www.w3.org/2001/XMLSchema#string">http://www.langual.org/langual_thesaurus.asp?termid=J0181</oboInOwl:hasDbXref>
        <rdfs:comment xml:lang="en">LanguaL curation note: This term is for CLASSIFICATION ONLY; DO NOT USE term in indexing. Use a more precise narrower term.</rdfs:comment>
        <rdfs:label xml:lang="en">filling conditions for pasteurization</rdfs:label>
    </owl:Class>
    


    <!-- http://purl.obolibrary.org/obo/FOODON_03470182 -->

    <owl:Class rdf:about="http://purl.obolibrary.org/obo/FOODON_03470182">
        <rdfs:subClassOf rdf:resource="http://purl.obolibrary.org/obo/FOODON_03470135"/>
        <obo:IAO_0000115 xml:lang="en">Low-Temperature-Long-Time Treatment (LTLT) uses low heat for a longer time to kill pathogenic bacteria. For example, milk is pasteurized at 63° C (145° F) for 30 minutes.</obo:IAO_0000115>
        <oboInOwl:hasDbXref rdf:datatype="http://www.w3.org/2001/XMLSchema#string">http://www.langual.org/langual_thesaurus.asp?termid=J0182</oboInOwl:hasDbXref>
        <oboInOwl:hasExactSynonym xml:lang="en">batch pasteurization | holding pasteurization | LTLT</oboInOwl:hasExactSynonym>
        <rdfs:label xml:lang="en">low-temperature-long-time (LTLT) pasteurization</rdfs:label>
    </owl:Class>
</rdf:RDF>



<!-- Generated by the OWL API (version 4.5.9.2019-02-01T07:24:44Z) https://github.com/owlcs/owlapi -->

